@prefix icd-kg: <http://icd_kg/6/ontology/> .
@prefix icd-schema: <http://id.who.int/icd/schema/> .
@prefix owl: <http://www.w3.org/2002/07/owl#> .
@prefix rdfs: <http://www.w3.org/2000/01/rdf-schema#> .
@prefix schema: <https://schema.org/> .
@prefix skos: <http://www.w3.org/2004/02/skos/core#> .
@prefix xsd: <http://www.w3.org/2001/XMLSchema#> .

icd-kg:Acute_and_transient_psychotic_first_episode a owl:Class ;
    rdfs:subClassOf icd-kg:Acute_and_transient_psychotic ;
    skos:definition "Acute and transient psychotic disorder, first episode should be used to identify individuals experiencing symptoms that meet the diagnostic requirements for acute and transient psychotic disorder but who have never before experienced a similar episode."^^xsd:string ;
    skos:prefLabel "Acute and transient psychotic first episode"^^xsd:string .

icd-kg:Acute_and_transient_psychotic_multiple_episodes a owl:Class ;
    rdfs:subClassOf icd-kg:Acute_and_transient_psychotic ;
    skos:definition "Acute and transient psychotic disorder, multiple episodes should be used to identify individuals experiencing symptoms that meet the diagnostic requirements for acute and transient psychotic disorder and who have experienced similar episodes in the past."^^xsd:string ;
    skos:prefLabel "Acute and transient psychotic multiple episodes"^^xsd:string .

icd-kg:Acute_intoxication_fentanyl a owl:Class ;
    rdfs:subClassOf icd-kg:Opioid_intoxication ;
    skos:prefLabel "Acute intoxication fentanyl"^^xsd:string .

icd-kg:Agoraphobia a owl:Class ;
    rdfs:subClassOf icd-kg:Anxiety_or_fearrelated ;
    skos:definition "Agoraphobia is characterised by marked and excessive fear or anxiety that occurs in response to multiple situations where escape might be difficult or help might not be available, such as using public transportation, being in crowds, being outside the home alone (e.g., in shops, theatres, standing in line). The individual is consistently anxious about these situations due to a fear of specific negative outcomes (e.g., panic attacks, other incapacitating or embarrassing physical symptoms). The situations are actively avoided, entered only under specific circumstances such as in the presence of a trusted companion, or endured with intense fear or anxiety. The symptoms persist for at least several months, and are sufficiently severe to result in significant distress or significant impairment in personal, family, social, educational, occupational, or other important areas of functioning."^^xsd:string ;
    skos:prefLabel "Agoraphobia"^^xsd:string .

icd-kg:Alcohol_intoxication a owl:Class ;
    icd-schema:exclusion <http://id.who.int/icd/entity/1950708583> ;
    rdfs:subClassOf icd-kg:Alcohol ;
    skos:definition "Alcohol intoxication is a clinically significant transient condition that develops during or shortly after the consumption of alcohol that is characterised by disturbances in consciousness, cognition, perception, affect, behaviour, or coordination. These disturbances are caused by the known pharmacological effects of alcohol and their intensity is closely related to the amount of alcohol consumed. They are time-limited and abate as alcohol is cleared from the body. Presenting features may include impaired attention, inappropriate or aggressive behaviour, lability of mood and emotions, impaired judgment, poor coordination, unsteady gait, fine nystagmus and slurred speech. At more severe levels of intoxication, stupor or coma may occur. Alcohol intoxication may facilitate suicidal ideation or behaviour."^^xsd:string ;
    skos:prefLabel "Alcohol intoxication"^^xsd:string .

icd-kg:Alcohol_withdrawal_with_seizures a owl:Class ;
    rdfs:subClassOf icd-kg:Alcohol_withdrawal ;
    skos:definition "All diagnostic requirements for Alcohol withdrawal are met and the withdrawal state is accompanied by seizures (i.e., generalised tonic-clonic seizures) but not by perceptual disturbances."^^xsd:string ;
    skos:prefLabel "Alcohol withdrawal with seizures"^^xsd:string .

icd-kg:Alcoholinduced_mood a owl:Class ;
    rdfs:subClassOf icd-kg:Certain_specified_alcoholinduced_mental_or_behavioural,
        icd-kg:Substanceinduced_mood ;
    skos:definition "Alcohol-induced mood disorder is characterised by mood symptoms (e.g., depressed or elevated mood, decreased engagement in pleasurable activities, increased or decreased energy levels) that develop during or soon after intoxication with or withdrawal from alcohol. The intensity or duration of the symptoms is substantially in excess of mood disturbances that are characteristic of Alcohol intoxication or Alcohol withdrawal. The amount and duration of alcohol use must be capable of producing mood symptoms. The symptoms are not better explained by a primary mental disorder (e.g., a Depressive disorder, a Bipolar disorder, Schizoaffective disorder), as might be the case if the mood symptoms preceded the onset of the alcohol use, if the symptoms persist for a substantial period of time after cessation of the alcohol use or withdrawal, or if there is other evidence of a pre-existing primary mental disorder with mood symptoms (e.g., a history of prior episodes not associated with alcohol use)."^^xsd:string ;
    skos:prefLabel "Alcoholinduced mood"^^xsd:string .

icd-kg:Alcoholinduced_psychotic a owl:Class ;
    rdfs:subClassOf icd-kg:Alcohol,
        icd-kg:Substanceinduced_psychotic ;
    skos:definition "Alcohol-induced psychotic disorder is characterised by psychotic symptoms (e.g. delusions, hallucinations, disorganised thinking, grossly disorganised behaviour) that develop during or soon after intoxication with or withdrawal from alcohol. The intensity or duration of the symptoms is substantially in excess of psychotic-like disturbances of perception, cognition, or behaviour that are characteristic of Alcohol intoxication or Alcohol withdrawal. The amount and duration of alcohol use must be capable of producing psychotic symptoms. The symptoms are not better explained by a primary mental disorder (e.g. Schizophrenia, a Mood disorder with psychotic symptoms), as might be the case if the psychotic symptoms preceded the onset of the alcohol use, if the symptoms persist for a substantial period of time after cessation of the alcohol use or withdrawal, or if there is other evidence of a pre-existing primary mental disorder with psychotic symptoms (e.g. a history of prior episodes not associated with alcohol use)."^^xsd:string ;
    skos:prefLabel "Alcoholinduced psychotic"^^xsd:string .

icd-kg:Amnestic_psychoactive_substances_including_medications a owl:Class ;
    rdfs:subClassOf icd-kg:Amnestic ;
    skos:definition "All definitional requirements for amnestic disorder are met. The memory symptoms are judged to be the direct consequence of psychoactive substance use. The intensity and duration of substance use must be known to be capable of producing memory impairment. The memory impairment may develop during or soon after substance intoxication or withdrawal, but its intensity and duration are substantially in excess of those normally associated with these conditions. The symptoms are not better accounted for by another disorder or medical condition, as might be the case if the amnestic symptoms preceded the onset of substance use."^^xsd:string ;
    skos:prefLabel "Amnestic psychoactive substances including medications"^^xsd:string .

icd-kg:Anorexia_nervosa_with_dangerously_low_body_weight a owl:Class ;
    rdfs:subClassOf icd-kg:Anorexia_nervosa ;
    skos:definition "Anorexia Nervosa with dangerously low body weight meets all definitional requirements for Anorexia Nervosa, with BMI under 14.0 kg/m² in adults or under the 0.3rd percentile for BMI-for-age in children and adolescents. In the context of Anorexia Nervosa, severe underweight status is an important prognostic factor that is associated with high risk of physical complications and substantially increased mortality."^^xsd:string ;
    skos:prefLabel "Anorexia nervosa with dangerously low body weight"^^xsd:string .

icd-kg:Anorexia_nervosa_with_significantly_low_body_weight a owl:Class ;
    rdfs:subClassOf icd-kg:Anorexia_nervosa ;
    skos:definition "Anorexia Nervosa with significantly low body weight meets all definitional requirements for Anorexia Nervosa, with BMI between 18.5 kg/m2 and 14.0 kg/m² for adults or between the fifth percentile and the 0.3 percentile for BMI-for-age in children and adolescents."^^xsd:string ;
    skos:prefLabel "Anorexia nervosa with significantly low body weight"^^xsd:string .

icd-kg:Anorgasmia a owl:Class ;
    icd-schema:inclusion "Psychogenic anorgasmy"^^xsd:string ;
    rdfs:subClassOf icd-kg:Orgasmic_dysfunctions ;
    skos:definition "Anorgasmia is characterised by the absence or marked infrequency of the orgasm experience or markedly diminished intensity of orgasmic sensations. In women, this includes a marked delay in orgasm, which in men would be diagnosed as Male Delayed Ejaculation. The pattern of absence, delay, or diminished frequency or intensity of orgasm occurs despite adequate sexual stimulation, including the desire for sexual activity and orgasm, has occurred episodically or persistently over a period at least several months, and is associated with clinically significant distress."^^xsd:string ;
    skos:prefLabel "Anorgasmia"^^xsd:string .

icd-kg:Antisocial_personality a owl:Class ;
    rdfs:subClassOf icd-kg:Personality ;
    skos:definition "Personality disorder characterised by disregard for social obligations, and callous unconcern for the feelings of others. There is gross disparity between behaviour and the prevailing social norms. Behaviour is not readily modifiable by adverse experience, including punishment. There is a low tolerance to frustration and a low threshold for discharge of aggression, including violence; there is a tendency to blame others, or to offer plausible rationalizations for the behaviour bringing the patient into conflict with society."^^xsd:string ;
    skos:prefLabel "Antisocial personality"^^xsd:string .

icd-kg:Attention_deficit_hyperactivity a owl:Class ;
    icd-schema:inclusion "attention deficit disorder with hyperactivity"^^xsd:string,
        "attention deficit syndrome with hyperactivity"^^xsd:string ;
    rdfs:subClassOf icd-kg:Neurodevelopmental ;
    skos:definition "Attention deficit hyperactivity disorder is characterised by a persistent pattern (at least 6 months) of inattention and/or hyperactivity-impulsivity that has a direct negative impact on academic, occupational, or social functioning. There is evidence of significant inattention and/or hyperactivity-impulsivity symptoms prior to age 12, typically by early to mid-childhood, though some individuals may first come to clinical attention later. The degree of inattention and hyperactivity-impulsivity is outside the limits of normal variation expected for age and level of intellectual functioning. Inattention refers to significant difficulty in sustaining attention to tasks that do not provide a high level of stimulation or frequent rewards, distractibility and problems with organisation. Hyperactivity refers to excessive motor activity and difficulties with remaining still, most evident in structured situations that require behavioural self-control. Impulsivity is a tendency to act in response to immediate stimuli, without deliberation or consideration of the risks and consequences. The relative balance and the specific manifestations of inattentive and hyperactive-impulsive characteristics varies across individuals and may change over the course of development. In order for a diagnosis to be made, manifestations of inattention and/or hyperactivity-impulsivity must be evident across multiple situations or settings (e.g., home, school, work, with friends or relatives), but are likely to vary according to the structure and demands of the setting. Symptoms are not better accounted for by another mental, behavioural, or neurodevelopmental disorder and are not due to the effect of a substance or medication."^^xsd:string ;
    skos:prefLabel "Attention deficit hyperactivity"^^xsd:string .

icd-kg:Autism_spectrum_with_of_intellectual_development_and_with_absence_of_functional_language a owl:Class ;
    rdfs:subClassOf icd-kg:Autism_spectrum ;
    skos:definition "All definitional requirements for both autism spectrum disorder and disorder of intellectual development are met and there is complete, or almost complete, absence of ability relative to the individual’s age to use functional language (spoken or signed) for instrumental purposes, such as to express personal needs and desires"^^xsd:string ;
    skos:prefLabel "Autism spectrum with of intellectual development and with absence of functional language"^^xsd:string .

icd-kg:Autism_spectrum_with_of_intellectual_development_and_with_impaired_functional_language_with_loss_of_previously_acquired_skills a owl:Class ;
    rdfs:subClassOf icd-kg:Autism_spectrum_with_of_intellectual_development_and_with_impaired_functional_language ;
    skos:definition "All definitional requirements for both autism spectrum disorder and disorder of intellectual development are met and there is marked impairment in functional language (spoken or signed) relative to the individual’s age, with the individual not able to use more than single words or simple phrases for instrumental purposes, such as to express personal needs and desires. In addition, the individual’s clinical history includes a loss of previously acquired skills, most commonly the loss of language and social skills during the second year of life. Loss of previously acquired skills is rare after three years of age, and when it occurs is more likely to involve cognitive and adaptive skills (e.g., loss of bowel and bladder control, impaired sleep) and to present together with increasing emotional and behavioural disturbance."^^xsd:string ;
    skos:prefLabel "Autism spectrum with of intellectual development and with impaired functional language with loss of previously acquired skills"^^xsd:string .

icd-kg:Autism_spectrum_with_of_intellectual_development_and_with_mild_or_no_impairment_of_functional_language a owl:Class ;
    rdfs:subClassOf icd-kg:Autism_spectrum ;
    skos:definition "All definitional requirements for both autism spectrum disorder and disorder of intellectual development are met and there is only mild or no impairment in the individual's capacity to use functional language (spoken or signed) for instrumental purposes, such as to express personal needs and desires."^^xsd:string ;
    skos:prefLabel "Autism spectrum with of intellectual development and with mild or no impairment of functional language"^^xsd:string .

icd-kg:Autism_spectrum_without_of_intellectual_development_and_with_absence_of_functional_language a owl:Class ;
    rdfs:subClassOf icd-kg:Autism_spectrum ;
    skos:definition "All definitional requirements for autism spectrum disorder are met, intellectual functioning and adaptive behaviour are found to be at least within the average range (approximately greater than the 2.3rd percentile), and there is complete, or almost complete, absence of ability relative to the individual’s age to use functional language (spoken or signed) for instrumental purposes, such as to express personal needs and desires."^^xsd:string ;
    skos:prefLabel "Autism spectrum without of intellectual development and with absence of functional language"^^xsd:string .

icd-kg:Autism_spectrum_without_of_intellectual_development_and_with_impaired_functional_language a owl:Class ;
    rdfs:subClassOf icd-kg:Autism_spectrum ;
    skos:definition "All definitional requirements for autism spectrum disorder are met, intellectual functioning and adaptive behaviour are found to be at least within the average range (approximately greater than the 2.3rd percentile), and there is marked impairment in functional language (spoken or signed) relative to the individual’s age, with the individual not able to use more than single words or simple phrases for instrumental purposes, such as to express personal needs and desires."^^xsd:string ;
    skos:prefLabel "Autism spectrum without of intellectual development and with impaired functional language"^^xsd:string .

icd-kg:Autism_spectrum_without_of_intellectual_development_and_with_mild_or_no_impairment_of_functional_language a owl:Class ;
    rdfs:subClassOf icd-kg:Autism_spectrum ;
    skos:definition "All definitional requirements for autism spectrum disorder are met, intellectual functioning and adaptive behaviour are found to be at least within the average range (approximately greater than the 2.3rd percentile), and there is only mild or no impairment in the individual's capacity to use functional language (spoken or signed) for instrumental purposes, such as to express personal needs and desires."^^xsd:string ;
    skos:prefLabel "Autism spectrum without of intellectual development and with mild or no impairment of functional language"^^xsd:string .

icd-kg:Behavioural_or_psychological_disturbances_in_dementia a owl:Class ;
    icd-schema:exclusion icd-kg:Secondary_mental_or_behavioural_syndromes_associated_with_or_diseases_classified_elsewhere ;
    rdfs:subClassOf icd-kg:Dementia ;
    skos:definition "In addition to the cognitive disturbances characteristic of dementia, the current clinical picture includes clinically significant behavioural or psychological disturbances."^^xsd:string ;
    skos:prefLabel "Behavioural or psychological disturbances in dementia"^^xsd:string .

icd-kg:Bipolar_type_i_current_episode_depressive_mild a owl:Class ;
    rdfs:subClassOf icd-kg:Bipolar_type_i ;
    skos:definition "Bipolar type I disorder, current episode depressive, mild is diagnosed when the definitional requirements for Bipolar type I disorder have been met and the current episode is depressive at a mild level of severity. A depressive episode is characterised by a period of depressed mood or diminished interest in activities occurring most of the day, nearly every day during a period lasting at least two weeks accompanied by other symptoms such as difficulty concentrating, feelings of worthlessness or excessive or inappropriate guilt, hopelessness, recurrent thoughts of death or suicide, changes in appetite or sleep, psychomotor agitation or retardation, and reduced energy or fatigue. In a mild depressive episode, the individual is usually distressed by the symptoms and has some difficulty in continuing to function in one or more domains (personal, family, social, educational, occupational, or other important domains). There are no delusions or hallucinations during the episode."^^xsd:string ;
    skos:prefLabel "Bipolar type i current episode depressive mild"^^xsd:string .

icd-kg:Bipolar_type_i_current_episode_depressive_moderate_with_psychotic_symptoms a owl:Class ;
    rdfs:subClassOf icd-kg:Bipolar_type_i ;
    skos:definition "Bipolar type I disorder, current episode depressive, moderate, with psychotic symptoms diagnosed when the definitional requirements for Bipolar type I disorder have been met and the current episode is depressive at a moderate level of severity and there are delusions or hallucinations during the episode. A depressive episode is characterised by a period of depressed mood or diminished interest in activities occurring most of the day, nearly every day during a period lasting at least two weeks accompanied by other symptoms such as difficulty concentrating, feelings of worthlessness or excessive or inappropriate guilt, hopelessness, recurrent thoughts of death or suicide, changes in appetite or sleep, psychomotor agitation or retardation, and reduced energy or fatigue. In a moderate depressive episode, several symptoms of a depressive episode are present to a marked degree, or a large number of depressive symptoms of lesser severity are present overall. The individual typically has considerable difficulty functioning in multiple domains (personal, family, social, educational, occupational, or other important domains)."^^xsd:string ;
    skos:prefLabel "Bipolar type i current episode depressive moderate with psychotic symptoms"^^xsd:string .

icd-kg:Bipolar_type_i_current_episode_depressive_moderate_without_psychotic_symptoms a owl:Class ;
    rdfs:subClassOf icd-kg:Bipolar_type_i ;
    skos:definition "Bipolar type I disorder, current episode depressive, moderate, without psychotic symptoms is diagnosed when the definitional requirements for Bipolar type I disorder have been met and the current episode is depressive at a moderate level of severity and there are no delusions or hallucinations during the episode. A depressive episode is characterised by a period of depressed mood or diminished interest in activities occurring most of the day, nearly every day during a period lasting at least two weeks accompanied by other symptoms such as difficulty concentrating, feelings of worthlessness or excessive or inappropriate guilt, hopelessness, recurrent thoughts of death or suicide, changes in appetite or sleep, psychomotor agitation or retardation, and reduced energy or fatigue. In a moderate depressive episode, several symptoms of a depressive episode are present to a marked degree, or a large number of depressive symptoms of lesser severity are present overall. The individual typically has considerable difficulty functioning in multiple domains (personal, family, social, educational, occupational, or other important domains)."^^xsd:string ;
    skos:prefLabel "Bipolar type i current episode depressive moderate without psychotic symptoms"^^xsd:string .

icd-kg:Bipolar_type_i_current_episode_depressive_severe_with_psychotic_symptoms a owl:Class ;
    rdfs:subClassOf icd-kg:Bipolar_type_i ;
    skos:definition "Bipolar type I disorder, current episode depressive, severe, with psychotic symptoms is diagnosed when the definitional requirements for Bipolar type I disorder are met and the current episode is severe and there are delusions or hallucinations during the episode. A depressive episode is characterised by a period of depressed mood or diminished interest in activities occurring most of the day, nearly every day during a period lasting at least two weeks accompanied by other symptoms such as difficulty concentrating, feelings of worthlessness or excessive or inappropriate guilt, hopelessness, recurrent thoughts of death or suicide, changes in appetite or sleep, psychomotor agitation or retardation, and reduced energy or fatigue. In a severe depressive episode, many or most symptoms of a Depressive Episode are present to a marked degree, or a smaller number of symptoms are present and manifest to an intense degree. The individual has serious difficulty continuing to function in most domains (personal, family, social, educational, occupational, or other important domains)."^^xsd:string ;
    skos:prefLabel "Bipolar type i current episode depressive severe with psychotic symptoms"^^xsd:string .

icd-kg:Bipolar_type_i_current_episode_depressive_severe_without_psychotic_symptoms a owl:Class ;
    rdfs:subClassOf icd-kg:Bipolar_type_i ;
    skos:definition "Bipolar type I disorder, current episode depressive, severe, without psychotic symptoms is diagnosed when the definitional requirements for Bipolar type I disorder are met and the current episode is severe and there are no delusions or hallucinations during the episode. A depressive episode is characterised by a period of depressed mood or diminished interest in activities occurring most of the day, nearly every day during a period lasting at least two weeks accompanied by other symptoms such as difficulty concentrating, feelings of worthlessness or excessive or inappropriate guilt, hopelessness, recurrent thoughts of death or suicide, changes in appetite or sleep, psychomotor agitation or retardation, and reduced energy or fatigue. In a severe depressive episode, many or most symptoms of a Depressive Episode are present to a marked degree, or a smaller number of symptoms are present and manifest to an intense degree. The individual has serious difficulty continuing to function in most domains (personal, family, social, educational, occupational, or other important domains)."^^xsd:string ;
    skos:prefLabel "Bipolar type i current episode depressive severe without psychotic symptoms"^^xsd:string .

icd-kg:Bipolar_type_i_current_episode_hypomanic a owl:Class ;
    rdfs:subClassOf icd-kg:Bipolar_type_i ;
    skos:definition "Bipolar type I disorder, current episode hypomanic is diagnosed when the definitional requirements for Bipolar type I disorder have been met and the current episode is hypomanic. A hypomanic episode is a persistent mood state lasting at least several days characterised by mild elevation of mood or increased irritability and increased activity or a subjective experience of increased energy, accompanied by other characteristic symptoms such as rapid speech, rapid or racing thoughts, increased self-esteem, an increase in sexual drive or sociability, decreased need for sleep, distractibility, or impulsive or reckless behaviour. The symptoms are not severe enough to cause marked impairment in occupational functioning or in usual social activities or relationships with others, does not necessitate hospitalization, and there are no accompanying delusions or hallucinations."^^xsd:string ;
    skos:prefLabel "Bipolar type i current episode hypomanic"^^xsd:string .

icd-kg:Bipolar_type_i_current_episode_manic_with_psychotic_symptoms a owl:Class ;
    rdfs:subClassOf icd-kg:Bipolar_type_i ;
    skos:definition "Bipolar type I disorder, current episode manic with psychotic symptoms is diagnosed when the definitional requirements for Bipolar type I Disorder have been met, the current episode is Manic and there are delusions or hallucinations present during the episode. A manic episode is an extreme mood state lasting at least one week unless shortened by a treatment intervention characterised by euphoria, irritability, or expansiveness, and by increased activity or a subjective experience of increased energy, accompanied by other characteristic symptoms such as rapid or pressured speech, flight of ideas, increased self-esteem or grandiosity, decreased need for sleep, distractibility, impulsive or reckless behaviour, and rapid changes among different mood states (i.e., mood lability). If the individual has experienced Manic or Mixed Episodes in the past, a duration of one week is not required in order to diagnose a current episode if all other diagnostic requirements are met."^^xsd:string ;
    skos:prefLabel "Bipolar type i current episode manic with psychotic symptoms"^^xsd:string .

icd-kg:Bipolar_type_i_current_episode_manic_without_psychotic_symptoms a owl:Class ;
    rdfs:subClassOf icd-kg:Bipolar_type_i ;
    skos:definition "Bipolar type I disorder, current episode manic, without psychotic symptoms is diagnosed when the definitional requirements for Bipolar type I disorder are met, the current episode is manic, and there are no delusions or hallucinations present during the episode. A manic episode is an extreme mood state lasting at least one week unless shortened by a treatment intervention characterised by euphoria, irritability, or expansiveness, and by increased activity or a subjective experience of increased energy, accompanied by other characteristic symptoms such as rapid or pressured speech, flight of ideas, increased self-esteem or grandiosity, decreased need for sleep, distractibility, impulsive or reckless behaviour, and rapid changes among different mood states (i.e., mood lability). If the individual has experienced Manic or Mixed Episodes in the past, a duration of one week is not required in order to diagnose a current episode if all other diagnostic requirements are met."^^xsd:string ;
    skos:prefLabel "Bipolar type i current episode manic without psychotic symptoms"^^xsd:string .

icd-kg:Bipolar_type_i_current_episode_mixed_with_psychotic_symptoms a owl:Class ;
    rdfs:subClassOf icd-kg:Bipolar_type_i ;
    skos:definition "Bipolar type I disorder, current episode mixed, with psychotic symptoms is diagnosed when the definitional requirements for Bipolar type I disorder are met and the current episode is mixed and there are delusions or hallucinations present during the episode. A mixed episode is characterised by the presence of several prominent manic and several prominent depressive symptoms consistent with those observed in manic episodes and depressive episodes, which either occur simultaneously or alternate very rapidly (from day to day or within the same day). Symptoms must include an altered mood state consistent with a manic and/or depressive episode (i.e., depressed, dysphoric, euphoric or expansive mood), and be present most of the day, nearly every day, during a period of at least 2 weeks, unless shortened by a treatment intervention. If the individual has experienced Manic or Mixed Episodes in the past, a duration of 2 weeks is not required in order to diagnose a current episode if all other diagnostic requirements are met."^^xsd:string ;
    skos:prefLabel "Bipolar type i current episode mixed with psychotic symptoms"^^xsd:string .

icd-kg:Bipolar_type_i_current_episode_mixed_without_psychotic_symptoms a owl:Class ;
    rdfs:subClassOf icd-kg:Bipolar_type_i ;
    skos:definition "Bipolar type I disorder, current episode mixed, without psychotic symptoms is diagnosed when the definitional requirements for Bipolar type I disorder are met and the current episode is mixed and there are no delusions or hallucinations present during the episode. A mixed episode is characterised by the presence of several prominent manic and several prominent depressive symptoms consistent with those observed in manic episodes and depressive episodes, which either occur simultaneously or alternate very rapidly (from day to day or within the same day). Symptoms must include an altered mood state consistent with a manic and/or depressive episode (i.e., depressed, dysphoric, euphoric or expansive mood), and be present most of the day, nearly every day, during a period of at least 2 weeks, unless shortened by a treatment intervention. If the individual has experienced Manic or Mixed Episodes in the past, a duration of 2 weeks is not required in order to diagnose a current episode if all other diagnostic requirements are met."^^xsd:string ;
    skos:prefLabel "Bipolar type i current episode mixed without psychotic symptoms"^^xsd:string .

icd-kg:Bipolar_type_ii_current_episode_depressive_mild a owl:Class ;
    rdfs:subClassOf icd-kg:Bipolar_type_ii ;
    skos:definition "Bipolar type II disorder, current episode depressive, mild is diagnosed when the definitional requirements for Bipolar type II disorder have been met and the current episode is depressive at a mild level of severity. A depressive episode is characterised by a period of depressed mood or diminished interest in activities occurring most of the day, nearly every day during a period lasting at least two weeks accompanied by other symptoms such as difficulty concentrating, feelings of worthlessness or excessive or inappropriate guilt, hopelessness, recurrent thoughts of death or suicide, changes in appetite or sleep, psychomotor agitation or retardation, and reduced energy or fatigue. In a mild depressive episode, the individual is usually distressed by the symptoms and has some difficulty in continuing to function in one or more domains (personal, family, social, educational, occupational, or other important domains). There are no delusions or hallucinations during the episode."^^xsd:string ;
    skos:prefLabel "Bipolar type ii current episode depressive mild"^^xsd:string .

icd-kg:Bipolar_type_ii_current_episode_depressive_moderate_with_psychotic_symptoms a owl:Class ;
    rdfs:subClassOf icd-kg:Bipolar_type_ii ;
    skos:definition "Bipolar type II disorder, current episode depressive, moderate, with psychotic symptoms diagnosed when the definitional requirements for Bipolar type II disorder have been met and the current episode is depressive at a moderate level of severity and there are delusions or hallucinations during the episode. A depressive episode is characterised by a period of depressed mood or diminished interest in activities occurring most of the day, nearly every day during a period lasting at least two weeks accompanied by other symptoms such as difficulty concentrating, feelings of worthlessness or excessive or inappropriate guilt, hopelessness, recurrent thoughts of death or suicide, changes in appetite or sleep, psychomotor agitation or retardation, and reduced energy or fatigue. In a moderate depressive episode, several symptoms of a depressive episode are present to a marked degree, or a large number of depressive symptoms of lesser severity are present overall. The individual typically has considerable difficulty functioning in multiple domains (personal, family, social, educational, occupational, or other important domains)."^^xsd:string ;
    skos:prefLabel "Bipolar type ii current episode depressive moderate with psychotic symptoms"^^xsd:string .

icd-kg:Bipolar_type_ii_current_episode_depressive_moderate_without_psychotic_symptoms a owl:Class ;
    rdfs:subClassOf icd-kg:Bipolar_type_ii ;
    skos:definition "Bipolar type II disorder, current episode depressive, moderate, without psychotic symptoms is diagnosed when the definitional requirements for Bipolar type II disorder have been met and the current episode is depressive at a moderate level of severity and there are no delusions or hallucinations during the episode. A depressive episode is characterised by a period of depressed mood or diminished interest in activities occurring most of the day, nearly every day during a period lasting at least two weeks accompanied by other symptoms such as difficulty concentrating, feelings of worthlessness or excessive or inappropriate guilt, hopelessness, recurrent thoughts of death or suicide, changes in appetite or sleep, psychomotor agitation or retardation, and reduced energy or fatigue. In a moderate depressive episode, several symptoms of a depressive episode are present to a marked degree, or a large number of depressive symptoms of lesser severity are present overall. The individual typically has considerable difficulty functioning in multiple domains (personal, family, social, educational, occupational, or other important domains)."^^xsd:string ;
    skos:prefLabel "Bipolar type ii current episode depressive moderate without psychotic symptoms"^^xsd:string .

icd-kg:Bipolar_type_ii_current_episode_depressive_severe_with_psychotic_symptoms a owl:Class ;
    rdfs:subClassOf icd-kg:Bipolar_type_ii ;
    skos:definition "Bipolar type II disorder, current episode depressive, severe, with psychotic symptoms is diagnosed when the definitional requirements for Bipolar type II disorder are met and the current episode is severe and there are delusions or hallucinations during the episode. A depressive episode is characterised by a period of depressed mood or diminished interest in activities occurring most of the day, nearly every day during a period lasting at least two weeks accompanied by other symptoms such as difficulty concentrating, feelings of worthlessness or excessive or inappropriate guilt, hopelessness, recurrent thoughts of death or suicide, changes in appetite or sleep, psychomotor agitation or retardation, and reduced energy or fatigue. In a severe depressive episode, many or most symptoms of a Depressive Episode are present to a marked degree, or a smaller number of symptoms are present and manifest to an intense degree. The individual has serious difficulty continuing to function in most domains (personal, family, social, educational, occupational, or other important domains)."^^xsd:string ;
    skos:prefLabel "Bipolar type ii current episode depressive severe with psychotic symptoms"^^xsd:string .

icd-kg:Bipolar_type_ii_current_episode_depressive_severe_without_psychotic_symptoms a owl:Class ;
    rdfs:subClassOf icd-kg:Bipolar_type_ii ;
    skos:definition "Bipolar type II disorder, current episode depressive, severe, without psychotic symptoms is diagnosed when the definitional requirements for Bipolar type II disorder are met and the current episode is severe and there are no delusions or hallucinations during the episode. A depressive episode is characterised by a period of depressed mood or diminished interest in activities occurring most of the day, nearly every day during a period lasting at least two weeks accompanied by other symptoms such as difficulty concentrating, feelings of worthlessness or excessive or inappropriate guilt, hopelessness, recurrent thoughts of death or suicide, changes in appetite or sleep, psychomotor agitation or retardation, and reduced energy or fatigue. In a severe depressive episode, many or most symptoms of a Depressive Episode are present to a marked degree, or a smaller number of symptoms are present and manifest to an intense degree. The individual has serious difficulty continuing to function in most domains (personal, family, social, educational, occupational, or other important domains)."^^xsd:string ;
    skos:prefLabel "Bipolar type ii current episode depressive severe without psychotic symptoms"^^xsd:string .

icd-kg:Bipolar_type_ii_current_episode_hypomanic a owl:Class ;
    rdfs:subClassOf icd-kg:Bipolar_type_ii ;
    skos:definition "Bipolar type II disorder, current episode hypomanic is diagnosed when the definitional requirements for Bipolar type II disorder have been met and the current episode is hypomanic. A hypomanic episode is a persistent mood state lasting at least several days characterised by mild elevation of mood or increased irritability and increased activity or a subjective experience of increased energy, accompanied by other characteristic symptoms such as rapid speech, rapid or racing thoughts, increased self-esteem, an increase in sexual drive or sociability, decreased need for sleep, distractibility, or impulsive or reckless behaviour. The symptoms are not severe enough to cause marked impairment in occupational functioning or in usual social activities or relationships with others, does not necessitate hospitalization, and there are no accompanying delusions or hallucinations."^^xsd:string ;
    skos:prefLabel "Bipolar type ii current episode hypomanic"^^xsd:string .

icd-kg:Cannabisinduced_mood a owl:Class ;
    rdfs:subClassOf icd-kg:Certain_specified_cannabisinduced_mental_or_behavioural,
        icd-kg:Substanceinduced_mood ;
    skos:definition "Cannabis-induced mood disorder is characterised by mood symptoms (e.g., depressed or elevated mood, decreased engagement in pleasurable activities, increased or decreased energy levels) that develop during or soon after intoxication with or withdrawal from cannabis. The intensity or duration of the symptoms is substantially in excess of mood disturbances that are characteristic of Cannabis intoxication or Cannabis withdrawal. The amount and duration of cannabis use must be capable of producing mood symptoms. The symptoms are not better explained by a primary mental disorder (e.g., a Depressive disorder, a Bipolar disorder, Schizoaffective disorder), as might be the case if the mood symptoms preceded the onset of the cannabis use, if the symptoms persist for a substantial period of time after cessation of the cannabis use or withdrawal, or if there is other evidence of a pre-existing primary mental disorder with mood symptoms (e.g., a history of prior episodes not associated with cannabis use)."^^xsd:string ;
    skos:prefLabel "Cannabisinduced mood"^^xsd:string .

icd-kg:Catatonia_induced_by_substances_or_medications a owl:Class ;
    icd-schema:exclusion <http://id.who.int/icd/entity/498240876>,
        <http://id.who.int/icd/entity/678764364> ;
    rdfs:subClassOf icd-kg:Catatonia,
        icd-kg:Substance_use ;
    skos:definition "Catatonia induced by substances or medications is a syndrome of primarily psychomotor disturbances, characterized by the co-occurrence of several symptoms of decreased, increased, or abnormal psychomotor activity, which develops during or soon after intoxication or withdrawal from certain psychoactive substances, including phencyclidine (PCP), cannabis, hallucinogens such as mescaline or LSD, cocaine and MDMA or related drugs, or during the use of certain psychoactive and non-psychoactive medications (e.g. antipsychotic medications, benzodiazepines, steroids, disulfiram, ciprofloxacin)."^^xsd:string ;
    skos:prefLabel "Catatonia induced by substances or medications"^^xsd:string .

icd-kg:Central_sleep_apnoeas a owl:Class ;
    icd-schema:exclusion <http://id.who.int/icd/entity/252052617> ;
    rdfs:subClassOf icd-kg:Sleeprelated_breathing ;
    skos:definition """Central sleep apnoeas are characterised by reduction or cessation of airflow due to absent or reduced respiratory effort. Central apnoea (cessation of airflow) or hypopnea (reduction in airflow) may occur in a cyclical or intermittent fashion. Patients with central sleep apnoea of various etiologies may also exhibit obstructive events, in which case diagnoses of both central sleep apnoea and obstructive sleep apnoea may be given.

Note: A definitive diagnosis requires objective evidence based on polysomnography."""^^xsd:string ;
    skos:prefLabel "Central sleep apnoeas"^^xsd:string .

icd-kg:Certain_specified_caffeineinduced_mental_or_behavioural a owl:Class ;
    rdfs:subClassOf icd-kg:Caffeine ;
    skos:prefLabel "Certain specified caffeineinduced mental or behavioural"^^xsd:string .

icd-kg:Certain_specified_primary_degenerative_dementias a owl:Class ;
    rdfs:subClassOf icd-kg:Dementia_diseases_classified_elsewhere ;
    skos:prefLabel "Certain specified primary degenerative dementias"^^xsd:string .

icd-kg:Circadian_rhythm_sleepwake a owl:Class ;
    rdfs:subClassOf icd-kg:Sleepwake ;
    skos:definition "Circadian rhythm sleep-wake disorders are disturbances of the sleep-wake cycle (typically manifest as insomnia, excessive sleepiness, or both) due to alterations of the circadian time-keeping system, its entrainment mechanisms, or a misalignment of the endogenous circadian rhythm and the external environment. Sleep logs and, if possible, actigraphy for a minimum of one week should be utilized to define the specific sleep-wake schedule disturbance."^^xsd:string ;
    skos:prefLabel "Circadian rhythm sleepwake"^^xsd:string .

icd-kg:Conductdissocial_adolescent_onset a owl:Class ;
    rdfs:subClassOf icd-kg:Conductdissocial ;
    skos:definition "Conduct-dissocial disorder, adolescent onset is characterised by a repetitive and persistent pattern of behaviour in which the basic rights of others or major age-appropriate societal norms, rules, or laws are violated such as aggression towards people or animals; destruction of property; deceitfulness or theft; and serious violations of rules. No features of the disorder are present during childhood prior to adolescence (e.g., before 10 years of age). To be diagnosed, the behaviour pattern must be enduring over a significant period of time (e.g., 12 months or more). Isolated dissocial or criminal acts are thus not in themselves grounds for the diagnosis."^^xsd:string ;
    skos:prefLabel "Conductdissocial adolescent onset"^^xsd:string .

icd-kg:Conductdissocial_childhood_onset a owl:Class ;
    rdfs:subClassOf icd-kg:Conductdissocial ;
    skos:definition "Conduct-dissocial disorder, childhood onset is characterised by a repetitive and persistent pattern of behaviour in which the basic rights of others or major age-appropriate societal norms, rules, or laws are violated such as aggression towards people or animals; destruction of property; deceitfulness or theft; and serious violations of rules. To be diagnosed, features of the disorder must be present during childhood prior to adolescence (e.g., before 10 years of age) and the behaviour pattern must be enduring over a significant period of time (e.g., 12 months or more). Isolated dissocial or criminal acts are thus not in themselves grounds for the diagnosis."^^xsd:string ;
    skos:prefLabel "Conductdissocial childhood onset"^^xsd:string .

icd-kg:Delusional a owl:Class ;
    rdfs:subClassOf icd-kg:Schizophrenia_or_other_primary_psychotic ;
    skos:definition "Delusional disorder is characterised by the development of a delusion or set of related delusions, typically persisting for at least 3 months and often much longer, in the absence of a Depressive, Manic, or Mixed mood episode. The delusions are variable in content across individuals, but typically stable within individuals, although they may evolve over time. Other characteristic symptoms of Schizophrenia (i.e. clear and persistent hallucinations, negative symptoms, disorganised thinking, or experiences of influence, passivity, or control) are not present, although various forms of perceptual disturbances (e.g. hallucinations, illusions, misidentifications of persons) thematically related to the delusion are still consistent with the diagnosis. Apart from actions and attitudes directly related to the delusion or delusional system, affect, speech, and behavior are typically unaffected. The symptoms are not a manifestation of another medical condition (e.g., a brain tumour) and are not due to the effect of a substance or medication on the central nervous system (e.g. corticosteroids), including withdrawal effects (e.g. alcohol withdrawal)."^^xsd:string ;
    skos:prefLabel "Delusional"^^xsd:string .

icd-kg:Dementia_alzheimer_disease_with_early_onset a owl:Class ;
    rdfs:subClassOf icd-kg:Dementia_alzheimer_disease ;
    skos:definition "Dementia due to Alzheimer disease in which symptoms emerge before the age of 65 years. It is relatively rare, representing less than 5% of all cases, and may be genetically determined (autosomal dominant Alzheimer disease). Clinical presentation may be similar to cases with later onset, but progression of cognitive deficits may be more rapid."^^xsd:string ;
    skos:prefLabel "Dementia alzheimer disease with early onset"^^xsd:string .

icd-kg:Dementia_certain_specified_central_nervous_system_degenerative_diseases a owl:Class ;
    rdfs:subClassOf icd-kg:Dementia_diseases_classified_elsewhere ;
    skos:prefLabel "Dementia certain specified central nervous system degenerative diseases"^^xsd:string .

icd-kg:Dementia_certain_specified_infectious_diseases a owl:Class ;
    rdfs:subClassOf icd-kg:Dementia_diseases_classified_elsewhere ;
    skos:definition "None of these are specific syndromes, though can cause dementia."^^xsd:string ;
    skos:prefLabel "Dementia certain specified infectious diseases"^^xsd:string .

icd-kg:Dementia_chromosomal_anomalies a owl:Class ;
    rdfs:subClassOf icd-kg:Dementia_diseases_classified_elsewhere ;
    skos:prefLabel "Dementia chromosomal anomalies"^^xsd:string .

icd-kg:Dementia_metabolic_abnormalities a owl:Class ;
    rdfs:subClassOf icd-kg:Dementia_diseases_classified_elsewhere ;
    skos:definition "Dementia due to primary metabolic disorders involving the brain such as an adrenoleukodystrophy, Wilson's disease or MELAS (mitochondrial encephalomyopathy, lactic acidosis and stroke-like episodes) and there is evidence from history, physical examination, or laboratory findings that the disturbance is caused by the direct physiological consequences of the metabolic disorder. The identified etiology should be classified separately."^^xsd:string ;
    skos:prefLabel "Dementia metabolic abnormalities"^^xsd:string .

icd-kg:Dementia_nutritional_deficiency a owl:Class ;
    rdfs:subClassOf icd-kg:Dementia_diseases_classified_elsewhere ;
    skos:definition "Mixed evidence offers weak support for a link between PTH, cognition and dementia due to the paucity of high quality research in this area."^^xsd:string ;
    skos:prefLabel "Dementia nutritional deficiency"^^xsd:string .

icd-kg:Dementia_prion_disease a owl:Class ;
    rdfs:subClassOf icd-kg:Dementia_certain_specified_of_the_central_nervous_system ;
    skos:definition "Dementia due to prion disease is a primary neurodegenerative disease caused by a group of spongiform encephalopathies resulting from abnormal prion protein accumulation in the brain. These can be sporadic, genetic (caused by mutations in the prion-protein gene), or transmissible (acquired from an infected individual). Onset is insidious and there is a rapid progression of symptoms and impairment characterised by cognitive deficits, ataxia, and motor symptoms (myoclonus, chorea, or dystonia). Diagnosis is typically made on the basis of brain imaging studies, presence of characteristic proteins in spinal fluid, EEG, or genetic testing."^^xsd:string ;
    skos:prefLabel "Dementia prion disease"^^xsd:string .

icd-kg:Dementia_psychoactive_substances_including_medications a owl:Class ;
    rdfs:subClassOf icd-kg:Dementia ;
    skos:definition "Dementia due to psychoactive substances including medications includes forms of dementia that are judged to be a direct consequence of substance use and that persist beyond the usual duration of action or withdrawal syndrome associated with the substance. The amount and duration of substance use must be sufficient to produce the cognitive impairment. The cognitive impairment is not better accounted for by a disorder that is not induced by substances such as a dementia due to another medical condition."^^xsd:string ;
    skos:prefLabel "Dementia psychoactive substances including medications"^^xsd:string .

icd-kg:Dementia_rheumatological_diseases a owl:Class ;
    rdfs:subClassOf icd-kg:Dementia_diseases_classified_elsewhere ;
    skos:prefLabel "Dementia rheumatological diseases"^^xsd:string .

icd-kg:Dependent_personality a owl:Class ;
    rdfs:subClassOf icd-kg:Personality ;
    skos:definition "Personality disorder characterised by pervasive passive reliance on other people to make one's major and minor life decisions, great fear of abandonment, feelings of helplessness and incompetence, passive compliance with the wishes of elders and others, and a weak response to the demands of daily life. Lack of vigour may show itself in the intellectual or emotional spheres; there is often a tendency to transfer responsibility to others."^^xsd:string ;
    skos:prefLabel "Dependent personality"^^xsd:string .

icd-kg:Dissociative_amnesia a owl:Class ;
    icd-schema:exclusion <http://id.who.int/icd/entity/1397288146>,
        <http://id.who.int/icd/entity/1405777748>,
        <http://id.who.int/icd/entity/661071789>,
        <http://id.who.int/icd/entity/67207871> ;
    rdfs:subClassOf icd-kg:Dissociative ;
    skos:definition "Dissociative amnesia is characterised by an inability to recall important autobiographical memories, typically of recent traumatic or stressful events, that is inconsistent with ordinary forgetting. The amnesia does not occur exclusively during another dissociative disorder and is not better explained by another mental, behavioural or neurodevelopmental disorder. The amnesia is not due to the direct effects of a substance or medication on the central nervous system, including withdrawal effects, and is not due to a disease of the nervous system or to head trauma. The amnesia results in significant impairment in personal, family, social, educational, occupational or other important areas of functioning."^^xsd:string ;
    skos:prefLabel "Dissociative amnesia"^^xsd:string .

icd-kg:Dissociative_druginduced_mood_including_ketamine_or_pcp a owl:Class ;
    rdfs:subClassOf icd-kg:Certain_specified_dissociative_druginduced_mental_or_behavioural_including_ketamine_and_phencyclidine_%5Bpcp%5D,
        icd-kg:Substanceinduced_mood ;
    skos:definition "Dissociative drug-induced mood disorder including Ketamine or PCP is characterised by mood symptoms (e.g., depressed or elevated mood, decreased engagement in pleasurable activities, increased or decreased energy levels) that develop during or soon after intoxication with dissociative drugs. The intensity or duration of the symptoms is substantially in excess of mood disturbances that are characteristic of Dissociative drug intoxication. The amount and duration of Dissociative drug use must be capable of producing mood symptoms. The symptoms are not better explained by a primary mental disorder (e.g., a Depressive disorder, a Bipolar disorder, Schizoaffective disorder), as might be the case if the mood symptoms preceded the onset of the dissociative drug use, if the symptoms persist for a substantial period of time after cessation of the dissociative drug use, or if there is other evidence of a pre-existing primary mental disorder with mood symptoms (e.g., a history of prior episodes not associated with dissociative drug use)."^^xsd:string ;
    skos:prefLabel "Dissociative druginduced mood including ketamine or pcp"^^xsd:string .

icd-kg:Dissociative_neurological_symptom_with_paresis_or_weakness a owl:Class ;
    rdfs:subClassOf icd-kg:Dissociative_neurological_symptom ;
    skos:definition "Dissociative neurological symptom disorder, with paresis or weakness is characterised by a difficulty or inability to intentionally move parts of the body or to coordinate movements that is not consistent with a recognised disease of the nervous system, other mental, behavioural or neurodevelopmental disorder, or other medical condition and does not occur exclusively during another dissociative disorder."^^xsd:string ;
    skos:prefLabel "Dissociative neurological symptom with paresis or weakness"^^xsd:string .

icd-kg:Dissociative_neurological_symptom_with_visual_disturbance a owl:Class ;
    rdfs:subClassOf icd-kg:Dissociative_neurological_symptom ;
    skos:definition "Dissociative neurological symptom disorder, with visual disturbance is characterised by visual symptoms such as blindness, tunnel vision, diplopia, visual distortions or hallucinations that are not consistent with a recognised disease of the nervous system, other mental, behavioural or neurodevelopmental disorder, or other medical condition and do not occur exclusively during another dissociative disorder."^^xsd:string ;
    skos:prefLabel "Dissociative neurological symptom with visual disturbance"^^xsd:string .

icd-kg:Dysthymic a owl:Class ;
    icd-schema:inclusion "Dysthymia"^^xsd:string ;
    rdfs:subClassOf icd-kg:Depressive ;
    skos:definition "Dysthymic disorder is characterised by a persistent depressive mood (i.e., lasting 2 years or more), for most of the day, for more days than not. In children and adolescents depressed mood can manifest as pervasive irritability. The depressed mood is accompanied by additional symptoms such as markedly diminished interest or pleasure in activities, reduced concentration and attention or indecisiveness, low self-worth or excessive or inappropriate guilt, hopelessness about the future, disturbed sleep or increased sleep, diminished or increased appetite, or low energy or fatigue. During the first 2 years of the disorder, there has never been a 2-week period during which the number and duration of symptoms were sufficient to meet the diagnostic requirements for a Depressive Episode. There is no history of Manic, Mixed, or Hypomanic Episodes."^^xsd:string ;
    skos:prefLabel "Dysthymic"^^xsd:string .

icd-kg:Emotionally_unstable_personality a owl:Class ;
    rdfs:subClassOf icd-kg:Personality ;
    skos:prefLabel "Emotionally unstable personality"^^xsd:string .

icd-kg:Encopresis a owl:Class ;
    rdfs:subClassOf icd-kg:Elimination ;
    skos:definition "Encopresis is the repeated passage of faeces in inappropriate places. Encopresis should be diagnosed if inappropriate passage of faeces occurs repeatedly (e.g., at least once per month over a period of several months) in an individual who has reached the developmental age when faecal continence is ordinarily expected (4 years). The faecal incontinence may have been present from birth (i.e., an atypical extension of normal infantile incontinence), or may have arisen following a period of acquired bowel control. Encopresis should not be diagnosed if faecal soiling is fully attributable to another health condition (e.g., aganglionic megacolon, spina bifida, dementia), congenital or acquired abnormalities of the bowel, gastrointestinal infection, or excessive use of laxatives."^^xsd:string ;
    skos:prefLabel "Encopresis"^^xsd:string .

icd-kg:Enuresis a owl:Class ;
    icd-schema:exclusion <http://id.who.int/icd/entity/1140964489>,
        <http://id.who.int/icd/entity/1342466282>,
        <http://id.who.int/icd/entity/138852207>,
        <http://id.who.int/icd/entity/1471418842>,
        <http://id.who.int/icd/entity/429926918>,
        <http://id.who.int/icd/entity/444605491> ;
    icd-schema:inclusion "Functional enuresis"^^xsd:string,
        "Psychogenic enuresis"^^xsd:string,
        "Urinary incontinence of nonorganic origin"^^xsd:string ;
    rdfs:subClassOf icd-kg:Elimination ;
    skos:definition "Enuresis is the repeated voiding of urine into clothes or bed, which may occur during the day or at night, in an individual who has reached a developmental age when urinary continence is ordinarily expected (5 years). The urinary incontinence may have been present from birth (i.e., an atypical extension of normal infantile incontinence), or may have arisen following a period of acquired bladder control. In most cases, the behaviour is involuntary but in some cases it appears intentional. Enuresis should not be diagnosed if unintentional voiding of urine is due to a health condition that interferes with continence (e.g., diseases of the nervous system or musculoskeletal disorders) or by congenital or acquired abnormalities of the urinary tract."^^xsd:string ;
    skos:prefLabel "Enuresis"^^xsd:string .

icd-kg:Erectile_dysfunction_caused_by_endocrine a owl:Class ;
    rdfs:subClassOf icd-kg:Male_erectile_dysfunction ;
    skos:prefLabel "Erectile dysfunction caused by endocrine"^^xsd:string .

icd-kg:Factitious_imposed_on_another_person a owl:Class ;
    icd-schema:exclusion <http://id.who.int/icd/entity/1136473465> ;
    rdfs:subClassOf icd-kg:Factitious ;
    skos:definition "Factitious disorder imposed on another is characterised by feigning, falsifying, or inducing medical, psychological, or behavioural signs and symptoms or injury in another person, most commonly a child dependent, associated with identified deception. If a pre-existing disorder or disease is present in the other person, the individual intentionally aggravates existing symptoms or falsifies or induces additional symptoms. The individual seeks treatment for the other person or otherwise presents him or her as ill, injured, or impaired based on the feigned, falsified, or induced signs, symptoms, or injuries. The deceptive behaviour is not solely motivated by obvious external rewards or incentives (e.g., obtaining disability payments or avoiding criminal prosecution for child or elder abuse)."^^xsd:string ;
    skos:prefLabel "Factitious imposed on another person"^^xsd:string .

icd-kg:Female_sexual_arousal_dysfunction a owl:Class ;
    rdfs:subClassOf icd-kg:Sexual_arousal_dysfunctions ;
    skos:definition "Female sexual arousal dysfunction is characterised by absence or marked reduction in response to sexual stimulation in women, as manifested by any of the following: 1) Absence or marked reduction in genital response, including vulvovaginal lubrication, engorgement of the genitalia, and sensitivity of the genitalia; 2) Absence or marked reduction in non-genital responses such as hardening of the nipples, flushing of the skin, increased heart rate, increased blood pressure, and increased respiration rate; 3) Absence or marked reduction in feelings of sexual arousal (sexual excitement and sexual pleasure) from any type of sexual stimulation. The absence or marked reduction in response to sexual stimulation occurs despite the desire for sexual activity and adequate sexual stimulation, has occurred episodically or persistently over a period at least several months, and is associated with clinically significant distress."^^xsd:string ;
    skos:prefLabel "Female sexual arousal dysfunction"^^xsd:string .

icd-kg:Frontotemporal_dementia_genetic_mutation a owl:Class ;
    rdfs:subClassOf icd-kg:Frontotemporal_dementia ;
    skos:prefLabel "Frontotemporal dementia genetic mutation"^^xsd:string .

icd-kg:Frontotemporal_dementia_language_variant a owl:Class ;
    rdfs:subClassOf icd-kg:Frontotemporal_dementia ;
    skos:definition "A clinical syndrome primarily affecting language. It is characterised by an insidious onset and gradual progressive impairment of language that affects activities of daily living. Aphasia should be the most prominent deficit during the initial phases of the disease. As the clinical syndrome progresses, other cognitive functions may be involved as well, but language remains the most impaired domain throughout the disease."^^xsd:string ;
    skos:prefLabel "Frontotemporal dementia language variant"^^xsd:string .

icd-kg:Functional_movement a owl:Class ;
    rdfs:subClassOf icd-kg:Dissociative_neurological_symptom_with_movement_disturbance ;
    skos:definition "Movement disorder of a limb or body part in which there is positive evidence of either internal inconsistency or incongruity with other causes of movement disorder."^^xsd:string ;
    skos:prefLabel "Functional movement"^^xsd:string .

icd-kg:Gambling a owl:Class ;
    icd-schema:exclusion icd-kg:Bipolar_type_i,
        icd-kg:Bipolar_type_ii,
        <http://id.who.int/icd/entity/233747706> ;
    icd-schema:inclusion "Compulsive gambling"^^xsd:string ;
    rdfs:subClassOf icd-kg:Addictive_behaviours,
        icd-kg:Impulse_control ;
    skos:definition """Gambling disorder is characterised by a pattern of persistent or recurrent gambling behaviour, which may be online (i.e., over the internet) or offline, manifested by:

1. impaired control over gambling (e.g., onset, frequency, intensity, duration, termination, context);

2. increasing priority given to gambling to the extent that gambling takes precedence over other life interests and daily activities; and

3. continuation or escalation of gambling despite the occurrence of negative consequences.

The pattern of gambling behaviour may be continuous or episodic and recurrent. The pattern of gambling behaviour results in significant distress or in significant impairment in personal, family, social, educational, occupational or other important areas of functioning. The gambling behaviour and other features are normally evident over a period of at least 12 months in order for a diagnosis to be assigned, although the required duration may be shortened if all diagnostic requirements are met and symptoms are severe."""^^xsd:string ;
    skos:prefLabel "Gambling"^^xsd:string .

icd-kg:Gaming_predominantly_online a owl:Class ;
    rdfs:subClassOf icd-kg:Gaming ;
    skos:definition """!markdown
Gaming disorder, predominantly online is characterised by a pattern of persistent or recurrent gaming behaviour (‘digital gaming’ or ‘video-gaming’) that is primarily conducted over the internet and is manifested by: 

1. impaired control over gaming (e.g., onset, frequency, intensity, duration, termination, context); 
2. increasing priority given to gaming to the extent that gaming takes precedence over other life interests and daily activities; and 
3. continuation or escalation of gaming despite the occurrence of negative consequences. The behaviour pattern is of sufficient severity to result in significant impairment in personal, family, social, educational, occupational or other important areas of functioning. 

The pattern of gaming behaviour may be continuous or episodic and recurrent. The gaming behaviour and other features are normally evident over a period of at least 12 months in order for a diagnosis to be assigned, although the required duration may be shortened if all diagnostic requirements are met and symptoms are severe."""^^xsd:string ;
    skos:prefLabel "Gaming predominantly online"^^xsd:string .

icd-kg:Ganser_syndrome a owl:Class ;
    rdfs:subClassOf icd-kg:Dissociative ;
    skos:prefLabel "Ganser syndrome"^^xsd:string .

icd-kg:Hallucinogeninduced_mood a owl:Class ;
    rdfs:subClassOf icd-kg:Certain_specified_hallucinogeninduced_mental_or_behavioural,
        icd-kg:Substanceinduced_mood ;
    skos:definition "Hallucinogen-induced mood disorder is characterised by mood symptoms (e.g., depressed or elevated mood, decreased engagement in pleasurable activities, increased or decreased energy levels) that develop during or soon after intoxication with hallucinogens. The intensity or duration of the symptoms is substantially in excess of mood disturbances that are characteristic of hallucinogen intoxication. The amount and duration of hallucinogen use must be capable of producing mood symptoms. The symptoms are not better explained by a primary mental disorder (e.g., a Depressive disorder, a Bipolar disorder, Schizoaffective disorder), as might be the case if the mood symptoms preceded the onset of the hallucinogen use, if the symptoms persist for a substantial period of time after cessation of the hallucinogen use, or if there is other evidence of a pre-existing primary mental disorder with mood symptoms (e.g., a history of prior episodes not associated with hallucinogen use)."^^xsd:string ;
    skos:prefLabel "Hallucinogeninduced mood"^^xsd:string .

icd-kg:Harmful_pattern_of_alcohol_continuous a owl:Class ;
    icd-schema:exclusion icd-kg:Alcohol_dependence ;
    rdfs:subClassOf icd-kg:Harmful_pattern_of_alcohol ;
    skos:definition "A pattern of continuous (daily or almost daily) alcohol use that has caused damage to a person’s physical or mental health or has resulted in behaviour leading to harm to the health of others. The pattern of continuous alcohol use is evident over a period of at least one month. Harm to health of the individual occurs due to one or more of the following: (1) behaviour related to intoxication; (2) direct or secondary toxic effects on body organs and systems; or (3) a harmful route of administration. Harm to health of others includes any form of physical harm, including trauma, or mental disorder that is directly attributable to behaviour related to alcohol intoxication on the part of the person to whom the diagnosis of Harmful pattern of use of alcohol applies."^^xsd:string ;
    skos:prefLabel "Harmful pattern of alcohol continuous"^^xsd:string .

icd-kg:Harmful_pattern_of_nonpsychoactive_substances a owl:Class ;
    icd-schema:exclusion icd-kg:Harmful_pattern_of_other_specified_psychoactive_substance ;
    rdfs:subClassOf icd-kg:Nonpsychoactive_substances ;
    skos:definition "A pattern of use of non-psychoactive substances that has caused clinically significant harm to a person’s physical or mental health. The pattern of use is evident over a period of at least 12 months if use is episodic and at least one month if use is continuous (i.e., daily or almost daily). Harm may be caused by the direct or secondary toxic effects of the substance on body organs and systems, or a harmful route of administration."^^xsd:string ;
    skos:prefLabel "Harmful pattern of nonpsychoactive substances"^^xsd:string .

icd-kg:Hoarding a owl:Class ;
    rdfs:subClassOf icd-kg:Obsessivecompulsive_or_related ;
    skos:definition "Hoarding disorder is characterised by accumulation of possessions that results in living spaces becoming cluttered to the point that their use or safety is compromised. Accumulation occurs due to both repetitive urges or behaviours related to amassing items and difficulty discarding possessions due to a perceived need to save items and distress associated with discarding them. If living areas are uncluttered this is only due to the intervention of third parties (e.g., family members, cleaners, authorities). Amassment may be passive (e.g. accumulation of incoming flyers or mail) or active (e.g. excessive acquisition of free, purchased, or stolen items). The symptoms result in significant distress or significant impairment in personal, family, social, educational, occupational or other important areas of functioning."^^xsd:string ;
    skos:prefLabel "Hoarding"^^xsd:string .

icd-kg:Hypoactive_sexual_desire_dysfunction a owl:Class ;
    rdfs:subClassOf icd-kg:Sexual_dysfunctions ;
    skos:definition "Hypoactive Sexual Desire Dysfunction is characterised by absence or marked reduction in desire or motivation to engage in sexual activity as manifested by any of the following: 1) reduced or absent spontaneous desire (sexual thoughts or fantasies); 2) reduced or absent responsive desire to erotic cues and stimulation; or 3) inability to sustain desire or interest in sexual activity once initiated. The pattern of diminished or absent spontaneous or responsive desire or inability to sustain desire or interest in sexual activity has occurred episodically or persistently over a period at least several months, and is associated with clinically significant distress."^^xsd:string ;
    skos:prefLabel "Hypoactive sexual desire dysfunction"^^xsd:string .

icd-kg:Insomnia a owl:Class ;
    rdfs:subClassOf icd-kg:Sleepwake ;
    skos:definition "Insomnia disorders are characterised by the complaint of persistent difficulty with sleep initiation, duration, consolidation, or quality that occurs despite adequate opportunity and circumstances for sleep, and results in some form of daytime impairment. Daytime symptoms typically include fatigue, depressed mood or irritability, general malaise, and cognitive impairment. Individuals who report sleep related symptoms in the absence of daytime impairment are not regarded as having an insomnia disorder."^^xsd:string ;
    skos:prefLabel "Insomnia"^^xsd:string .

icd-kg:Intoxication_multiple_specified_psychoactive_substances a owl:Class ;
    rdfs:subClassOf icd-kg:Multiple_specified_psychoactive_substances_including_medications ;
    skos:definition "Intoxication due to multiple specified psychoactive substances is a clinically significant transient condition that develops during or shortly after the consumption of multiple specified substances or medications that is characterised by disturbances in consciousness, cognition, perception, affect, behaviour, or coordination. These disturbances are caused by the known pharmacological effects of the multiple specified psychoactive substances and their intensity is closely related to the amount of the substances consumed. They are time-limited and abate as the multiple specified substances are cleared from the body."^^xsd:string ;
    skos:prefLabel "Intoxication multiple specified psychoactive substances"^^xsd:string .

icd-kg:Language_with_impairment_of_mainly_expressive_language a owl:Class ;
    icd-schema:exclusion icd-kg:Language_with_impairment_of_receptive_and_expressive_language,
        <http://id.who.int/icd/entity/1167055901>,
        <http://id.who.int/icd/entity/1296093776>,
        <http://id.who.int/icd/entity/1705858040>,
        <http://id.who.int/icd/entity/348544271>,
        <http://id.who.int/icd/entity/947280473> ;
    icd-schema:inclusion "Developmental dysphasia or aphasia, expressive type"^^xsd:string ;
    rdfs:subClassOf icd-kg:Language ;
    skos:definition "Developmental language disorder with impairment of mainly expressive language is characterised by persistent difficulties in the acquisition, production, and use of language that arise during the developmental period, typically during early childhood, and cause significant limitations in the individual’s ability to communicate. The ability to produce and use spoken or signed language (i.e., expressive language) is markedly below the expected level given the individual’s age and level of intellectual functioning, but the ability to understand spoken or signed language (i.e., receptive language) is relatively intact."^^xsd:string ;
    skos:prefLabel "Language with impairment of mainly expressive language"^^xsd:string .

icd-kg:Learning_with_impairment_in_reading a owl:Class ;
    icd-schema:exclusion icd-kg:Of_intellectual_development ;
    rdfs:subClassOf icd-kg:Learning ;
    skos:definition "Developmental learning disorder with impairment in reading is characterised by significant and persistent difficulties in learning academic skills related to reading, such as word reading accuracy, reading fluency, and reading comprehension. The individual’s performance in reading is markedly below what would be expected for chronological age and level of intellectual functioning and results in significant impairment in the individual’s academic or occupational functioning. Developmental learning disorder with impairment in reading is not due to a disorder of intellectual development, sensory impairment (vision or hearing), neurological disorder, lack of availability of education, lack of proficiency in the language of academic instruction, or psychosocial adversity."^^xsd:string ;
    skos:prefLabel "Learning with impairment in reading"^^xsd:string .

icd-kg:Male_delayed_ejaculation a owl:Class ;
    rdfs:subClassOf icd-kg:Ejaculatory_dysfunctions ;
    skos:definition "Male delayed ejaculation is characterised by an inability to achieve ejaculation or an excessive or increased latency of ejaculation, despite adequate sexual stimulation and the desire to ejaculate. The pattern of delayed ejaculation has occurred episodically or persistently over a period at least several months, and is associated with clinically significant distress."^^xsd:string ;
    skos:prefLabel "Male delayed ejaculation"^^xsd:string .

icd-kg:Mdma_or_related_druginduced_mood_including_mda a owl:Class ;
    rdfs:subClassOf icd-kg:Certain_specified_mdma_or_related_druginduced_mental_or_behavioural_including_mda,
        icd-kg:Substanceinduced_mood ;
    skos:definition "MDMA or related drug-induced mood disorder, including MDA is characterised by mood symptoms (e.g., depressed or elevated mood, decreased engagement in pleasurable activities, increased or decreased energy levels) that develop during or soon after intoxication with MDMA or related drugs. The intensity or duration of the symptoms is substantially in excess of mood disturbances that are characteristic of MDMA or related drug intoxication, including MDA. The amount and duration of MDMA or related drug use must be capable of producing mood symptoms. The symptoms are not better explained by a primary mental disorder (e.g., a Depressive disorder, a Bipolar disorder, Schizoaffective disorder), as might be the case if the mood symptoms preceded the onset of the MDMA or related drug use, if the symptoms persist for a substantial period of time after cessation of the MDMA or related drug use, or if there is other evidence of a pre-existing primary mental disorder with mood symptoms (e.g., a history of prior episodes not associated with MDMA or related drug use)."^^xsd:string ;
    skos:prefLabel "Mdma or related druginduced mood including mda"^^xsd:string .

icd-kg:Mental_or_behavioural_associated_with_pregnancy_childbirth_or_the_puerperium_with_psychotic_symptoms a owl:Class ;
    rdfs:subClassOf icd-kg:Mental_or_behavioural_associated_with_pregnancy_childbirth_or_the_puerperium,
        icd-kg:Symptomatic_and_course_presentations_for_mood_episodes_in_mood ;
    skos:definition "A syndrome associated with pregnancy or the puerperium (commencing within about 6 weeks after delivery) that involves significant mental and behavioural features, including delusions, hallucinations, or other psychotic symptoms. Mood symptoms (depressive and/or manic) are also typically present. If the symptoms meet the diagnostic requirements for a specific mental disorder, that diagnosis should also be assigned."^^xsd:string ;
    skos:prefLabel "Mental or behavioural associated with pregnancy childbirth or the puerperium with psychotic symptoms"^^xsd:string .

icd-kg:Mental_or_behavioural_associated_with_pregnancy_childbirth_or_the_puerperium_without_psychotic_symptoms a owl:Class ;
    rdfs:subClassOf icd-kg:Mental_or_behavioural_associated_with_pregnancy_childbirth_or_the_puerperium,
        icd-kg:Symptomatic_and_course_presentations_for_mood_episodes_in_mood ;
    skos:definition "A syndrome associated with pregnancy or the puerperium (commencing within about 6 weeks after delivery) that involves significant mental and behavioural features, most commonly depressive symptoms. The syndrome does not include delusions, hallucinations, or other psychotic symptoms. If the symptoms meet the diagnostic requirements for a specific mental disorder, that diagnosis should also be assigned. This designation should not be used to describe mild and transient depressive symptoms that do not meet the diagnostic requirements for a depressive episode, which may occur soon after delivery (so-called postpartum blues)."^^xsd:string ;
    skos:prefLabel "Mental or behavioural associated with pregnancy childbirth or the puerperium without psychotic symptoms"^^xsd:string .

icd-kg:Mild_personality a owl:Class ;
    rdfs:subClassOf icd-kg:Personality ;
    skos:definition "All general diagnostic requirements for Personality Disorder are met. Disturbances affect some areas of personality functioning but not others (e.g., problems with self-direction in the absence of problems with stability and coherence of identity or self-worth), and may not be apparent in some contexts. There are problems in many interpersonal relationships and/or in performance of expected occupational and social roles, but some relationships are maintained and/or some roles carried out. Specific manifestations of personality disturbances are generally of mild severity. Mild Personality Disorder is typically not associated with substantial harm to self or others, but may be associated with substantial distress or with impairment in personal, family, social, educational, occupational or other important areas of functioning that is either limited to circumscribed areas (e.g., romantic relationships; employment) or present in more areas but milder."^^xsd:string ;
    skos:prefLabel "Mild personality"^^xsd:string .

icd-kg:Moderate_personality a owl:Class ;
    rdfs:subClassOf icd-kg:Personality ;
    skos:definition "All general diagnostic requirements for Personality Disorder are met. Disturbances affect multiple areas of personality functioning (e.g., identity or sense of self, ability to form intimate relationships, ability to control impulses and modulate behaviour). However, some areas of personality functioning may be relatively less affected. There are marked problems in most interpersonal relationships and the performance of most expected social and occupational roles is compromised to some degree. Relationships are likely to be characterised by conflict, avoidance, withdrawal, or extreme dependency (e.g., few friendships maintained, persistent conflict in work relationships and consequent occupational problems, romantic relationships characterised by serious disruption or inappropriate submissiveness). Specific manifestations of personality disturbance are generally of moderate severity. Moderate Personality Disorder is sometimes associated with harm to self or others, and is associated with marked impairment in personal, family, social, educational, occupational or other important areas of functioning, although functioning in circumscribed areas may be maintained."^^xsd:string ;
    skos:prefLabel "Moderate personality"^^xsd:string .

icd-kg:Mood_induced_by_multiple_specified_psychoactive_substances a owl:Class ;
    rdfs:subClassOf icd-kg:Certain_multiple_specified_psychoactive_substancesinduced_mental_or_behavioural ;
    skos:definition "Mood disorder induced by multiple specified psychoactive substances is characterised by mood symptoms (e.g., depressed or elevated mood, decreased engagement in pleasurable activities, increased or decreased energy levels) that develop during or soon after intoxication with or withdrawal from multiple specified psychoactive substances. The intensity or duration of the symptoms is substantially in excess of mood disturbances that are characteristic of intoxication with or withdrawal from multiple specified psychoactive substances. The amount and duration of use of the multiple specified psychoactive substances must be capable of producing mood symptoms. The symptoms are not better explained by a primary mental disorder (e.g., a Depressive disorder, a Bipolar disorder, Schizoaffective disorder), as might be the case if the mood symptoms preceded the onset of the use of the multiple specified psychoactive substances, if the symptoms persist for a substantial period of time after cessation of the use of the multiple specified psychoactive substances or withdrawal from the multiple specified psychoactive substances, or if there is other evidence of a pre-existing primary mental disorder with mood symptoms (e.g., a history of prior episodes not associated with the use of the multiple specified psychoactive substances)."^^xsd:string ;
    skos:prefLabel "Mood induced by multiple specified psychoactive substances"^^xsd:string .

icd-kg:Mood_induced_by_other_specified_psychoactive_substance a owl:Class ;
    rdfs:subClassOf icd-kg:Certain_other_specified_psychoactive_substanceinduced_mental_or_behavioural ;
    skos:definition "Mood disorder induced by other specified psychoactive substance is characterised by mood symptoms (e.g., depressed or elevated mood, decreased engagement in pleasurable activities, increased or decreased energy levels) that develop during or soon after intoxication with or withdrawal from a specified psychoactive substance. The intensity or duration of the symptoms is substantially in excess of mood disturbances that are characteristic of intoxication with or withdrawal from a specified psychoactive substance. The amount and duration of use of the specified psychoactive substance must be capable of producing mood symptoms. The symptoms are not better explained by a primary mental disorder (e.g., a Depressive disorder, a Bipolar disorder, Schizoaffective disorder), as might be the case if the mood symptoms preceded the onset of the use of the specified psychoactive substance, if the symptoms persist for a substantial period of time after cessation of the use of the specified psychoactive substance or withdrawal from the specified psychoactive substance, or if there is other evidence of a pre-existing primary mental disorder with mood symptoms (e.g., a history of prior episodes not associated with the use of the specified psychoactive substance)."^^xsd:string ;
    skos:prefLabel "Mood induced by other specified psychoactive substance"^^xsd:string .

icd-kg:Mood_induced_by_unknown_or_unspecified_psychoactive_substance a owl:Class ;
    rdfs:subClassOf icd-kg:Certain_unknown_or_unspecified_psychoactive_substanceinduced_mental_or_behavioural ;
    skos:definition "Mood disorder induced by unknown or unspecified psychoactive substance is characterised by mood symptoms (e.g., depressed or elevated mood, decreased engagement in pleasurable activities, increased or decreased energy levels) that develop during or soon after intoxication with or withdrawal from a specified psychoactive substance. The symptoms are not better explained by a primary mental disorder (e.g., a Depressive disorder, a Bipolar disorder, Schizoaffective disorder), as might be the case if the mood symptoms preceded the onset of the use of the unknown or unspecified psychoactive substance, if the symptoms persist for a substantial period of time after cessation of the use of the unknown or unspecified psychoactive substance or withdrawal from the unknown or unspecified psychoactive substance, or if there is other evidence of a pre-existing primary mental disorder with mood symptoms (e.g., a history of prior episodes not associated with the use of the unknown or unspecified psychoactive substance)."^^xsd:string ;
    skos:prefLabel "Mood induced by unknown or unspecified psychoactive substance"^^xsd:string .

icd-kg:Multiple_specified_psychoactive_substances_withdrawal a owl:Class ;
    rdfs:subClassOf icd-kg:Multiple_specified_psychoactive_substances_including_medications ;
    skos:definition "Multiple specified psychoactive substance withdrawal is a clinically significant cluster of symptoms, behaviours and physiological features, varying in degree of severity and duration, that occurs upon cessation or reduction of use of multiple specified substances in individuals who have developed dependence or have used the specified substances for a prolonged period or in large amounts. Multiple specified psychoactive substance withdrawal can also occur when prescribed psychoactive medications have been used in standard therapeutic doses. The specific features of the withdrawal state depend on the pharmacological properties of the specified substances and their interactions."^^xsd:string ;
    skos:prefLabel "Multiple specified psychoactive substances withdrawal"^^xsd:string .

icd-kg:Nailbiting a owl:Class ;
    rdfs:subClassOf icd-kg:Repetitive_selfbiting_behaviour ;
    skos:definition "Nail-biting is a common obsessive-compulsive disorder characterised by compulsive biting or chewing the nails and nailfolds."^^xsd:string ;
    skos:prefLabel "Nailbiting"^^xsd:string .

icd-kg:Narcolepsy a owl:Class ;
    rdfs:subClassOf icd-kg:Hypersomnolence ;
    skos:definition "Narcolepsy is a disorder characterised by daily periods of irrepressible need to sleep or daytime lapses into sleep occurring for at least several months, accompanied by abnormal manifestations of REM sleep. Multiple sleep latency testing (MSLT) demonstrates a mean sleep latency of <8 minutes and two or more sleep-onset REM periods (SOREMP’s), or one or more SOREMP’s on MSLT and a SOREMP on the preceding overnight polysomnography (PSG). Nighttime sleep is often disturbed, and brief daytime naps are typically refreshing."^^xsd:string ;
    skos:prefLabel "Narcolepsy"^^xsd:string .

icd-kg:Neurogenic_cluttering a owl:Class ;
    rdfs:subClassOf icd-kg:Speech_fluency ;
    skos:prefLabel "Neurogenic cluttering"^^xsd:string .

icd-kg:Neurogenic_mixed_stuttering_and_cluttering a owl:Class ;
    rdfs:subClassOf icd-kg:Speech_fluency ;
    skos:prefLabel "Neurogenic mixed stuttering and cluttering"^^xsd:string .

icd-kg:Neurogenic_stuttering a owl:Class ;
    rdfs:subClassOf icd-kg:Speech_fluency ;
    skos:prefLabel "Neurogenic stuttering"^^xsd:string .

icd-kg:Nonamnestic_alzheimer_disease_dementia_logopenic_variant a owl:Class ;
    rdfs:subClassOf icd-kg:Nonamnestic_alzheimer_disease_dementia_subtypes ;
    skos:definition "Clinical variant of Alzheimer disease dementia presenting with predominant language problems, characterised by impairment of single-word retrieval in spontaneous speech and naming, and impaired repetition of sentences. Phonologic errors are usually present, with preservation of single-word comprehension and object knowledge. Episodic memory is proportionally less impaired. Neuroimaging abnormalities are observed, namely left posterior perisylvian or parietal atrophy on magnetic resonance, in association with hypoperfusion or hypometabolism in these same areas on SPECT or FDG-PET, respectively."^^xsd:string ;
    skos:prefLabel "Nonamnestic alzheimer disease dementia logopenic variant"^^xsd:string .

icd-kg:Nonamnestic_alzheimer_disease_dementia_visuospatial_variant a owl:Class ;
    rdfs:subClassOf icd-kg:Nonamnestic_alzheimer_disease_dementia_subtypes ;
    skos:definition "Clinical variant of Alzheimer disease dementia presenting with predominant visual perception and/or visuospatial deficits with intact primary visual function. Clinical features include elements of Balint’s syndrome (optic ataxia, ocular apraxia and simultagnosia) associated or not with Gerstmann’s syndrome (acalculia, agraphia, left–right disorientation and finger agnosia) Episodic memory is proportionally less impaired. There is prominent atrophy in the posterior cortical regions on magnetic resonance and hypometabolism on FDG-PET examination."^^xsd:string ;
    skos:prefLabel "Nonamnestic alzheimer disease dementia visuospatial variant"^^xsd:string .

icd-kg:Obesity_hypoventilation_syndrome a owl:Class ;
    icd-schema:inclusion "Pickwickian syndrome"^^xsd:string ;
    rdfs:subClassOf icd-kg:Sleeprelated_hypoventilation_or_hypoxemia ;
    skos:definition """Obesity hypoventilation syndrome is characterised by obesity (in adults, Body-Mass-Index > 30 kg/m²) and daytime hypercapnia indicated by arterial partial pressure of carbon dioxide (PaCO2) > 45 mm Hg that cannot be fully attributed to an underlying cardiopulmonary or neurologic disease. Hypercapnia worsens during sleep and is often associated with severe arterial oxygen desaturation. Obstructive sleep apnoea is also present in the majority of cases and should be diagnosed in addition to obesity hypoventilation.

Note: A definitive diagnosis requires demonstration of daytime hypercapnia and objective evidence based on polysomnography, with carbon dioxide (CO2) monitoring (by arterial, end-tidal or transcutaneous measures)."""^^xsd:string ;
    skos:prefLabel "Obesity hypoventilation syndrome"^^xsd:string .

icd-kg:Obsessivecompulsive a owl:Class ;
    icd-schema:exclusion <http://id.who.int/icd/entity/1682814866> ;
    icd-schema:inclusion "anankastic neurosis"^^xsd:string,
        "obsessive-compulsive neurosis"^^xsd:string ;
    rdfs:subClassOf icd-kg:Obsessivecompulsive_or_related ;
    skos:definition "Obsessive-Compulsive Disorder is characterised by the presence of persistent obsessions or compulsions, or most commonly both. Obsessions are repetitive and persistent thoughts, images, or impulses/urges that are intrusive, unwanted, and are commonly associated with anxiety. The individual attempts to ignore or suppress obsessions or to neutralize them by performing compulsions. Compulsions are repetitive behaviours including repetitive mental acts that the individual feels driven to perform in response to an obsession, according to rigid rules, or to achieve a sense of ‘completeness’. In order for obsessive-compulsive disorder to be diagnosed, obsessions and compulsions must be time consuming (e.g. taking more than an hour per day) or result in significant distress or significant impairment in personal, family, social, educational, occupational or other important areas of functioning."^^xsd:string ;
    skos:prefLabel "Obsessivecompulsive"^^xsd:string .

icd-kg:Obstructive_sleep_apnoea a owl:Class ;
    icd-schema:exclusion <http://id.who.int/icd/entity/1421696615> ;
    rdfs:subClassOf icd-kg:Sleeprelated_breathing ;
    skos:definition """Obstructive sleep apnoea is characterised by repetitive episodes of apnoea or hypopnea that are caused by upper airway obstruction occurring during sleep. These events often result in reductions in blood oxygen saturation and are usually terminated by brief arousals from sleep. Excessive sleepiness is a major presenting complaint in many but not all cases. Reports of insomnia, poor sleep quality, and fatigue are also common. Upper airway resistance syndrome shares the same pathophysiology and should be classified here. In adults (> 18 years), obstructive sleep apnoea is diagnosed when the frequency of obstructive events (apnoeas, hypopneas or respiratory-event related arousals) is greater than 15 per hour. The disorder may also be diagnosed when the frequency is greater than five per hour and: a) symptoms attributable to the disorder (e.g., sleepiness or sleep disruption) are present; or b) nocturnal respiratory distress or observed apnoea/habitual snoring are reported; or c) when hypertension, a mood disorder, cognitive dysfunction, coronary artery disease, stroke, congestive heart failure, atrial fibrillation, or type 2 diabetes mellitus are present. In children, the disorder is diagnosed when the frequency of obstructive events is greater than one per hour, accompanied by signs or symptoms related to the breathing disorder.

Note: A definitive diagnosis requires objective evidence based on polysomnography."""^^xsd:string ;
    skos:prefLabel "Obstructive sleep apnoea"^^xsd:string .

icd-kg:Of_arousal_from_nonrem_sleep a owl:Class ;
    rdfs:subClassOf icd-kg:Parasomnia ;
    skos:definition "Disorders of arousal from non-REM sleep are characterised by experiences or behaviours such as confusion, ambulation, terror, or extreme autonomic arousal that typically arise as a result of incomplete arousals from deep non-REM (N3) sleep. An exception is sleep-related eating disorder, which has been observed to arise during all stages of non-REM sleep. This group of disorders is also characterised by partial or complete amnesia for the event, inappropriate or absent responsiveness to efforts by others to intervene or redirect the person during the episode, and limited (e.g., a single visual scene) or no associated cognition or dream imagery. The experiences or behaviours are sufficiently severe to result in significant distress or significant impairment in personal, family, social, educational, occupational or other important areas of functioning or significant risk of injury to the individual or to others (e.g., thrashing or striking out in response to efforts to restrain the individual)."^^xsd:string ;
    skos:prefLabel "Of arousal from nonrem sleep"^^xsd:string .

icd-kg:Olfactory_reference a owl:Class ;
    rdfs:subClassOf icd-kg:Obsessivecompulsive_or_related ;
    skos:definition "Olfactory Reference Disorder is characterised by persistent preoccupation with the belief that one is emitting a perceived foul or offensive body odour or breath that is either unnoticeable or only slightly noticeable to others. Individuals experience excessive self-consciousness about the perceived odour, often with ideas of reference (i.e., the conviction that people are taking notice, judging, or talking about the odour). In response to their preoccupation, individuals engage in repetitive and excessive behaviours such as repeatedly checking for body odour or checking the perceived source of the smell, or repeatedly seeking reassurance, excessive attempts to camouflage, alter, or prevent the perceived odour, or marked avoidance of social situations or triggers that increase distress about the perceived foul or offensive odour. The symptoms are sufficiently severe to result in significant distress or significant impairment in personal, family, social, educational, occupational or other important areas of functioning."^^xsd:string ;
    skos:prefLabel "Olfactory reference"^^xsd:string .

icd-kg:Opioid_withdrawal a owl:Class ;
    rdfs:subClassOf icd-kg:Opioids ;
    skos:definition "Opioid withdrawal is a clinically significant cluster of symptoms, behaviours and/or physiological features, varying in degree of severity and duration, that occurs upon cessation or reduction of use of opioids in individuals who have developed Opioid dependence or have used opioids for a prolonged period or in large amounts. Opioid withdrawal can also occur when prescribed opioids have been used in standard therapeutic doses. Presenting features of Opioid withdrawal may include dysphoric mood, craving for an opioid, anxiety, nausea or vomiting, abdominal cramps, muscle aches, yawning, perspiration, hot and cold flushes, lacrimation, rhinorrhea, hypersomnia (typically in the initial phase) or insomnia, diarrhea, piloerection, and pupillary dilatation."^^xsd:string ;
    skos:prefLabel "Opioid withdrawal"^^xsd:string .

icd-kg:Opioidinduced_delirium a owl:Class ;
    icd-schema:inclusion "Delirium induced by opioid withdrawal"^^xsd:string ;
    rdfs:subClassOf icd-kg:Delirium_psychoactive_substances_including_medications,
        icd-kg:Opioids ;
    skos:definition "Opioid-induced delirium is characterised by an acute state of disturbed attention and awareness with specific features of delirium that develops during or soon after substance intoxication or withdrawal or during the use of opioids. The amount and duration of opioid use must be capable of producing delirium. The symptoms are not better explained by a primary mental disorder, by use of or withdrawal from a different substance, or by another health condition that is not classified under Mental, Behavioural, and Neurodevelopmental Disorders."^^xsd:string ;
    skos:prefLabel "Opioidinduced delirium"^^xsd:string .

icd-kg:Opioidinduced_mood a owl:Class ;
    rdfs:subClassOf icd-kg:Certain_specified_opioidinduced_mental_or_behavioural,
        icd-kg:Substanceinduced_mood ;
    skos:definition "Opioid-induced mood disorder is characterised by mood symptoms (e.g., depressed or elevated mood, decreased engagement in pleasurable activities, increased or decreased energy levels) that develop during or soon after intoxication with or withdrawal from opioids. The intensity or duration of the symptoms is substantially in excess of mood disturbances that are characteristic of Opioid intoxication or Opioid withdrawal. The amount and duration of opioid use must be capable of producing mood symptoms. The symptoms are not better explained by a primary mental disorder (e.g., a Depressive disorder, a Bipolar disorder, Schizoaffective disorder), as might be the case if the mood symptoms preceded the onset of the opioid use, if the symptoms persist for a substantial period of time after cessation of the opioid use or withdrawal, or if there is other evidence of a pre-existing primary mental disorder with mood symptoms (e.g., a history of prior episodes not associated with opioid use)."^^xsd:string ;
    skos:prefLabel "Opioidinduced mood"^^xsd:string .

icd-kg:Oppositional_defiant_with_chronic_irritabilityanger a owl:Class ;
    rdfs:subClassOf icd-kg:Oppositional_defiant ;
    skos:definition "All definitional requirements for oppositional defiant disorder are met. This form of oppositional defiant disorder is characterised by prevailing, persistent angry or irritable mood that may be present independent of any apparent provocation. The negative mood is often accompanied by regularly occurring severe temper outbursts that are grossly out of proportion in intensity or duration to the provocation. Chronic irritability and anger are characteristic of the individual’s functioning nearly every day, are observable across multiple settings or domains of functioning (e.g., home, school, social relationships), and are not restricted to the individual’s relationship with his/her parents or guardians. The pattern of chronic irritability and anger is not limited to occasional episodes (e.g., developmentally typical irritability) or discrete periods (e.g., irritable mood in the context of manic or depressive episodes)."^^xsd:string ;
    skos:prefLabel "Oppositional defiant with chronic irritabilityanger"^^xsd:string .

icd-kg:Oppositional_defiant_without_chronic_irritabilityanger a owl:Class ;
    rdfs:subClassOf icd-kg:Oppositional_defiant ;
    skos:definition "Meets all definitional requirements for oppositional defiant disorder. This form of oppositional defiant disorder is not characterised by prevailing, persistent, angry or irritable mood, but does feature headstrong, argumentative, and defiant behaviour."^^xsd:string ;
    skos:prefLabel "Oppositional defiant without chronic irritabilityanger"^^xsd:string .

icd-kg:Orofacial_motor_coordination a owl:Class ;
    rdfs:subClassOf icd-kg:Motor_coordination ;
    skos:prefLabel "Orofacial motor coordination"^^xsd:string .

icd-kg:Other_parasomnias a owl:Class ;
    rdfs:subClassOf icd-kg:Parasomnia ;
    skos:definition "Other parasomnias include Hypnogogic exploding head syndrome, Sleep-related hallucinations, and abnormal sleep related complex movements, behaviours, emotions, perceptions, dreams, or autonomic nervous system activity related to a medical condition or due to a medication or substance. The experiences are sufficiently severe to result in significant distress or significant impairment in personal, family, social, educational, occupational or other important areas of functioning or significant risk of injury to the individual or to others."^^xsd:string ;
    skos:prefLabel "Other parasomnias"^^xsd:string .

icd-kg:Other_specified_psychoactive_substance_withdrawal a owl:Class ;
    rdfs:subClassOf icd-kg:Other_specified_psychoactive_substances_including_medications ;
    skos:definition "Other specified psychoactive substance withdrawal is a clinically significant cluster of symptoms, behaviours and/or physiological features, varying in degree of severity and duration, that occurs upon cessation or reduction of use of the specified substance in individuals who have developed dependence or have used the specified substance for a prolonged period or in large amounts. Other specified psychoactive substance withdrawal can also occur when prescribed psychoactive medications have been used in standard therapeutic doses. The specific features of the withdrawal state depend on the pharmacological properties of the specified substance."^^xsd:string ;
    skos:prefLabel "Other specified psychoactive substance withdrawal"^^xsd:string .

icd-kg:Parasomnias_related_to_rem_sleep a owl:Class ;
    rdfs:subClassOf icd-kg:Parasomnia ;
    skos:definition "Parasomnias related to REM (rapid eye movement) sleep are characterised by experiences or behaviours such as vocalization or complex motor behaviours, sleep paralysis, or nightmares that are associated with REM sleep. The experiences are sufficiently severe to result in significant distress or significant impairment in personal, family, social, educational, occupational or other important areas of functioning or significant risk of injury to the individual or to others."^^xsd:string ;
    skos:prefLabel "Parasomnias related to rem sleep"^^xsd:string .

icd-kg:Pica a owl:Class ;
    rdfs:subClassOf icd-kg:Feeding_or_eating ;
    skos:definition "Pica is characterised by the regular consumption of non-nutritive substances, such as non-food objects and materials (e.g., clay, soil, chalk, plaster, plastic, metal and paper) or raw food ingredients (e.g., large quantities of salt or corn flour) that is persistent or severe enough to require clinical attention in an individual who has reached a developmental age at which they would be expected to distinguish between edible and non-edible substances (approximately 2 years). That is, the behaviour causes damage to health, impairment in functioning, or significant risk due to the frequency, amount or nature of the substances or objects ingested."^^xsd:string ;
    skos:prefLabel "Pica"^^xsd:string .

icd-kg:Postconcussional_syndrome a owl:Class ;
    rdfs:subClassOf icd-kg:Mild_neurocognitive ;
    skos:definition "A syndrome that occurs following head trauma (usually sufficiently severe to result in loss of consciousness) and includes a number of disparate symptoms such as headache, dizziness, fatigue, irritability, difficulty in concentration and performing mental tasks, impairment of memory, insomnia, and reduced tolerance to stress, emotional excitement, or alcohol."^^xsd:string ;
    skos:prefLabel "Postconcussional syndrome"^^xsd:string .

icd-kg:Prominent_personality_traits_or_patterns a owl:Class ;
    rdfs:subClassOf icd-kg:Personality_and_related_traits ;
    skos:definition "Trait domain qualifiers may be applied to Personality Disorders or Personality Difficulty to describe the characteristics of the individual’s personality that are most prominent and that contribute to personality disturbance. Trait domains are continuous with normal personality characteristics in individuals who do not have Personality Disorder or Personality Difficulty. Trait domains are not diagnostic categories, but rather represent a set of dimensions that correspond to the underlying structure of personality. As many trait domain qualifiers may be applied as necessary to describe personality functioning. Individuals with more severe personality disturbance tend to have a greater number of prominent trait domains."^^xsd:string ;
    skos:prefLabel "Prominent personality traits or patterns"^^xsd:string .

icd-kg:Propriospinal_myoclonus_at_sleep_onset a owl:Class ;
    rdfs:subClassOf icd-kg:Sleeprelated_movement ;
    skos:definition "Propriospinal myoclonus at sleep onset consists of sudden myoclonic jerks of the trunk, hips, and knees in a fixed pattern that occur during the transition from wakefulness to sleep and, more rarely, during nighttime awakenings or upon awakening in the morning. The jerks arise mainly in spinally innervated muscles and thereafter propagate to rostral and caudal muscles at a low speed, typical of propriospinal pathways. The movements result in clinically significant difficulty with sleep initiation or maintenance."^^xsd:string ;
    skos:prefLabel "Propriospinal myoclonus at sleep onset"^^xsd:string .

icd-kg:Recurrent_depressive_current_episode_mild a owl:Class ;
    rdfs:subClassOf icd-kg:Recurrent_depressive ;
    skos:definition "Recurrent depressive disorder, current episode mild is diagnosed when the definitional requirements for Recurrent depressive disorder have been met and there is currently a depressive episode of mild severity. A depressive episode is characterised by a period of depressed mood or diminished interest in activities occurring most of the day, nearly every day during a period lasting at least two weeks accompanied by other symptoms such as difficulty concentrating, feelings of worthlessness or excessive or inappropriate guilt, hopelessness, recurrent thoughts of death or suicide, changes in appetite or sleep, psychomotor agitation or retardation, and reduced energy or fatigue. In a mild depressive episode, the individual is usually distressed by the symptoms and has some difficulty in continuing to function in one or more domains (personal, family, social, educational, occupational, or other important domains). There are no delusions or hallucinations during the episode."^^xsd:string ;
    skos:prefLabel "Recurrent depressive current episode mild"^^xsd:string .

icd-kg:Recurrent_depressive_current_episode_moderate_with_psychotic_symptoms a owl:Class ;
    rdfs:subClassOf icd-kg:Recurrent_depressive ;
    skos:definition "Recurrent depressive disorder, current episode moderate, with psychotic symptoms is diagnosed when the definitional requirements for Recurrent depressive disorder have been met and there is currently a depressive episode of moderate severity, and there are delusions or hallucinations during the episode. A depressive episode is characterised by a period of depressed mood or diminished interest in activities occurring most of the day, nearly every day during a period lasting at least two weeks accompanied by other symptoms such as difficulty concentrating, feelings of worthlessness or excessive or inappropriate guilt, hopelessness, recurrent thoughts of death or suicide, changes in appetite or sleep, psychomotor agitation or retardation, and reduced energy or fatigue. In a moderate depressive episode, several symptoms of a depressive episode are present to a marked degree, or a large number of depressive symptoms of lesser severity are present overall. The individual typically has considerable difficulty functioning in multiple domains (personal, family, social, educational, occupational, or other important domains)."^^xsd:string ;
    skos:prefLabel "Recurrent depressive current episode moderate with psychotic symptoms"^^xsd:string .

icd-kg:Recurrent_depressive_current_episode_moderate_without_psychotic_symptoms a owl:Class ;
    rdfs:subClassOf icd-kg:Recurrent_depressive ;
    skos:definition "Recurrent depressive disorder, current episode moderate, without psychotic symptoms is diagnosed when the definitional requirements for recurrent depressive disorder have been met and there is currently a depressive episode of moderate severity, and there are no delusions or hallucinations during the episode. A depressive episode is characterised by a period of depressed mood or diminished interest in activities occurring most of the day, nearly every day during a period lasting at least two weeks accompanied by other symptoms such as difficulty concentrating, feelings of worthlessness or excessive or inappropriate guilt, hopelessness, recurrent thoughts of death or suicide, changes in appetite or sleep, psychomotor agitation or retardation, and reduced energy or fatigue. In a moderate depressive episode, several symptoms of a depressive episode are present to a marked degree, or a large number of depressive symptoms of lesser severity are present overall. The individual typically has considerable difficulty functioning in multiple domains (personal, family, social, educational, occupational, or other important domains)."^^xsd:string ;
    skos:prefLabel "Recurrent depressive current episode moderate without psychotic symptoms"^^xsd:string .

icd-kg:Recurrent_depressive_current_episode_severe_with_psychotic_symptoms a owl:Class ;
    icd-schema:inclusion "Endogenous depression with psychotic symptoms"^^xsd:string,
        "Manic-depressive psychosis, depressed type with psychotic symptoms"^^xsd:string ;
    rdfs:subClassOf icd-kg:Recurrent_depressive ;
    skos:definition "Recurrent depressive disorder, current episode severe, with psychotic symptoms is diagnosed when the definitional requirements for Recurrent depressive disorder are met and the current episode is severe and there are delusions or hallucinations during the episode. A depressive episode is characterised by a period of depressed mood or diminished interest in activities occurring most of the day, nearly every day during a period lasting at least two weeks accompanied by other symptoms such as difficulty concentrating, feelings of worthlessness or excessive or inappropriate guilt, hopelessness, recurrent thoughts of death or suicide, changes in appetite or sleep, psychomotor agitation or retardation, and reduced energy or fatigue. In a severe depressive episode, many or most symptoms of a Depressive Episode are present to a marked degree, or a smaller number of symptoms are present and manifest to an intense degree. The individual has serious difficulty continuing to function in most domains (personal, family, social, educational, occupational, or other important domains). In a severe depressive episode, many or most symptoms of a Depressive Episode are present to a marked degree, or a smaller number of symptoms are present and manifest to an intense degree. The individual has serious difficulty continuing to function in most domains (personal, family, social, educational, occupational, or other important domains)."^^xsd:string ;
    skos:prefLabel "Recurrent depressive current episode severe with psychotic symptoms"^^xsd:string .

icd-kg:Recurrent_depressive_current_episode_severe_without_psychotic_symptoms a owl:Class ;
    icd-schema:inclusion "Endogenous depression without psychotic symptoms"^^xsd:string,
        "Major depression, recurrent without psychotic symptoms"^^xsd:string,
        "Manic-depressive psychosis, depressed type without psychotic symptoms"^^xsd:string,
        "Vital depression, recurrent without psychotic symptoms"^^xsd:string ;
    rdfs:subClassOf icd-kg:Recurrent_depressive ;
    skos:definition "Recurrent depressive disorder, current episode severe, without psychotic symptoms is diagnosed when the definitional requirements for Recurrent depressive disorder are met and the current episode is severe and there are no delusions or hallucinations during the episode. A depressive episode is characterised by a period of depressed mood or diminished interest in activities occurring most of the day, nearly every day during a period lasting at least two weeks accompanied by other symptoms such as difficulty concentrating, feelings of worthlessness or excessive or inappropriate guilt, hopelessness, recurrent thoughts of death or suicide, changes in appetite or sleep, psychomotor agitation or retardation, and reduced energy or fatigue. In a severe depressive episode, many or most symptoms of a Depressive Episode are present to a marked degree, or a smaller number of symptoms are present and manifest to an intense degree. The individual has serious difficulty continuing to function in most domains (personal, family, social, educational, occupational, or other important domains)."^^xsd:string ;
    skos:prefLabel "Recurrent depressive current episode severe without psychotic symptoms"^^xsd:string .

icd-kg:Ruminationregurgitation a owl:Class ;
    icd-schema:exclusion <http://id.who.int/icd/entity/55732315>,
        <http://id.who.int/icd/entity/677319549> ;
    rdfs:subClassOf icd-kg:Feeding_or_eating ;
    skos:definition "Rumination-regurgitation disorder is characterised by the intentional and repeated bringing up of previously swallowed food back to the mouth (i.e., regurgitation), which may be re-chewed and re-swallowed (i.e. rumination), or may be deliberately spat out (but not as in vomiting). The regurgitation behaviour is frequent (at least several times per week) and sustained over a period of at least several weeks. The regurgitation behaviour is not fully accounted for by another medical condition that directly causes regurgitation (e.g., oesophageal strictures or neuromuscular disorders affecting oesophageal functioning) or causes nausea or vomiting (e.g. pyloric stenosis). Rumination-regurgitation disorder should only be diagnosed in individuals who have reached a developmental age of at least 2 years."^^xsd:string ;
    skos:prefLabel "Ruminationregurgitation"^^xsd:string .

icd-kg:Schizoaffective_continuous a owl:Class ;
    rdfs:subClassOf icd-kg:Schizoaffective ;
    skos:definition "Symptoms fulfilling all definitional requirements of Schizoaffective disorder have been present for almost all of the illness course over a period of at least one year, with periods of subthreshold symptoms being very brief relative to the overall course."^^xsd:string ;
    skos:prefLabel "Schizoaffective continuous"^^xsd:string .

icd-kg:Schizoaffective_first_episode a owl:Class ;
    rdfs:subClassOf icd-kg:Schizoaffective ;
    skos:definition "Schizoaffective disorder, first episode should be used to identify individuals experiencing symptoms that meet the diagnostic requirements for Schizoaffective disorder (including duration) but who have never before experienced an episode during which diagnostic requirements for Schizoaffective disorder or Schizophrenia were met."^^xsd:string ;
    skos:prefLabel "Schizoaffective first episode"^^xsd:string .

icd-kg:Schizoaffective_multiple_episodes a owl:Class ;
    rdfs:subClassOf icd-kg:Schizoaffective ;
    skos:definition "Schizoaffective disorder, multiple episodes should be used to identify individuals experiencing symptoms that meet the diagnostic requirements for Schizoaffective disorder and who have also previously experienced episodes during which diagnostic requirements for Schizoaffective disorder or Schizophrenia were met, with substantial remission of symptoms between episodes. Some attenuated symptoms may remain during period of remission, and remissions may have occurred in response to medication or other treatment."^^xsd:string ;
    skos:prefLabel "Schizoaffective multiple episodes"^^xsd:string .

icd-kg:Schizophrenia_continuous a owl:Class ;
    rdfs:subClassOf icd-kg:Schizophrenia ;
    skos:definition "Symptoms fulfilling all definitional requirements of Schizophrenia have been present for almost all of the illness course over a period of at least one year, with periods of subthreshold symptoms being very brief relative to the overall course."^^xsd:string ;
    skos:prefLabel "Schizophrenia continuous"^^xsd:string .

icd-kg:Schizophrenia_first_episode a owl:Class ;
    rdfs:subClassOf icd-kg:Schizophrenia ;
    skos:definition "Schizophrenia, first episode should be used to identify individuals experiencing symptoms that meet the diagnostic requirements for Schizophrenia (including duration) but who have never before experienced an episode during which diagnostic requirements for Schizophrenia were met."^^xsd:string ;
    skos:prefLabel "Schizophrenia first episode"^^xsd:string .

icd-kg:Schizophrenia_multiple_episodes a owl:Class ;
    rdfs:subClassOf icd-kg:Schizophrenia ;
    skos:definition "Schizophrenia, multiple episodes should be used to identify individuals experiencing symptoms that meet the diagnostic requirements for Schizophrenia and who have also previously experienced episodes during which diagnostic requirements were met, with substantial remission of symptoms between episodes. Some attenuated symptoms may remain during periods of remission, and remissions may have occurred in response to medication or other treatment."^^xsd:string ;
    skos:prefLabel "Schizophrenia multiple episodes"^^xsd:string .

icd-kg:Secondary_mood_syndrome a owl:Class ;
    icd-schema:exclusion icd-kg:Adjustment,
        icd-kg:Delirium ;
    rdfs:subClassOf icd-kg:Mood,
        icd-kg:Secondary_mental_or_behavioural_syndromes_associated_with_or_diseases_classified_elsewhere ;
    skos:definition "A syndrome characterised by the presence of prominent mood symptoms (i.e., depression, elevated mood, irritability) judged to be a direct pathophysiological consequence of a health condition not classified under mental and behavioural disorders, based on evidence from the history, physical examination, or laboratory findings. The symptoms are not accounted for by delirium or by another mental and behavioural disorder, and are not a psychologically mediated response to a severe medical condition (e.g., depressive symptoms in response to a life-threatening diagnosis). This category should be used in addition to the diagnosis for the presumed underlying disorder or disease when the mood symptoms are sufficiently severe to warrant specific clinical attention."^^xsd:string ;
    skos:prefLabel "Secondary mood syndrome"^^xsd:string .

icd-kg:Secondary_neurodevelopmental_syndrome a owl:Class ;
    icd-schema:exclusion icd-kg:Autism_spectrum,
        icd-kg:Of_intellectual_development,
        icd-kg:Stereotyped_movement ;
    rdfs:subClassOf icd-kg:Neurodevelopmental,
        icd-kg:Secondary_mental_or_behavioural_syndromes_associated_with_or_diseases_classified_elsewhere ;
    skos:definition """A syndrome that involves significant neurodevelopmental features that do not fulfill the diagnostic requirements of any of the specific neurodevelopmental disorders that is judged to be a direct pathophysiological consequence of a health condition not classified under mental and behavioural disorders (e.g., autistic-like features in Rett syndrome; aggression and self-mutilation in Lesch-Nyhan syndrome, abnormalities in language development in Williams syndrome), based on evidence from the history, physical examination, or laboratory findings.

This category should be used in addition to the diagnosis for the presumed underlying disorder or disease when the neurodevelopmental problems are sufficiently severe to warrant specific clinical attention."""^^xsd:string ;
    skos:prefLabel "Secondary neurodevelopmental syndrome"^^xsd:string .

icd-kg:Secondary_psychotic_syndrome a owl:Class ;
    icd-schema:exclusion icd-kg:Acute_and_transient_psychotic,
        icd-kg:Delirium,
        icd-kg:Mood ;
    rdfs:subClassOf icd-kg:Schizophrenia_or_other_primary_psychotic,
        icd-kg:Secondary_mental_or_behavioural_syndromes_associated_with_or_diseases_classified_elsewhere ;
    skos:definition "A syndrome characterised by the presence of prominent hallucinations or delusions judged to be a direct pathophysiological consequence of a health condition not classified under mental and behavioural disorders, based on evidence from the history, physical examination, or laboratory findings. The symptoms are not accounted for by delirium or by another mental and behavioural disorder, and are not a psychologically mediated response to a severe medical condition (e.g., an acute stress reaction in response to a life-threatening diagnosis). This category should be used in addition to the diagnosis for the presumed underlying disorder or disease when the psychotic symptoms are sufficiently severe to warrant specific clinical attention."^^xsd:string ;
    skos:prefLabel "Secondary psychotic syndrome"^^xsd:string .

icd-kg:Sedative_hypnotic_or_anxiolytic_intoxication a owl:Class ;
    icd-schema:exclusion <http://id.who.int/icd/entity/305023629> ;
    icd-schema:inclusion "\"Bad trips\" due to sedatives, hypnotics or anxiolytics"^^xsd:string ;
    rdfs:subClassOf icd-kg:Sedatives_hypnotics_or_anxiolytics ;
    skos:definition "Sedative, hypnotic or anxiolytic intoxication is a clinically significant transient condition that develops during or shortly after the consumption of sedatives, hypnotics or anxiolytics that is characterised by disturbances in consciousness, cognition, perception, affect, behaviour, or coordination. These disturbances are caused by the known pharmacological effects of sedatives, hypnotics or anxiolytics and their intensity is closely related to the amount of sedatives, hypnotics or anxiolytics consumed. They are time-limited and abate as sedatives, hypnotics or anxiolytics are cleared from the body. Presenting features may include somnolence, impaired judgment, inappropriate behavior (including sexual behavior or aggression), slurred speech, impaired motor coordination, unsteady gait, mood changes, as well as impaired memory, attention and concentration. Nystagmus (repetitive, uncontrolled eye movements) is a common physical sign. In severe cases stupor or coma may occur."^^xsd:string ;
    skos:prefLabel "Sedative hypnotic or anxiolytic intoxication"^^xsd:string .

icd-kg:Sedative_hypnotic_or_anxiolytic_withdrawal a owl:Class ;
    rdfs:subClassOf icd-kg:Sedatives_hypnotics_or_anxiolytics ;
    skos:definition "Sedative, hypnotic or anxiolytic withdrawal is a clinically significant cluster of symptoms, behaviours and/or physiological features, varying in degree of severity and duration, that occurs upon cessation or reduction of use of sedatives, hypnotics or anxiolytics in individuals who have developed dependence or have used sedatives, hypnotics or anxiolytics for a prolonged period or in large amounts. Sedative, hypnotic or anxiolytic withdrawal can also occur when prescribed sedatives, hypnotics or anxiolytics have been used in standard therapeutic doses. Presenting features of Sedative, hypnotic or anxiolytic withdrawal may include anxiety, psychomotor agitation, insomnia, increased hand tremor, nausea or vomiting, and transient visual, tactile or auditory illusions or hallucinations. There may be signs of autonomic hyperactivity (e.g., tachycardia, hypertension, sweating), or postural hypotension. The withdrawal state may be complicated by seizures. Less commonly, there may be progression to a more severe withdrawal state characterised by confusion and disorientation, delusions, and more prolonged visual, tactile or auditory hallucinations. In such cases, a separate diagnosis of Sedative, hypnotic, or anxiolytic-induced delirium should be assigned."^^xsd:string ;
    skos:prefLabel "Sedative hypnotic or anxiolytic withdrawal"^^xsd:string .

icd-kg:Sedative_hypnotic_or_anxiolyticinduced_delirium a owl:Class ;
    icd-schema:inclusion "Delirium induced by sedative, hypnotic or anxiolytic withdrawal"^^xsd:string ;
    rdfs:subClassOf icd-kg:Delirium_psychoactive_substances_including_medications,
        icd-kg:Sedatives_hypnotics_or_anxiolytics ;
    skos:definition "Sedative, hypnotic or anxiolytic-induced delirium is characterised by an acute state of disturbed attention and awareness with specific features of delirium that develops during or soon after substance intoxication or withdrawal or during the use of sedatives, hypnotics, or anxiolytics. Specific features of Sedative, hypnotic or anxiolytic-induced delirium may include confusion and disorientation, paranoid delusions, and recurrent visual, tactile or auditory hallucinations. The amount and duration of sedative, hypnotic, or anxiolytic use must be capable of producing delirium. The symptoms are not better explained by a primary mental disorder, by use of or withdrawal from a different substance, or by another health condition that is not classified under Mental, behavioural and neurodevelopmental disorders."^^xsd:string ;
    skos:prefLabel "Sedative hypnotic or anxiolyticinduced delirium"^^xsd:string .

icd-kg:Sedative_hypnotic_or_anxiolyticinduced_mood a owl:Class ;
    rdfs:subClassOf icd-kg:Certain_specified_sedatives_hypnotics_or_anxiolyticinduced_mental_or_behavioural,
        icd-kg:Substanceinduced_mood ;
    skos:definition "Sedative, hypnotic or anxiolytic-induced mood disorder is characterised by mood symptoms (e.g., depressed or elevated mood, decreased engagement in pleasurable activities, increased or decreased energy levels) that develop during or soon after intoxication with or withdrawal from sedatives, hypnotics or anxiolytics. The intensity or duration of the symptoms is substantially in excess of mood disturbances that are characteristic of intoxication or withdrawal due to sedatives, hypnotics or anxiolytics. The amount and duration of sedative, hypnotic or anxiolytic use must be capable of producing mood symptoms. The symptoms are not better explained by a primary mental disorder (e.g., a Depressive disorder, a Bipolar disorder, Schizoaffective disorder), as might be the case if the mood symptoms preceded the onset of the sedative, hypnotic or anxiolytic use, if the symptoms persist for a substantial period of time after cessation of the sedative, hypnotic or anxiolytic use or withdrawal, or if there is other evidence of a pre-existing primary mental disorder with mood symptoms (e.g., a history of prior episodes not associated with sedative, hypnotic or anxiolytic use)."^^xsd:string ;
    skos:prefLabel "Sedative hypnotic or anxiolyticinduced mood"^^xsd:string .

icd-kg:Selfinflicted_hairdamaging a owl:Class ;
    rdfs:subClassOf icd-kg:Bodyfocused_repetitive_behaviour ;
    skos:definition "Hair disorders resulting from an irresistible compulsion to inflict damage on the hair by pulling, twisting, cutting etc."^^xsd:string ;
    skos:prefLabel "Selfinflicted hairdamaging"^^xsd:string .

icd-kg:Severe_personality a owl:Class ;
    rdfs:subClassOf icd-kg:Personality ;
    skos:definition "All general diagnostic requirements for Personality Disorder are met. There are severe disturbances in functioning of the self (e.g., sense of self may be so unstable that individuals report not having a sense of who they are or so rigid that they refuse to participate in any but an extremely narrow range of situations; self view may be characterised by self-contempt or be grandiose or highly eccentric). Problems in interpersonal functioning seriously affect virtually all relationships and the ability and willingness to perform expected social and occupational roles is absent or severely compromised. Specific manifestations of personality disturbance are severe and affect most, if not all, areas of personality functioning. Severe Personality Disorder is often associated with harm to self or others, and is associated with severe impairment in all or nearly all areas of life, including personal, family, social, educational, occupational, and other important areas of functioning."^^xsd:string ;
    skos:prefLabel "Severe personality"^^xsd:string .

icd-kg:Sexual_dysfunction_associated_with_pelvic_organ_prolapse a owl:Class ;
    rdfs:subClassOf icd-kg:Sexual_dysfunctions ;
    skos:definition "A condition affecting women, characterised by difficulties experienced in the sensations or function of the genital system during normal sexual activity. This condition is associated with abnormal displacement of the vagina, introitus, or pelvic floor tissues."^^xsd:string ;
    skos:prefLabel "Sexual dysfunction associated with pelvic organ prolapse"^^xsd:string .

icd-kg:Single_episode_depressive_mild a owl:Class ;
    rdfs:subClassOf icd-kg:Single_episode_depressive ;
    skos:definition "Single episode depressive disorder, mild, is diagnosed when the definitional requirements of a Depressive episode are met and the episode is of mild severity. A depressive episode is characterised by a period of depressed mood or diminished interest in activities occurring most of the day, nearly every day during a period lasting at least two weeks accompanied by other symptoms such as difficulty concentrating, feelings of worthlessness or excessive or inappropriate guilt, hopelessness, recurrent thoughts of death or suicide, changes in appetite or sleep, psychomotor agitation or retardation, and reduced energy or fatigue. In a mild depressive episode, the individual is usually distressed by the symptoms and has some difficulty in continuing to function in one or more domains (personal, family, social, educational, occupational, or other important domains). There are no delusions or hallucinations during the episode."^^xsd:string ;
    skos:prefLabel "Single episode depressive mild"^^xsd:string .

icd-kg:Single_episode_depressive_moderate_with_psychotic_symptoms a owl:Class ;
    rdfs:subClassOf icd-kg:Single_episode_depressive ;
    skos:definition "Single episode depressive disorder, moderate, with psychotic symptoms is diagnosed when the definitional requirements of a depressive episode have been met, there is no history of prior depressive episodes, the episode is of moderate severity, and there are delusions or hallucinations during the episode. A depressive episode is characterised by a period of depressed mood or diminished interest in activities occurring most of the day, nearly every day during a period lasting at least two weeks accompanied by other symptoms such as difficulty concentrating, feelings of worthlessness or excessive or inappropriate guilt, hopelessness, recurrent thoughts of death or suicide, changes in appetite or sleep, psychomotor agitation or retardation, and reduced energy or fatigue. In a moderate depressive episode, several symptoms of a depressive episode are present to a marked degree, or a large number of depressive symptoms of lesser severity are present overall. The individual typically has considerable difficulty functioning in multiple domains (personal, family, social, educational, occupational, or other important domains)."^^xsd:string ;
    skos:prefLabel "Single episode depressive moderate with psychotic symptoms"^^xsd:string .

icd-kg:Single_episode_depressive_moderate_without_psychotic_symptoms a owl:Class ;
    rdfs:subClassOf icd-kg:Single_episode_depressive ;
    skos:definition "Single episode depressive disorder, moderate, without psychotic symptoms is diagnosed when the definitional requirements of a depressive episode have been met, there is no history of prior depressive episodes, the episode is of moderate severity, and there are no delusions or hallucinations during the episode. A depressive episode is characterised by a period of depressed mood or diminished interest in activities occurring most of the day, nearly every day during a period lasting at least two weeks accompanied by other symptoms such as difficulty concentrating, feelings of worthlessness or excessive or inappropriate guilt, hopelessness, recurrent thoughts of death or suicide, changes in appetite or sleep, psychomotor agitation or retardation, and reduced energy or fatigue. In a moderate depressive episode, several symptoms of a depressive episode are present to a marked degree, or a large number of depressive symptoms of lesser severity are present overall. The individual typically has considerable difficulty functioning in multiple domains (personal, family, social, educational, occupational, or other important domains)."^^xsd:string ;
    skos:prefLabel "Single episode depressive moderate without psychotic symptoms"^^xsd:string .

icd-kg:Single_episode_depressive_severe_with_psychotic_symptoms a owl:Class ;
    rdfs:subClassOf icd-kg:Single_episode_depressive ;
    skos:definition "Single episode depressive disorder, severe, with psychotic symptoms is diagnosed when the definitional requirements for Single episode depressive disorder are met and the current episode is severe and there are delusions or hallucinations during the episode. A depressive episode is characterised by a period of depressed mood or diminished interest in activities occurring most of the day, nearly every day during a period lasting at least two weeks accompanied by other symptoms such as difficulty concentrating, feelings of worthlessness or excessive or inappropriate guilt, hopelessness, recurrent thoughts of death or suicide, changes in appetite or sleep, psychomotor agitation or retardation, and reduced energy or fatigue. In a severe depressive episode, many or most symptoms of a Depressive Episode are present to a marked degree, or a smaller number of symptoms are present and manifest to an intense degree. The individual has serious difficulty continuing to function in most domains (personal, family, social, educational, occupational, or other important domains). In a severe depressive episode, many or most symptoms of a Depressive Episode are present to a marked degree, or a smaller number of symptoms are present and manifest to an intense degree. The individual has serious difficulty continuing to function in most domains (personal, family, social, educational, occupational, or other important domains)."^^xsd:string ;
    skos:prefLabel "Single episode depressive severe with psychotic symptoms"^^xsd:string .

icd-kg:Single_episode_depressive_severe_without_psychotic_symptoms a owl:Class ;
    icd-schema:inclusion "Major depression single episode without psychotic symptoms"^^xsd:string,
        "Vital depression single episode without psychotic symptoms"^^xsd:string ;
    rdfs:subClassOf icd-kg:Single_episode_depressive ;
    skos:definition "Single episode depressive disorder, severe, without psychotic symptoms is diagnosed when the definitional requirements for Single episode depressive disorder are met and the current episode is severe and there are no delusions or hallucinations during the episode. A depressive episode is characterised by a period of depressed mood or diminished interest in activities occurring most of the day, nearly every day during a period lasting at least two weeks accompanied by other symptoms such as difficulty concentrating, feelings of worthlessness or excessive or inappropriate guilt, hopelessness, recurrent thoughts of death or suicide, changes in appetite or sleep, psychomotor agitation or retardation, and reduced energy or fatigue. In a severe depressive episode, many or most symptoms of a Depressive Episode are present to a marked degree, or a smaller number of symptoms are present and manifest to an intense degree. The individual has serious difficulty continuing to function in most domains (personal, family, social, educational, occupational, or other important domains)."^^xsd:string ;
    skos:prefLabel "Single episode depressive severe without psychotic symptoms"^^xsd:string .

icd-kg:Sleeprelated_movement_a_medical_condition a owl:Class ;
    rdfs:subClassOf icd-kg:Sleeprelated_movement ;
    skos:definition "Sleep-related movement disorder due to a medical condition is characterised by sleep-related movement abnormalities that are directly attributable to an underlying neurological or medical condition. Many medical conditions, particularly diseases of the nervous system, may be associated with movement abnormalities that are evident in wake and sleep. In some cases, the nocturnal manifestations of the movement abnormalities may be apparent before establishment of a firm neurological diagnosis. Once the presence of a medical or neurological condition is clearly established, this diagnosis should only be assigned if the sleep-related aspects of the movement abnormality or its sequelae are the focus of independent clinical attention."^^xsd:string ;
    skos:prefLabel "Sleeprelated movement a medical condition"^^xsd:string .

icd-kg:Specific_phobia a owl:Class ;
    icd-schema:exclusion icd-kg:Body_dysmorphic,
        icd-kg:Hypochondriasis ;
    icd-schema:inclusion "Simple phobia"^^xsd:string ;
    rdfs:subClassOf icd-kg:Anxiety_or_fearrelated ;
    skos:definition "Specific phobia is characterised by a marked and excessive fear or anxiety that consistently occurs upon exposure or anticipation of exposure to one or more specific objects or situations (e.g., proximity to certain animals, flying, heights, closed spaces, sight of blood or injury) that is out of proportion to actual danger. The phobic objects or situations are avoided or else endured with intense fear or anxiety. Symptoms persist for at least several months and are sufficiently severe to result in significant distress or significant impairment in personal, family, social, educational, occupational, or other important areas of functioning."^^xsd:string ;
    skos:prefLabel "Specific phobia"^^xsd:string .

icd-kg:Speech_sound a owl:Class ;
    icd-schema:exclusion <http://id.who.int/icd/entity/1296093776>,
        <http://id.who.int/icd/entity/15113838>,
        <http://id.who.int/icd/entity/1703207856>,
        <http://id.who.int/icd/entity/947280473> ;
    icd-schema:inclusion "Functional speech articulation disorder"^^xsd:string ;
    rdfs:subClassOf icd-kg:Speech_or_language ;
    skos:definition "Developmental speech sound disorder is characterised by difficulties in the acquisition, production and perception of speech that result in errors of pronunciation, either in number or types of speech errors made or the overall quality of speech production, that are outside the limits of normal variation expected for age and level of intellectual functioning and result in reduced intelligibility and significantly affect communication. The errors in pronunciation arise during the early developmental period and cannot be explained by social, cultural, and other environmental variations (e.g., regional dialects). The speech errors are not fully explained by a hearing impairment or a structural or neurological abnormality."^^xsd:string ;
    skos:prefLabel "Speech sound"^^xsd:string .

icd-kg:Stimulant_intoxication_including_amphetamines_methamphetamine_or_methcathinone a owl:Class ;
    icd-schema:exclusion <http://id.who.int/icd/entity/117248623> ;
    rdfs:subClassOf icd-kg:Stimulants_including_amphetamines_methamphetamine_or_methcathinone ;
    skos:definition "Stimulant intoxication including amphetamines, methamphetamine and methcathinone but excluding caffeine, cocaine and synthetic cathinones is a clinically significant transient condition that develops during or shortly after the consumption of amphetamine or other stimulants that is characterised by disturbances in consciousness, cognition, perception, affect, behaviour, or coordination. These disturbances are caused by the known pharmacological effects of amphetamine or other stimulants and their intensity is closely related to the amount of amphetamine or other stimulant consumed. They are time-limited and abate as amphetamine or another stimulant is cleared from the body. Presenting features may include anxiety, anger, impaired attention, hypervigilance, psychomotor agitation, paranoid ideation (possibly of delusional intensity), transient auditory hallucinations, transitory confusion, and changes in sociability. Perspiration or chills, nausea or vomiting, and palpitations may be experienced. Physical signs may include tachycardia, elevated blood pressure, pupillary dilatation, dyskinesias and dystonias, and skin sores. In rare instances, usually in severe intoxication, use of stimulants including amphetamines, methamphetamine and methcathinone can result in seizures."^^xsd:string ;
    skos:prefLabel "Stimulant intoxication including amphetamines methamphetamine or methcathinone"^^xsd:string .

icd-kg:Stimulantinduced_mood_including_amphetamines_methamphetamine_or_methcathinone a owl:Class ;
    icd-schema:exclusion icd-kg:Caffeine,
        icd-kg:Cocaineinduced_mood,
        icd-kg:Synthetic_cathinoneinduced_mood ;
    rdfs:subClassOf icd-kg:Certain_specified_stimulantinduced_mental_or_behavioural_including_amphetamines_methamphetamine_or_methcathinone,
        icd-kg:Substanceinduced_mood ;
    skos:definition "Stimulant-induced mood disorder including amphetamines, methamphetamine and methcathinone is characterised by mood symptoms (e.g., depressed or elevated mood, decreased engagement in pleasurable activities, increased or decreased energy levels) that develop during or soon after intoxication or withdrawal due to stimulants. The intensity or duration of the symptoms is substantially in excess of mood disturbances that are characteristic of Stimulant intoxication or Stimulant withdrawal. The amount and duration of stimulant use must be capable of producing mood symptoms. The symptoms are not better explained by a primary mental disorder (e.g., a Depressive disorder, a Bipolar disorder, Schizoaffective disorder), as might be the case if the mood symptoms preceded the onset of the stimulant use, if the symptoms persist for a substantial period of time after cessation of the stimulant use or withdrawal, or if there is other evidence of a pre-existing primary mental disorder with mood symptoms (e.g., a history of prior episodes not associated with use of stimulants)."^^xsd:string ;
    skos:prefLabel "Stimulantinduced mood including amphetamines methamphetamine or methcathinone"^^xsd:string .

icd-kg:Stimulantinduced_psychotic_including_amphetamines_methamphetamine_or_methcathinone a owl:Class ;
    icd-schema:exclusion icd-kg:Caffeine,
        icd-kg:Cocaineinduced_psychotic,
        icd-kg:Synthetic_cathinoneinduced_psychotic ;
    rdfs:subClassOf icd-kg:Stimulants_including_amphetamines_methamphetamine_or_methcathinone,
        icd-kg:Substanceinduced_psychotic ;
    skos:definition "Stimulant-induced psychotic disorder including amphetamines, methamphetamine and methcathinone is characterised by psychotic symptoms (e.g., delusions, hallucinations, disorganised thinking, grossly disorganised behaviour) that develop during or soon after intoxication or withdrawal due to stimulants. The intensity or duration of the symptoms is substantially in excess of psychotic-like disturbances of perception, cognition, or behaviour that are characteristic of Stimulant intoxication or Stimulant withdrawal. The amount and duration of stimulant use must be capable of producing psychotic symptoms. The symptoms are not better explained by a primary mental disorder (e.g., Schizophrenia, a Mood disorder with psychotic symptoms), as might be the case if the psychotic symptoms preceded the onset of the stimulant use, if the symptoms persist for a substantial period of time after cessation of the stimulant use or withdrawal, or if there is other evidence of a pre-existing primary mental disorder with psychotic symptoms (e.g., a history of prior episodes not associated with use of stimulants)."^^xsd:string ;
    skos:prefLabel "Stimulantinduced psychotic including amphetamines methamphetamine or methcathinone"^^xsd:string .

icd-kg:Stressrelated_physiological_response_affecting_or_diseases_classified_elsewhere a owl:Class ;
    rdfs:subClassOf icd-kg:Psychological_or_behavioural_factors_affecting_or_diseases_classified_elsewhere ;
    skos:definition "All diagnostic requirements for Psychological or behavioural factors affecting disorders or diseases classified elsewhere are met. The individual exhibits stress-related physiological responses that adversely affect the manifestation, treatment, or course of a disorder or disease classified in another chapter (e.g., stress-related exacerbation of ulcer, hypertension, arrhythmia, or tension headache)."^^xsd:string ;
    skos:prefLabel "Stressrelated physiological response affecting or diseases classified elsewhere"^^xsd:string .

icd-kg:Substanceinduced_anxiety a owl:Class ;
    rdfs:subClassOf icd-kg:Anxiety_or_fearrelated ;
    skos:prefLabel "Substanceinduced anxiety"^^xsd:string .

icd-kg:Substanceinduced_impulse_control a owl:Class ;
    rdfs:subClassOf icd-kg:Impulse_control ;
    skos:prefLabel "Substanceinduced impulse control"^^xsd:string .

icd-kg:Substanceinduced_obsessivecompulsive_or_related a owl:Class ;
    rdfs:subClassOf icd-kg:Obsessivecompulsive_or_related ;
    skos:prefLabel "Substanceinduced obsessivecompulsive or related"^^xsd:string .

icd-kg:Symptomatic_manifestations_of_primary_psychotic a owl:Class ;
    rdfs:subClassOf icd-kg:Schizophrenia_or_other_primary_psychotic ;
    skos:definition "These categories may be used to characterize the current clinical presentation in individuals diagnosed with Schizophrenia or another primary psychotic disorder, and should not be used in individuals without such a diagnosis. Multiple categories may be applied. Symptoms attributable to the direct pathophysiological consequences of a health condition or injury not classified under Mental, behavioural or neurodevelopmental disorders (e.g., a brain tumour or traumatic brain injury), or to the direct effects of a substance or medication on the central nervous system, including withdrawal effects, should not be considered as examples of the respective types of symptoms."^^xsd:string ;
    skos:prefLabel "Symptomatic manifestations of primary psychotic"^^xsd:string .

icd-kg:Synthetic_cannabinoidinduced_mood a owl:Class ;
    rdfs:subClassOf icd-kg:Certain_specified_synthetic_cannabinoidsinduced_mental_or_behavioural,
        icd-kg:Substanceinduced_mood ;
    skos:definition "Synthetic cannabinoid-induced mood disorder is characterised by mood symptoms (e.g., depressed or elevated mood, decreased engagement in pleasurable activities, increased or decreased energy levels) that develop during or soon after intoxication with or withdrawal from synthetic cannabinoids. The intensity or duration of the symptoms is substantially in excess of mood disturbances that are characteristic of Synthetic cannabinoid intoxication or Synthetic cannabinoid withdrawal. The amount and duration of synthetic cannabinoid use must be capable of producing mood symptoms. The symptoms are not better explained by a primary mental disorder (e.g., a Depressive disorder, a Bipolar disorder, Schizoaffective disorder), as might be the case if the mood symptoms preceded the onset of the synthetic cannabinoid use, if the symptoms persist for a substantial period of time after cessation of the synthetic cannabinoid use or withdrawal, or if there is other evidence of a pre-existing primary mental disorder with mood symptoms (e.g., a history of prior episodes not associated with synthetic cannabinoid use)."^^xsd:string ;
    skos:prefLabel "Synthetic cannabinoidinduced mood"^^xsd:string .

icd-kg:Transient_motor_tics a owl:Class ;
    rdfs:subClassOf icd-kg:Primary_tics_or_tic ;
    skos:definition "Tics are sudden, non-rhythmic stereotyped movements such as blinking, sniffing, tapping, etc. They should have been present for less than 1 year."^^xsd:string ;
    skos:prefLabel "Transient motor tics"^^xsd:string .

icd-kg:Vascular_dementia_ischaemic_subtype a owl:Class ;
    rdfs:subClassOf icd-kg:Dementia_cerebrovascular_disease ;
    skos:definition "Dementia due to one or more infarcts of ischemic pathophysiology. There are multiple subtypes depending on the number and location of these infarcts."^^xsd:string ;
    skos:prefLabel "Vascular dementia ischaemic subtype"^^xsd:string .

icd-kg:Volatile_inhalantinduced_mood a owl:Class ;
    rdfs:subClassOf icd-kg:Certain_specified_volatile_inhalantsinduced_mental_or_behavioural,
        icd-kg:Substanceinduced_mood ;
    skos:definition "Volatile inhalant-induced mood disorder is characterised by mood symptoms (e.g., depressed or elevated mood, decreased engagement in pleasurable activities, increased or decreased energy levels) that develop during or soon after intoxication with or withdrawal from volatile inhalants. The intensity or duration of the symptoms is substantially in excess of mood disturbances that are characteristic of Volatile inhalant intoxication or Volatile inhalant withdrawal. The amount and duration of volatile inhalant use must be capable of producing mood symptoms. The symptoms are not better explained by a primary mental disorder (e.g., a Depressive disorder, a Bipolar disorder, Schizoaffective disorder), as might be the case if the mood symptoms preceded the onset of the volatile inhalant use, if the symptoms persist for a substantial period of time after cessation of the volatile inhalant use or withdrawal, or if there is other evidence of a pre-existing primary mental disorder with mood symptoms (e.g., a history of prior episodes not associated with volatile inhalant use)."^^xsd:string ;
    skos:prefLabel "Volatile inhalantinduced mood"^^xsd:string .

icd-kg:Withdrawal_unknown_or_unspecified_psychoactive_substance a owl:Class ;
    rdfs:subClassOf icd-kg:Unknown_or_unspecified_psychoactive_substances ;
    skos:definition "Withdrawal due to unknown or unspecified psychoactive substance is a clinically significant cluster of symptoms, behaviours and/or physiological features, varying in degree of severity and duration, that occurs upon cessation or reduction of use of an unknown or unspecified substance in individuals who have developed dependence or have used the unknown or unspecified substance for a prolonged period or in large amounts. Withdrawal due to unknown or unspecified psychoactive substance can also occur when prescribed psychoactive medications have been used in standard therapeutic doses. The specific features of the withdrawal state depend on the pharmacological properties of the unknown or unspecified substance."^^xsd:string ;
    skos:prefLabel "Withdrawal unknown or unspecified psychoactive substance"^^xsd:string .

icd-kg:hasDiagnosticRequirements a owl:ObjectProperty ;
    rdfs:domain icd-kg:Disease ;
    rdfs:range icd-kg:DiagnosticCriteria .

icd-schema:exclusion a owl:ObjectProperty ;
    rdfs:domain icd-kg:Disease ;
    rdfs:range icd-kg:Disease .

icd-schema:inclusion a owl:DatatypeProperty ;
    rdfs:domain icd-kg:Disease ;
    rdfs:range xsd:string .

schema:drug a owl:ObjectProperty ;
    rdfs:domain icd-kg:Disease ;
    rdfs:range icd-kg:DrugClass .

schema:signOrSymptom a owl:ObjectProperty ;
    rdfs:domain icd-kg:Disease ;
    rdfs:range icd-kg:MedicalSignOrSymptom .

icd-kg:Alcohol_withdrawal a owl:Class ;
    rdfs:subClassOf icd-kg:Alcohol ;
    skos:definition "Alcohol withdrawal is a clinically significant cluster of symptoms, behaviours and/or physiological features, varying in degree of severity and duration, that occurs upon cessation or reduction of use of alcohol in individuals who have developed Alcohol dependence or have used alcohol for a prolonged period or in large amounts. Presenting features of Alcohol withdrawal may include autonomic hyperactivity (e.g. tachycardia, hypertension, perspiration), increased hand tremor, nausea, retching or vomiting, insomnia, anxiety, psychomotor agitation, depressed or dysphoric mood, transient visual, tactile or auditory illusions or hallucinations, and distractability. Less commonly, the withdrawal state is complicated by generalised tonic-clonic seizures. The withdrawal state may progress to a very severe form of delirium characterised by confusion and disorientation, delusions, and prolonged visual, tactile or auditory hallucinations. In such cases, a separate diagnosis of Alcohol-induced delirium should also be assigned."^^xsd:string ;
    skos:prefLabel "Alcohol withdrawal"^^xsd:string .

icd-kg:Amnestic a owl:Class ;
    icd-schema:exclusion icd-kg:Delirium,
        icd-kg:Dementia,
        icd-kg:Mild_neurocognitive ;
    rdfs:subClassOf icd-kg:Neurocognitive ;
    skos:definition "Amnestic disorder is characterised by prominent memory impairment relative to expectations for age and general premorbid level of cognitive functioning, which represents a decline from the individual’s previous level of functioning, in the absence of other significant cognitive impairment. It is manifested by a deficit in acquiring, learning, and/or retaining new information, and may include the inability to recall previously learned information, without disturbance of consciousness, altered mental status, or delirium. Recent memory is typically more disturbed than remote memory, and the ability to immediately recall a limited amount of information is usually relatively preserved. The memory impairment is severe enough to result in significant impairment in personal, family, social, educational, occupational, or other important areas of functioning. It is presumed to be attributable to an underlying acquired disease of the nervous system, a trauma, an infection or other disease process affecting the brain, to use of specific substances or medications, nutritional deficiency or exposure to toxins, or the etiology may be undetermined. The impairment is not due to current substance intoxication or withdrawal."^^xsd:string ;
    skos:prefLabel "Amnestic"^^xsd:string .

icd-kg:Autism_spectrum_with_of_intellectual_development_and_with_impaired_functional_language a owl:Class ;
    rdfs:subClassOf icd-kg:Autism_spectrum ;
    skos:definition "All definitional requirements for both autism spectrum disorder and disorder of intellectual development are met and there is marked impairment in functional language (spoken or signed) relative to the individual’s age, with the individual not able to use more than single words or simple phrases for instrumental purposes, such as to express personal needs and desires."^^xsd:string ;
    skos:prefLabel "Autism spectrum with of intellectual development and with impaired functional language"^^xsd:string .

icd-kg:Cannabis_dependence a owl:Class ;
    icd-schema:exclusion icd-kg:Harmful_pattern_of_cannabis ;
    rdfs:subClassOf icd-kg:Cannabis ;
    skos:definition "Cannabis dependence is a disorder of regulation of cannabis use arising from repeated or continuous use of cannabis. The characteristic feature is a strong internal drive to use cannabis, which is manifested by impaired ability to control use, increasing priority given to use over other activities and persistence of use despite harm or negative consequences. These experiences are often accompanied by a subjective sensation of urge or craving to use cannabis. Physiological features of dependence may also be present, including tolerance to the effects of cannabis, withdrawal symptoms following cessation or reduction in use of cannabis, or repeated use of cannabis or pharmacologically similar substances to prevent or alleviate withdrawal symptoms. The features of dependence are usually evident over a period of at least 12 months but the diagnosis may be made if cannabis use is continuous (daily or almost daily) for at least 3 months."^^xsd:string ;
    skos:prefLabel "Cannabis dependence"^^xsd:string .

icd-kg:Catatonia a owl:Class ;
    icd-schema:exclusion <http://id.who.int/icd/entity/1868408442> ;
    rdfs:subClassOf icd-kg:Mental_behavioural_or_neurodevelopmental_disorders ;
    skos:definition "Catatonia is a syndrome of primarily psychomotor disturbances, characterized by the co-occurrence of several symptoms of decreased, increased, or abnormal psychomotor activity. The assessment of catatonia is complex and requires observation, interview and physical exam. Catatonia can occur in the context of another mental disorder, such as Schizophrenia or Other Primary Psychotic Disorders, Mood Disorders, and Neurodevelopmental Disorders, especially Autism Spectrum Disorder. Catatonia can also develop during or soon after intoxication or withdrawal from certain psychoactive substances, including phencyclidine (PCP), cannabis, hallucinogens such as mescaline or LSD, cocaine and MDMA or related drugs, or during the use of certain psychoactive and non-psychoactive medications (e.g. antipsychotic medications, benzodiazepines, steroids, disulfiram, ciprofloxacin). Finally, Catatonia can occur as a direct pathophysiological consequence of a medical condition not classified under Mental, Behavioural or Neurodevelopmental Disorders. Examples of medical conditions that may be associated with Catatonia include diabetic ketoacidosis, hypercalcemia, hepatic encephalopathy, homocystinuria, neoplasms head trauma, cerebrovascular disease, and encephalitis."^^xsd:string ;
    skos:prefLabel "Catatonia"^^xsd:string .

icd-kg:Certain_multiple_specified_psychoactive_substancesinduced_mental_or_behavioural a owl:Class ;
    rdfs:subClassOf icd-kg:Multiple_specified_psychoactive_substances_including_medications ;
    skos:prefLabel "Certain multiple specified psychoactive substancesinduced mental or behavioural"^^xsd:string .

icd-kg:Certain_other_specified_psychoactive_substanceinduced_mental_or_behavioural a owl:Class ;
    rdfs:subClassOf icd-kg:Other_specified_psychoactive_substances_including_medications ;
    skos:prefLabel "Certain other specified psychoactive substanceinduced mental or behavioural"^^xsd:string .

icd-kg:Certain_specified_alcoholinduced_mental_or_behavioural a owl:Class ;
    rdfs:subClassOf icd-kg:Alcohol ;
    skos:prefLabel "Certain specified alcoholinduced mental or behavioural"^^xsd:string .

icd-kg:Certain_specified_cannabisinduced_mental_or_behavioural a owl:Class ;
    rdfs:subClassOf icd-kg:Cannabis ;
    skos:prefLabel "Certain specified cannabisinduced mental or behavioural"^^xsd:string .

icd-kg:Certain_specified_cocaineinduced_mental_or_behavioural a owl:Class ;
    rdfs:subClassOf icd-kg:Cocaine ;
    skos:prefLabel "Certain specified cocaineinduced mental or behavioural"^^xsd:string .

icd-kg:Certain_specified_dissociative_druginduced_mental_or_behavioural_including_ketamine_and_phencyclidine_%5Bpcp%5D a owl:Class ;
    rdfs:subClassOf icd-kg:Dissociative_drugs_including_ketamine_and_phencyclidine_%5Bpcp%5D ;
    skos:prefLabel "Certain specified dissociative druginduced mental or behavioural including ketamine and phencyclidine [pcp]"^^xsd:string .

icd-kg:Certain_specified_hallucinogeninduced_mental_or_behavioural a owl:Class ;
    rdfs:subClassOf icd-kg:Hallucinogens ;
    skos:prefLabel "Certain specified hallucinogeninduced mental or behavioural"^^xsd:string .

icd-kg:Certain_specified_mdma_or_related_druginduced_mental_or_behavioural_including_mda a owl:Class ;
    rdfs:subClassOf icd-kg:Mdma_or_related_drugs_including_mda ;
    skos:prefLabel "Certain specified mdma or related druginduced mental or behavioural including mda"^^xsd:string .

icd-kg:Certain_specified_opioidinduced_mental_or_behavioural a owl:Class ;
    rdfs:subClassOf icd-kg:Opioids ;
    skos:prefLabel "Certain specified opioidinduced mental or behavioural"^^xsd:string .

icd-kg:Certain_specified_sedatives_hypnotics_or_anxiolyticinduced_mental_or_behavioural a owl:Class ;
    rdfs:subClassOf icd-kg:Sedatives_hypnotics_or_anxiolytics ;
    skos:prefLabel "Certain specified sedatives hypnotics or anxiolyticinduced mental or behavioural"^^xsd:string .

icd-kg:Certain_specified_stimulantinduced_mental_or_behavioural_including_amphetamines_methamphetamine_or_methcathinone a owl:Class ;
    rdfs:subClassOf icd-kg:Stimulants_including_amphetamines_methamphetamine_or_methcathinone ;
    skos:prefLabel "Certain specified stimulantinduced mental or behavioural including amphetamines methamphetamine or methcathinone"^^xsd:string .

icd-kg:Certain_specified_synthetic_cannabinoidsinduced_mental_or_behavioural a owl:Class ;
    rdfs:subClassOf icd-kg:Synthetic_cannabinoids ;
    skos:prefLabel "Certain specified synthetic cannabinoidsinduced mental or behavioural"^^xsd:string .

icd-kg:Certain_specified_synthetic_cathinoneinduced_mental_or_behavioural a owl:Class ;
    rdfs:subClassOf icd-kg:Synthetic_cathinones ;
    skos:prefLabel "Certain specified synthetic cathinoneinduced mental or behavioural"^^xsd:string .

icd-kg:Certain_specified_volatile_inhalantsinduced_mental_or_behavioural a owl:Class ;
    rdfs:subClassOf icd-kg:Volatile_inhalants ;
    skos:prefLabel "Certain specified volatile inhalantsinduced mental or behavioural"^^xsd:string .

icd-kg:Certain_unknown_or_unspecified_psychoactive_substanceinduced_mental_or_behavioural a owl:Class ;
    rdfs:subClassOf icd-kg:Unknown_or_unspecified_psychoactive_substances ;
    skos:prefLabel "Certain unknown or unspecified psychoactive substanceinduced mental or behavioural"^^xsd:string .

icd-kg:Cocaineinduced_mood a owl:Class ;
    rdfs:subClassOf icd-kg:Certain_specified_cocaineinduced_mental_or_behavioural,
        icd-kg:Substanceinduced_mood ;
    skos:definition "Cocaine-induced mood disorder is characterised by mood symptoms (e.g., depressed or elevated mood, decreased engagement in pleasurable activities, increased or decreased energy levels) that develop during or soon after intoxication with or withdrawal from cocaine. The intensity or duration of the symptoms is substantially in excess of mood disturbances that are characteristic of Cocaine intoxication or Cocaine withdrawal. The amount and duration of cocaine use must be capable of producing mood symptoms. The symptoms are not better explained by a primary mental disorder (e.g., a Depressive disorder, a Bipolar disorder, Schizoaffective disorder), as might be the case if the mood symptoms preceded the onset of the cocaine use, if the symptoms persist for a substantial period of time after cessation of the cocaine use or withdrawal, or if there is other evidence of a pre-existing primary mental disorder with mood symptoms (e.g., a history of prior episodes not associated with cocaine use)."^^xsd:string ;
    skos:prefLabel "Cocaineinduced mood"^^xsd:string .

icd-kg:Cocaineinduced_psychotic a owl:Class ;
    rdfs:subClassOf icd-kg:Cocaine,
        icd-kg:Substanceinduced_psychotic ;
    skos:definition "Cocaine-induced psychotic disorder is characterised by psychotic symptoms (e.g. delusions, hallucinations, disorganised thinking, grossly disorganised behaviour) that develop during or soon after intoxication with or withdrawal from cocaine. The intensity or duration of the symptoms is substantially in excess of psychotic-like disturbances of perception, cognition, or behaviour that are characteristic of Cocaine intoxication or Cocaine withdrawal. The amount and duration of cocaine use must be capable of producing psychotic symptoms. The symptoms are not better explained by a primary mental disorder (e.g. Schizophrenia, a Mood disorder with psychotic symptoms), as might be the case if the psychotic symptoms preceded the onset of the cocaine use, if the symptoms persist for a substantial period of time after cessation of the cocaine use or withdrawal, or if there is other evidence of a pre-existing primary mental disorder with psychotic symptoms (e.g. a history of prior episodes not associated with cocaine use)."^^xsd:string ;
    skos:prefLabel "Cocaineinduced psychotic"^^xsd:string .

icd-kg:Complex_post_traumatic_stress a owl:Class ;
    icd-schema:exclusion icd-kg:Personality,
        icd-kg:Post_traumatic_stress ;
    rdfs:subClassOf icd-kg:Specifically_associated_with_stress ;
    skos:definition "Complex post traumatic stress disorder (Complex PTSD) is a disorder that may develop following exposure to an event or series of events of an extremely threatening or horrific nature, most commonly prolonged or repetitive events from which escape is difficult or impossible (e.g. torture, slavery, genocide campaigns, prolonged domestic violence, repeated childhood sexual or physical abuse). All diagnostic requirements for PTSD are met. In addition, Complex PTSD is characterised by severe and persistent 1) problems in affect regulation; 2) beliefs about oneself as diminished, defeated or worthless, accompanied by feelings of shame, guilt or failure related to the traumatic event; and 3) difficulties in sustaining relationships and in feeling close to others. These symptoms cause significant impairment in personal, family, social, educational, occupational or other important areas of functioning."^^xsd:string ;
    skos:prefLabel "Complex post traumatic stress"^^xsd:string .

icd-kg:Cyclothymic a owl:Class ;
    icd-schema:inclusion "Cycloid personality"^^xsd:string,
        "Cyclothymic personality"^^xsd:string ;
    rdfs:subClassOf icd-kg:Bipolar_or_related ;
    skos:definition "Cyclothymic disorder is characterised by a persistent instability of mood over a period of at least 2 years, involving numerous periods of hypomanic (e.g., euphoria, irritability, or expansiveness, psychomotor activation) and depressive (e.g., feeling down, diminished interest in activities, fatigue) symptoms that are present during more of the time than not. The hypomanic symptomatology may or may not be sufficiently severe or prolonged to meet the full definitional requirements of a hypomanic episode (see Bipolar type II disorder), but there is no history of manic or mixed episodes (see Bipolar type I disorder). The depressive symptomatology has never been sufficiently severe or prolonged to meet the diagnostic requirements for a depressive episode (see Bipolar type II disorder). The symptoms result in significant distress or significant impairment in personal, family, social, educational, occupational or other important areas of functioning."^^xsd:string ;
    skos:prefLabel "Cyclothymic"^^xsd:string .

icd-kg:Dementia_cerebrovascular_disease a owl:Class ;
    rdfs:subClassOf icd-kg:Dementia ;
    skos:definition "Dementia due to brain parenchyma injury resulting from cerebrovascular disease (ischemic or haemorrhagic). The onset of the cognitive deficits is temporally related to one or more vascular events. Cognitive decline is typically most prominent in speed of information processing, complex attention, and frontal-executive functioning. There is evidence of the presence of cerebrovascular disease considered to be sufficient to account for the neurocognitive deficits from history, physical examination and neuroimaging."^^xsd:string ;
    skos:prefLabel "Dementia cerebrovascular disease"^^xsd:string .

icd-kg:Dementia_certain_specified_of_the_central_nervous_system a owl:Class ;
    rdfs:subClassOf icd-kg:Dementia_diseases_classified_elsewhere ;
    skos:prefLabel "Dementia certain specified of the central nervous system"^^xsd:string .

icd-kg:Dissociative_drug_dependence_including_ketamine_or_pcp a owl:Class ;
    icd-schema:exclusion icd-kg:Harmful_pattern_of_dissociative_drugs_including_ketamine_or_pcp ;
    rdfs:subClassOf icd-kg:Dissociative_drugs_including_ketamine_and_phencyclidine_%5Bpcp%5D ;
    skos:definition "Dissociative drug dependence including ketamine or PCP is a disorder of regulation of dissociative drug use arising from repeated or continuous use of dissociative drugs. The characteristic feature is a strong internal drive to use dissociative drugs, which is manifested by impaired ability to control use, increasing priority given to use over other activities and persistence of use despite harm or negative consequences. These experiences are often accompanied by a subjective sensation of urge or craving to use dissociative drugs. The features of dependence are usually evident over a period of at least 12 months but the diagnosis may be made if dissociative drugs use is continuous (daily or almost daily) for at least 3 months."^^xsd:string ;
    skos:prefLabel "Dissociative drug dependence including ketamine or pcp"^^xsd:string .

icd-kg:Dissociative_neurological_symptom_with_movement_disturbance a owl:Class ;
    rdfs:subClassOf icd-kg:Dissociative_neurological_symptom ;
    skos:definition "Dissociative neurological symptom disorder, with movement disturbance is characterised by symptoms such as chorea, myoclonus, tremor, dystonia, facial spasm, parkinsonism, or dyskinesia that are not consistent with a recognised disease of the nervous system, other mental, behavioural or neurodevelopmental disorder, or other medical condition and do not occur exclusively during another dissociative disorder."^^xsd:string ;
    skos:prefLabel "Dissociative neurological symptom with movement disturbance"^^xsd:string .

icd-kg:DrugClass a owl:Class ;
    owl:equivalentClass schema:DrugClass ;
    skos:definition "A chemical or biologic substance, used as a medical therapy, that has a physiological effect on an organism. Here the term drug is used interchangeably with the term medicine although clinical knowledge makes a clear difference between them."^^xsd:string ;
    skos:prefLabel "Drug"^^xsd:string ;
    schema:drug icd-kg:Disease .

icd-kg:Excoriation a owl:Class ;
    icd-schema:exclusion icd-kg:Stereotyped_movement,
        <http://id.who.int/icd/entity/1764982361>,
        <http://id.who.int/icd/entity/2102474973> ;
    icd-schema:inclusion "skin picking disorder"^^xsd:string ;
    rdfs:subClassOf icd-kg:Bodyfocused_repetitive_behaviour ;
    skos:definition "Excoriation disorder is characterised by recurrent picking of one’s own skin leading to skin lesions, accompanied by unsuccessful attempts to decrease or stop the behaviour. The most commonly picked sites are the face, arms and hands, but many individuals pick from multiple body sites. Skin picking may occur in brief episodes scattered throughout the day or in less frequent but more sustained periods. The symptoms result in significant distress or significant impairment in personal, family, social, educational, occupational or other important areas of functioning."^^xsd:string ;
    skos:prefLabel "Excoriation"^^xsd:string .

icd-kg:Gaming a owl:Class ;
    icd-schema:exclusion icd-kg:Bipolar_type_i,
        icd-kg:Bipolar_type_ii,
        <http://id.who.int/icd/entity/1586542716> ;
    rdfs:subClassOf icd-kg:Addictive_behaviours,
        icd-kg:Impulse_control ;
    skos:definition """Gaming disorder is characterised by a pattern of persistent or recurrent gaming behaviour (‘digital gaming’ or ‘video-gaming’), which may be online (i.e., over the internet) or offline, manifested by:

1. impaired control over gaming (e.g., onset, frequency, intensity, duration, termination, context);

2. increasing priority given to gaming to the extent that gaming takes precedence over other life interests and daily activities; and

3. continuation or escalation of gaming despite the occurrence of negative consequences.

The pattern of gaming behaviour may be continuous or episodic and recurrent. The pattern of gaming behaviour results in marked distress or significant impairment in personal, family, social, educational, occupational, or other important areas of functioning. The gaming behaviour and other features are normally evident over a period of at least 12 months in order for a diagnosis to be assigned, although the required duration may be shortened if all diagnostic requirements are met and symptoms are severe."""^^xsd:string ;
    skos:prefLabel "Gaming"^^xsd:string .

icd-kg:Gender_incongruence a owl:Class ;
    icd-schema:exclusion icd-kg:Paraphilic ;
    rdfs:subClassOf icd-kg:Mental_behavioural_or_neurodevelopmental_disorders ;
    skos:definition "Gender incongruence is characterised by a marked and persistent incongruence between an individual’s experienced gender and the assigned sex. Gender variant behaviour and preferences alone are not a basis for assigning the diagnoses in this group."^^xsd:string ;
    skos:prefLabel "Gender incongruence"^^xsd:string .

icd-kg:Hallucinogen_dependence a owl:Class ;
    icd-schema:exclusion icd-kg:Harmful_pattern_of_hallucinogens ;
    rdfs:subClassOf icd-kg:Hallucinogens ;
    skos:definition "Hallucinogen dependence is a disorder of regulation of hallucinogen use arising from repeated or continuous use of hallucinogens. The characteristic feature is a strong internal drive to use hallucinogens, which is manifested by impaired ability to control use, increasing priority given to use over other activities and persistence of use despite harm or negative consequences. These experiences are often accompanied by a subjective sensation of urge or craving to use hallucinogens. The features of dependence are usually evident over a period of at least 12 months but the diagnosis may be made if hallucinogens use is continuous (daily or almost daily) for at least 3 months."^^xsd:string ;
    skos:prefLabel "Hallucinogen dependence"^^xsd:string .

icd-kg:Harmful_pattern_of_caffeine a owl:Class ;
    rdfs:subClassOf icd-kg:Caffeine ;
    skos:definition "A pattern of caffeine use that has caused clinically significant harm to a person’s physical or mental health or in which caffeine-induced behaviour has caused clinically significant harm to the health of other people. The pattern of caffeine use is evident over a period of at least 12 months if use is episodic and at least one month if use is continuous (i.e., daily or almost daily). Harm may be caused by the intoxicating effects of caffeine, the direct or secondary toxic effects on body organs and systems, or a harmful route of administration."^^xsd:string ;
    skos:prefLabel "Harmful pattern of caffeine"^^xsd:string .

icd-kg:Harmful_pattern_of_cannabis a owl:Class ;
    icd-schema:exclusion icd-kg:Cannabis_dependence ;
    rdfs:subClassOf icd-kg:Cannabis ;
    skos:definition "A pattern of cannabis use that has caused damage to a person’s physical or mental health or has resulted in behaviour leading to harm to the health of others. The pattern of cannabis use is evident over a period of at least 12 months if substance use is episodic or at least one month if use is continuous (i.e., daily or almost daily). Harm to health of the individual occurs due to one or more of the following: (1) behaviour related to intoxication; (2) direct or secondary toxic effects on body organs and systems; or (3) a harmful route of administration. Harm to health of others includes any form of physical harm, including trauma, or mental disorder that is directly attributable to behaviour related to cannabis intoxication on the part of the person to whom the diagnosis of Harmful pattern of use of cannabis applies."^^xsd:string ;
    skos:prefLabel "Harmful pattern of cannabis"^^xsd:string .

icd-kg:Harmful_pattern_of_dissociative_drugs_including_ketamine_or_pcp a owl:Class ;
    icd-schema:exclusion icd-kg:Dissociative_drug_dependence_including_ketamine_or_pcp ;
    rdfs:subClassOf icd-kg:Dissociative_drugs_including_ketamine_and_phencyclidine_%5Bpcp%5D ;
    skos:definition "A pattern of use of dissociative drugs, including ketamine and phencyclidine (PCP), that has caused damage to a person’s physical or mental health or has resulted in behaviour leading to harm to the health of others. The pattern of dissociative drug use is evident over a period of at least 12 months if use is episodic or at least one month if use is continuous (i.e., daily or almost daily). Harm to health of the individual occurs due to one or more of the following: (1) behaviour related to intoxication; (2) direct or secondary toxic effects on body organs and systems; or (3) a harmful route of administration. Harm to health of others includes any form of physical harm, including trauma, or mental disorder that is directly attributable to behaviour related to dissociative drug intoxication on the part of the person to whom the diagnosis of Harmful pattern of use of dissociative drugs, including ketamine and PCP applies."^^xsd:string ;
    skos:prefLabel "Harmful pattern of dissociative drugs including ketamine or pcp"^^xsd:string .

icd-kg:Harmful_pattern_of_hallucinogens a owl:Class ;
    icd-schema:exclusion icd-kg:Hallucinogen_dependence ;
    rdfs:subClassOf icd-kg:Hallucinogens ;
    skos:definition "A pattern of use of hallucinogens that has caused damage to a person’s physical or mental health or has resulted in behaviour leading to harm to the health of others. The pattern of hallucinogen use is evident over a period of at least 12 months if substance use is episodic or at least one month if use is continuous (i.e., daily or almost daily). Harm to health of the individual occurs due to one or more of the following: (1) behaviour related to intoxication; (2) direct or secondary toxic effects on body organs and systems; or (3) a harmful route of administration. Harm to health of others includes any form of physical harm, including trauma, or mental disorder that is directly attributable to behaviour related to hallucinogen intoxication on the part of the person to whom the diagnosis of Harmful pattern of use of hallucinogens applies."^^xsd:string ;
    skos:prefLabel "Harmful pattern of hallucinogens"^^xsd:string .

icd-kg:Harmful_pattern_of_mdma_or_related_drugs_including_mda a owl:Class ;
    icd-schema:exclusion icd-kg:Mdma_or_related_drug_dependence_including_mda ;
    rdfs:subClassOf icd-kg:Mdma_or_related_drugs_including_mda ;
    skos:definition "A pattern of use of MDMA or related drugs, including MDA, that has caused damage to a person’s physical or mental health or has resulted in behaviour leading to harm to the health of others. The pattern of use of MDMA or related drugs is evident over a period of at least 12 months if use is episodic or at least one month if use is continuous (i.e., daily or almost daily). Harm to health of the individual occurs due to one or more of the following: (1) behaviour related to intoxication; (2) direct or secondary toxic effects on body organs and systems; or (3) a harmful route of administration. Harm to health of others includes any form of physical harm, including trauma, or mental disorder that is directly attributable to behaviour related to MDMA or related drug intoxication on the part of the person to whom the diagnosis of Harmful pattern of use of MDMA or related drugs, including MDA applies."^^xsd:string ;
    skos:prefLabel "Harmful pattern of mdma or related drugs including mda"^^xsd:string .

icd-kg:Harmful_pattern_of_multiple_specified_psychoactive_substances a owl:Class ;
    icd-schema:exclusion icd-kg:Multiple_specified_psychoactive_substances_dependence ;
    rdfs:subClassOf icd-kg:Multiple_specified_psychoactive_substances_including_medications ;
    skos:definition "A pattern of use of multiple specified psychoactive substances or medications that are not included in the other substance classes specifically identified under Disorders Due to Substance Use that has caused damage to a person’s physical or mental health or has resulted in behaviour leading to harm to the health of others. The pattern of substance use is evident over a period of at least 12 months if use is episodic or at least one month if use is continuous (i.e., daily or almost daily). Harm to health of the individual occurs due to one or more of the following: (1) behaviour related to multiple substance intoxication or psychoactive medication use; (2) direct or secondary toxic effects on body organs and systems; or (3) a harmful route of administration. Harm to health of others includes any form of physical harm, including trauma, or mental disorder that is directly attributable to behaviour related to multiple substance intoxication or psychoactive medication use on the part of the person to whom the diagnosis of Harmful pattern of use of multiple specified psychoactive substances applies."^^xsd:string ;
    skos:prefLabel "Harmful pattern of multiple specified psychoactive substances"^^xsd:string .

icd-kg:Harmful_pattern_of_nicotine a owl:Class ;
    icd-schema:exclusion icd-kg:Nicotine_dependence ;
    rdfs:subClassOf icd-kg:Nicotine ;
    skos:definition "A pattern of nicotine use that has caused damage to a person’s physical or mental health. The pattern of nicotine use is evident over a period of at least 12 months if substance use is episodic or at least one month if use is continuous (i.e., daily or almost daily). Harm to health of the individual occurs due to one or more of the following: (1) direct or secondary toxic effects on body organs and systems; or (2) a harmful route of administration."^^xsd:string ;
    skos:prefLabel "Harmful pattern of nicotine"^^xsd:string .

icd-kg:Harmful_pattern_of_opioids a owl:Class ;
    icd-schema:exclusion icd-kg:Opioid_dependence ;
    rdfs:subClassOf icd-kg:Opioids ;
    skos:definition "A pattern of use of opioids that has caused damage to a person’s physical or mental health or has resulted in behaviour leading to harm to the health of others. The pattern of opioid use is evident over a period of at least 12 months if substance use is episodic or at least one month if use is continuous (i.e., daily or almost daily). Harm to health of the individual occurs due to one or more of the following: (1) behaviour related to intoxication; (2) direct or secondary toxic effects on body organs and systems; or (3) a harmful route of administration. Harm to health of others includes any form of physical harm, including trauma, or mental disorder that is directly attributable to behaviour related to opioid intoxication on the part of the person to whom the diagnosis of Harmful pattern of use of opioids applies."^^xsd:string ;
    skos:prefLabel "Harmful pattern of opioids"^^xsd:string .

icd-kg:Harmful_pattern_of_sedatives_hypnotics_or_anxiolytics a owl:Class ;
    icd-schema:exclusion icd-kg:Sedative_hypnotic_or_anxiolytic_dependence ;
    rdfs:subClassOf icd-kg:Sedatives_hypnotics_or_anxiolytics ;
    skos:definition "A pattern of sedative, hypnotic, or anxiolytic use that has caused clinically significant harm to a person’s physical or mental health or in which behaviour induced by sedatives, hypnotics or anxiolytics has caused clinically significant harm to the health of other people. The pattern of sedative, hypnotic, or anxiolytic use is evident over a period of at least 12 months if use is episodic and at least one month if use is continuous (i.e., daily or almost daily). Harm may be caused by the intoxicating effects of sedatives, hypnotics or anxiolytics, the direct or secondary toxic effects on body organs and systems, or a harmful route of administration."^^xsd:string ;
    skos:prefLabel "Harmful pattern of sedatives hypnotics or anxiolytics"^^xsd:string .

icd-kg:Harmful_pattern_of_stimulants_including_amphetamines_methamphetamine_or_methcathinone a owl:Class ;
    icd-schema:exclusion icd-kg:Harmful_pattern_of_caffeine,
        icd-kg:Harmful_pattern_of_cocaine,
        icd-kg:Harmful_pattern_of_synthetic_cathinones,
        icd-kg:Stimulant_dependence_including_amphetamines_methamphetamine_or_methcathinone ;
    rdfs:subClassOf icd-kg:Stimulants_including_amphetamines_methamphetamine_or_methcathinone ;
    skos:definition "A pattern of use of stimulants including amphetamines, methamphetamine and methcathinone but excluding caffeine, cocaine and synthetic cathinones that has caused damage to a person’s physical or mental health or has resulted in behaviour leading to harm to the health of others. The pattern of stimulant use is evident over a period of at least 12 months if substance use is episodic or at least one month if use is continuous. Harm to health of the individual occurs due to one or more of the following: (1) behaviour related to intoxication; (2) direct or secondary toxic effects on body organs and systems; or (3) a harmful route of administration. Harm to health of others includes any form of physical harm, including trauma, or mental disorder that is directly attributable to behaviour related to stimulant intoxication on the part of the person to whom the diagnosis of Harmful pattern of use of stimulants including amphetamines, methamphetamine and methcathinone applies."^^xsd:string ;
    skos:prefLabel "Harmful pattern of stimulants including amphetamines methamphetamine or methcathinone"^^xsd:string .

icd-kg:Harmful_pattern_of_synthetic_cannabinoids a owl:Class ;
    icd-schema:exclusion icd-kg:Synthetic_cannabinoid_dependence ;
    rdfs:subClassOf icd-kg:Synthetic_cannabinoids ;
    skos:definition "A pattern of use of synthetic cannabinoids that has caused damage to a person’s physical or mental health or has resulted in behaviour leading to harm to the health of others. The pattern of synthetic cannabinoid use is evident over a period of at least 12 months if substance use is episodic or at least one month if use is continuous (i.e., daily or almost daily). Harm to health of the individual occurs due to one or more of the following: (1) behaviour related to intoxication; (2) direct or secondary toxic effects on body organs and systems; or (3) a harmful route of administration. Harm to health of others includes any form of physical harm, including trauma, or mental disorder that is directly attributable to behaviour related to synthetic cannabinoid intoxication on the part of the person to whom the diagnosis of Harmful pattern of use of synthetic cannabinoids applies."^^xsd:string ;
    skos:prefLabel "Harmful pattern of synthetic cannabinoids"^^xsd:string .

icd-kg:Harmful_pattern_of_unknown_or_unspecified_psychoactive_substance a owl:Class ;
    icd-schema:exclusion icd-kg:Unknown_or_unspecified_psychoactive_substance_dependence ;
    rdfs:subClassOf icd-kg:Unknown_or_unspecified_psychoactive_substances ;
    skos:definition "A pattern of use of an unknown or unspecified psychoactive substance that has caused damage to a person’s physical or mental health or has resulted in behaviour leading to harm to the health of others. The pattern of substance use is evident over a period of at least 12 months if use is episodic or at least one month if use is continuous (i.e., daily or almost daily). Harm to health of the individual occurs due to one or more of the following: (1) behaviour related to intoxication; (2) direct or secondary toxic effects on body organs and systems; or (3) a harmful route of administration. Harm to health of others includes any form of physical harm, including trauma, or mental disorder that is directly attributable to behaviour related to substance intoxication on the part of the person to whom the diagnosis of Harmful pattern of use of unknown or unspecified psychoactive substance applies."^^xsd:string ;
    skos:prefLabel "Harmful pattern of unknown or unspecified psychoactive substance"^^xsd:string .

icd-kg:Harmful_pattern_of_volatile_inhalants a owl:Class ;
    icd-schema:exclusion icd-kg:Volatile_inhalant_dependence ;
    rdfs:subClassOf icd-kg:Volatile_inhalants ;
    skos:definition "A pattern of volatile inhalant use that has caused damage to a person’s physical or mental health. The pattern of volatile inhalant use is evident over a period of at least 12 months if substance use is episodic or at least one month if use is continuous (i.e., daily or almost daily). Harm to health of the individual occurs due to one or more of the following: (1) behaviour related to intoxication; (1) direct or secondary toxic effects on body organs and systems; or (2) a harmful route of administration. Harm to health of others includes any form of physical harm, including trauma, or mental disorder that is directly attributable to behaviour related to volatile inhalant intoxication on the part of the person to whom the diagnosis of Harmful pattern of use of volatile inhalants applies."^^xsd:string ;
    skos:prefLabel "Harmful pattern of volatile inhalants"^^xsd:string .

icd-kg:Hypersomnolence a owl:Class ;
    rdfs:subClassOf icd-kg:Sleepwake ;
    skos:definition "Hypersomnolence disorders are characterised by a complaint of daytime sleepiness that is not due to another sleep-wake disorder (e.g. disturbed nocturnal sleep, misaligned circadian rhythm, or breathing disorder). Individuals with excessive sleepiness may show irritability, concentration and attention deficits, reduced vigilance, distractibility, reduced motivation, anergia, dysphoria, fatigue, restlessness, and lack of coordination."^^xsd:string ;
    skos:prefLabel "Hypersomnolence"^^xsd:string .

icd-kg:Language_with_impairment_of_receptive_and_expressive_language a owl:Class ;
    icd-schema:exclusion icd-kg:Autism_spectrum,
        <http://id.who.int/icd/entity/1296093776>,
        <http://id.who.int/icd/entity/1705858040>,
        <http://id.who.int/icd/entity/348544271>,
        <http://id.who.int/icd/entity/947280473> ;
    icd-schema:inclusion "developmental dysphasia or aphasia, receptive type"^^xsd:string ;
    rdfs:subClassOf icd-kg:Language ;
    skos:definition "Developmental language disorder with impairment of receptive and expressive language is characterised by persistent difficulties in the acquisition, understanding, production, and use of language that arise during the developmental period, typically during early childhood, and cause significant limitations in the individual’s ability to communicate. The ability to understand spoken or signed language (i.e., receptive language) is markedly below the expected level given the individual’s age and level of intellectual functioning, and is accompanied by persistent impairment in the ability to produce and use spoken or signed language (i.e., expressive language)."^^xsd:string ;
    skos:prefLabel "Language with impairment of receptive and expressive language"^^xsd:string .

icd-kg:Learning a owl:Class ;
    icd-schema:exclusion <http://id.who.int/icd/entity/1875757565> ;
    rdfs:subClassOf icd-kg:Neurodevelopmental ;
    skos:definition "Developmental learning disorder is characterised by significant and persistent difficulties in learning academic skills, which may include reading, writing, or arithmetic. The individual’s performance in the affected academic skill(s) is markedly below what would be expected for chronological age and general level of intellectual functioning, and results in significant impairment in the individual’s academic or occupational functioning. Developmental learning disorder first manifests when academic skills are taught during the early school years. Developmental learning disorder is not due to a disorder of intellectual development, sensory impairment (vision or hearing), neurological or motor disorder, lack of availability of education, lack of proficiency in the language of academic instruction, or psychosocial adversity."^^xsd:string ;
    skos:prefLabel "Learning"^^xsd:string .

icd-kg:Male_early_ejaculation a owl:Class ;
    rdfs:subClassOf icd-kg:Ejaculatory_dysfunctions ;
    skos:definition "Male early ejaculation is characterised by ejaculation that occurs prior to or within a very short duration of the initiation of vaginal penetration or other relevant sexual stimulation, with no or little perceived control over ejaculation. The pattern of early ejaculation has occurred episodically or persistently over a period at least several months, and is associated with clinically significant distress."^^xsd:string ;
    skos:prefLabel "Male early ejaculation"^^xsd:string .

icd-kg:Male_erectile_dysfunction a owl:Class ;
    rdfs:subClassOf icd-kg:Sexual_arousal_dysfunctions ;
    skos:definition "Male erectile dysfunction is characterised by inability or marked reduction in the ability in men to attain or sustain a penile erection of sufficient duration or rigidity to allow for sexual activity. The pattern of erectile difficulty occurs despite the desire for sexual activity and adequate sexual stimulation, has occurred episodically or persistently over a period at least several months, and is associated with clinically significant distress."^^xsd:string ;
    skos:prefLabel "Male erectile dysfunction"^^xsd:string .

icd-kg:Mdma_or_related_drug_dependence_including_mda a owl:Class ;
    icd-schema:exclusion icd-kg:Harmful_pattern_of_mdma_or_related_drugs_including_mda ;
    rdfs:subClassOf icd-kg:Mdma_or_related_drugs_including_mda ;
    skos:definition "MDMA or related drug dependence, including MDA is a disorder of regulation of MDMA or related drug use arising from repeated or continuous use of MDMA or related drugs. The characteristic feature is a strong internal drive to use MDMA or related drugs, which is manifested by impaired ability to control use, increasing priority given to use over other activities and persistence of use despite harm or negative consequences. These experiences are often accompanied by a subjective sensation of urge or craving to use MDMA or related drugs. Physiological features of dependence may also be present, including tolerance to the effects of MDMA or related drugs, withdrawal symptoms following cessation or reduction in use of MDMA or related drugs, or repeated use of MDMA or pharmacologically similar substances to prevent or alleviate withdrawal symptoms. The features of dependence are usually evident over a period of at least 12 months but the diagnosis may be made if MDMA or related drug use is continuous (daily or almost daily) for at least 3 months."^^xsd:string ;
    skos:prefLabel "Mdma or related drug dependence including mda"^^xsd:string .

icd-kg:Motor_coordination a owl:Class ;
    icd-schema:exclusion <http://id.who.int/icd/entity/1296093776>,
        <http://id.who.int/icd/entity/1473673350>,
        <http://id.who.int/icd/entity/1543612222> ;
    rdfs:subClassOf icd-kg:Neurodevelopmental ;
    skos:definition "Developmental motor coordination disorder is characterised by a significant delay in the acquisition of gross and fine motor skills and impairment in the execution of coordinated motor skills that manifest in clumsiness, slowness, or inaccuracy of motor performance. Coordinated motor skills are markedly below that expected given the individual's chronological age and level of intellectual functioning. Onset of coordinated motor skills difficulties occurs during the developmental period and is typically apparent from early childhood. Coordinated motor skills difficulties cause significant and persistent limitations in functioning (e.g. in activities of daily living, school work, and vocational and leisure activities). Difficulties with coordinated motor skills are not solely attributable to a Disease of the Nervous System, Disease of the Musculoskeletal System or Connective Tissue, sensory impairment, and not better explained by a Disorder of Intellectual Development."^^xsd:string ;
    skos:prefLabel "Motor coordination"^^xsd:string .

icd-kg:Multiple_specified_psychoactive_substances_dependence a owl:Class ;
    icd-schema:exclusion icd-kg:Harmful_pattern_of_multiple_specified_psychoactive_substances ;
    rdfs:subClassOf icd-kg:Multiple_specified_psychoactive_substances_including_medications ;
    skos:definition "Multiple specified psychoactive substance dependence is a disorder of regulation of use of multiple specified substances arising from repeated or continuous use of the specified substances. The characteristic feature is a strong internal drive to use the specified substances, which is manifested by impaired ability to control use, increasing priority given to use over other activities and persistence of use despite harm or negative consequences. These experiences are often accompanied by a subjective sensation of urge or craving to use the specified substances. Physiological features of dependence may also be present, including tolerance to the effects of the specified substances, withdrawal symptoms following cessation or reduction in use of the specified substances, or repeated use of the specified substances or pharmacologically similar substances to prevent or alleviate withdrawal symptoms. The features of dependence are usually evident over a period of at least 12 months but the diagnosis may be made if use of the specified substances is continuous (daily or almost daily) for at least 3 months."^^xsd:string ;
    skos:prefLabel "Multiple specified psychoactive substances dependence"^^xsd:string .

icd-kg:Nicotine_dependence a owl:Class ;
    icd-schema:exclusion icd-kg:Harmful_pattern_of_nicotine ;
    rdfs:subClassOf icd-kg:Nicotine ;
    skos:definition "Nicotine dependence is a disorder of regulation of nicotine use arising from repeated or continuous use of nicotine. The characteristic feature is a strong internal drive to use nicotine, which is manifested by impaired ability to control use, increasing priority given to use over other activities and persistence of use despite harm or negative consequences. These experiences are often accompanied by a subjective sensation of urge or craving to use nicotine. Physiological features of dependence may also be present, including tolerance to the effects of nicotine, withdrawal symptoms following cessation or reduction in use of nicotine, or repeated use of nicotine or pharmacologically similar substances to prevent or alleviate withdrawal symptoms. The features of dependence are usually evident over a period of at least 12 months but the diagnosis may be made if nicotine use is continuous (daily or almost daily) for at least 3 months."^^xsd:string ;
    skos:prefLabel "Nicotine dependence"^^xsd:string .

icd-kg:Nonpsychoactive_substances a owl:Class ;
    rdfs:subClassOf icd-kg:Substance_use ;
    skos:definition "Disorders due to use of non-psychoactive substances are characterised by the pattern and consequences of non-medical use of non-psychoactive substances. Non-psychoactive substances include laxatives, anabolic steroids, growth hormone, erythropoietin, and non-steroidal anti-inflammatory drugs. They may also include proprietary or over-the-counter medicines and folk remedies. Non-medical use of these substances may be associated with harm to the individual due to the direct or secondary toxic effects of the non-psychoactive substance on body organs and systems, or a harmful route of administration (e.g., infections due to intravenous self-administration). They are not associated with intoxication or with a dependence or withdrawal syndrome and are not recognized causes of substance-induced mental disorders."^^xsd:string ;
    skos:prefLabel "Nonpsychoactive substances"^^xsd:string .

icd-kg:Of_bodily_distress_or_bodily_experience a owl:Class ;
    icd-schema:exclusion icd-kg:Dissociative_neurological_symptom,
        <http://id.who.int/icd/entity/1100199287> ;
    rdfs:subClassOf icd-kg:Mental_behavioural_or_neurodevelopmental_disorders ;
    skos:definition "Disorders of bodily distress and bodily experience are characterised by disturbances in the person’s experience of his or her body. Bodily distress disorder involves bodily symptoms that the individual finds distressing and to which excessive attention is directed. Body integrity dysphoria involves a disturbance in the person’s experience of the body manifested by the persistent desire to have a specific physical disability accompanied by persistent discomfort, or intense feelings of inappropriateness concerning current non-disabled body configuration."^^xsd:string ;
    skos:prefLabel "Of bodily distress or bodily experience"^^xsd:string .

icd-kg:Opioid_dependence a owl:Class ;
    icd-schema:exclusion icd-kg:Harmful_pattern_of_opioids ;
    rdfs:subClassOf icd-kg:Opioids ;
    skos:definition "Opioid dependence is a disorder of regulation of opioid use arising from repeated or continuous use of opioids. The characteristic feature is a strong internal drive to use opioids, which is manifested by impaired ability to control use, increasing priority given to use over other activities and persistence of use despite harm or negative consequences. These experiences are often accompanied by a subjective sensation of urge or craving to use opioids. Physiological features of dependence may also be present, including tolerance to the effects of opioids, withdrawal symptoms following cessation or reduction in use of opioids, or repeated use of opioids or pharmacologically similar substances to prevent or alleviate withdrawal symptoms. The features of dependence are usually evident over a period of at least 12 months but the diagnosis may be made if opioid use is continuous (daily or almost daily) for at least 3 months."^^xsd:string ;
    skos:prefLabel "Opioid dependence"^^xsd:string .

icd-kg:Opioid_intoxication a owl:Class ;
    icd-schema:exclusion <http://id.who.int/icd/entity/1573091976> ;
    rdfs:subClassOf icd-kg:Opioids ;
    skos:definition "Opioid intoxication is a clinically significant transient condition that develops during or shortly after the consumption of opioids that is characterised by disturbances in consciousness, cognition, perception, affect, behaviour, or coordination. These disturbances are caused by the known pharmacological effects of opioids and their intensity is closely related to the amount of opioids consumed. They are time-limited and abate as opioids are cleared from the body. Presenting features may include somnolence, stupor, mood changes (e.g. euphoria followed by apathy and dysphoria), psychomotor retardation, impaired judgment, respiratory depression, slurred speech, and impairment of memory and attention. In severe intoxication coma may ensue. A characteristic physical sign is pupillary constriction but this sign may be absent when intoxication is due to synthetic opioids. Severe opioid intoxication can lead to death due to respiratory depression."^^xsd:string ;
    skos:prefLabel "Opioid intoxication"^^xsd:string .

icd-kg:Orgasmic_dysfunctions a owl:Class ;
    icd-schema:exclusion icd-kg:Male_early_ejaculation ;
    rdfs:subClassOf icd-kg:Sexual_dysfunctions ;
    skos:definition "Orgasmic dysfunctions refer to difficulties related to the subjective experience of orgasm."^^xsd:string ;
    skos:prefLabel "Orgasmic dysfunctions"^^xsd:string .

icd-kg:Other_specified_psychoactive_substance_dependence a owl:Class ;
    icd-schema:exclusion icd-kg:Harmful_pattern_of_other_specified_psychoactive_substance ;
    rdfs:subClassOf icd-kg:Other_specified_psychoactive_substances_including_medications ;
    skos:definition "Other specified psychoactive substance dependence is a disorder of regulation of use of a specified substance arising from repeated or continuous use of the specified substance. The characteristic feature is a strong internal drive to use the specified substance, which is manifested by impaired ability to control use, increasing priority given to use over other activities and persistence of use despite harm or negative consequences. These experiences are often accompanied by a subjective sensation of urge or craving to use the specified substance. Physiological features of dependence may also be present, including tolerance to the effects of the specified substance, withdrawal symptoms following cessation or reduction in use of the specified substance, or repeated use of the specified substance or pharmacologically similar substances to prevent or alleviate withdrawal symptoms. The features of dependence are usually evident over a period of at least 12 months but the diagnosis may be made if use of the specified substance is continuous (daily or almost daily) for at least 3 months."^^xsd:string ;
    skos:prefLabel "Other specified psychoactive substance dependence"^^xsd:string .

icd-kg:Post_traumatic_stress a owl:Class ;
    icd-schema:exclusion icd-kg:Complex_post_traumatic_stress,
        <http://id.who.int/icd/entity/505909942> ;
    icd-schema:inclusion "Traumatic neurosis"^^xsd:string ;
    rdfs:subClassOf icd-kg:Specifically_associated_with_stress ;
    skos:definition "Post traumatic stress disorder (PTSD) may develop following exposure to an extremely threatening or horrific event or series of events. It is characterised by all of the following: 1) re-experiencing the traumatic event or events in the present in the form of vivid intrusive memories, flashbacks, or nightmares. Re-experiencing may occur via one or multiple sensory modalities and is typically accompanied by strong or overwhelming emotions, particularly fear or horror, and strong physical sensations; 2) avoidance of thoughts and memories of the event or events, or avoidance of activities, situations, or people reminiscent of the event(s); and 3) persistent perceptions of heightened current threat, for example as indicated by hypervigilance or an enhanced startle reaction to stimuli such as unexpected noises. The symptoms persist for at least several weeks and cause significant impairment in personal, family, social, educational, occupational or other important areas of functioning."^^xsd:string ;
    skos:prefLabel "Post traumatic stress"^^xsd:string .

icd-kg:Psychological_or_behavioural_factors_affecting_or_diseases_classified_elsewhere a owl:Class ;
    icd-schema:exclusion icd-kg:Mental_or_behavioural_associated_with_pregnancy_childbirth_or_the_puerperium ;
    icd-schema:inclusion "Psychological factors affecting physical conditions"^^xsd:string ;
    rdfs:subClassOf icd-kg:Mental_behavioural_or_neurodevelopmental_disorders ;
    skos:definition "Psychological and behavioural factors affecting disorders or diseases classified elsewhere are those that may adversely affect the manifestation, treatment, or course of a condition classified in another chapter of the ICD. These factors may adversely affect the manifestation, treatment, or course of the disorder or disease classified in another chapter by: interfering with the treatment of the disorder or disease by affecting treatment adherence or care seeking; constituting an additional health risk; or influencing the underlying pathophysiology to precipitate or exacerbate symptoms or otherwise necessitate medical attention. This diagnosis should be assigned only when the factors increase the risk of suffering, disability, or death and represent a focus of clinical attention, and should be assigned together with the diagnosis for the relevant other condition."^^xsd:string ;
    skos:prefLabel "Psychological or behavioural factors affecting or diseases classified elsewhere"^^xsd:string .

icd-kg:Repetitive_selfbiting_behaviour a owl:Class ;
    icd-schema:exclusion icd-kg:Stereotyped_movement,
        <http://id.who.int/icd/entity/1886495906> ;
    rdfs:subClassOf icd-kg:Bodyfocused_repetitive_behaviour ;
    skos:definition "Self-inflicted skin and mucous membrane damage resulting from a compulsive urge to bite."^^xsd:string ;
    skos:prefLabel "Repetitive selfbiting behaviour"^^xsd:string .

icd-kg:Secondary_neurocognitive_syndrome a owl:Class ;
    icd-schema:exclusion <http://id.who.int/icd/entity/1719545571> ;
    rdfs:subClassOf icd-kg:Neurocognitive,
        icd-kg:Secondary_mental_or_behavioural_syndromes_associated_with_or_diseases_classified_elsewhere ;
    skos:definition "A syndrome that involves significant cognitive features that do not fulfill the diagnostic requirements of any of the specific neurocognitive disorders and are judged to be a direct pathophysiological consequence of a health condition or injury not classified under mental and behavioural disorders (e.g., cognitive changes due to a brain tumour), based on evidence from the history, physical examination, or laboratory findings. This category should be used in addition to the diagnosis for the presumed underlying disorder or disease when the cognitive symptoms are sufficiently severe to warrant specific clinical attention."^^xsd:string ;
    skos:prefLabel "Secondary neurocognitive syndrome"^^xsd:string .

icd-kg:Sedative_hypnotic_or_anxiolytic_dependence a owl:Class ;
    icd-schema:exclusion icd-kg:Harmful_pattern_of_sedatives_hypnotics_or_anxiolytics ;
    rdfs:subClassOf icd-kg:Sedatives_hypnotics_or_anxiolytics ;
    skos:definition "Sedative, hypnotic or anxiolytic dependence is a disorder of regulation of sedative use arising from repeated or continuous use of these substances. The characteristic feature is a strong internal drive to use sedatives, hypnotics, or anxiolytics, which is manifested by impaired ability to control use, increasing priority given to use over other activities and persistence of use despite harm or negative consequences. These experiences are often accompanied by a subjective sensation of urge or craving to use these substances. Physiological features of dependence may also be present, including tolerance to the effects of sedatives, hypnotics or anxiolytics, withdrawal symptoms following cessation or reduction in use, or repeated use of sedatives or pharmacologically similar substances to prevent or alleviate withdrawal symptoms. The features of dependence are usually evident over a period of at least 12 months but the diagnosis may be made if sedative use is continuous (daily or almost daily) for at least 3 months."^^xsd:string ;
    skos:prefLabel "Sedative hypnotic or anxiolytic dependence"^^xsd:string .

icd-kg:Separation_anxiety a owl:Class ;
    icd-schema:exclusion icd-kg:Mood,
        icd-kg:Social_anxiety ;
    rdfs:subClassOf icd-kg:Anxiety_or_fearrelated ;
    skos:definition "Separation anxiety disorder is characterised by marked and excessive fear or anxiety about separation from specific attachment figures. In children and adolescents, separation anxiety typically focuses on caregivers, parents or other family members and the fear or anxiety is beyond what would be considered developmentally normative. In adults, the focus is typically a romantic partner or children. Manifestations of separation anxiety may include thoughts of harm or untoward events befalling the attachment figure, reluctance to go to school or work, recurrent excessive distress upon separation, reluctance or refusal to sleep away from the attachment figure, and recurrent nightmares about separation. The symptoms persist for at least several months and are sufficiently severe to result in significant distress or significant impairment in personal, family, social, educational, occupational, or other important areas of functioning."^^xsd:string ;
    skos:prefLabel "Separation anxiety"^^xsd:string .

icd-kg:Sleeprelated_hypoventilation_or_hypoxemia a owl:Class ;
    rdfs:subClassOf icd-kg:Sleeprelated_breathing ;
    skos:definition """The primary feature of these disorders is insufficient sleep related ventilation, resulting in abnormally elevated arterial partial pressure of carbon dioxide (PaCO2) during sleep. Sleep-related hypoxemia is diagnosed when overnight monitoring reveals sustained (> 5 minutes) decline in oxygen saturation to ≤ 88% in adults (or ≤ 90% in children) for ≥ 5 minutes.

Note: A definitive diagnosis requires objective evidence based on polysomnography as well as carbon dioxide (CO2) monitoring during sleep (by arterial, end-tidal or transcutaneous measures)."""^^xsd:string ;
    skos:prefLabel "Sleeprelated hypoventilation or hypoxemia"^^xsd:string .

icd-kg:Social_anxiety a owl:Class ;
    rdfs:subClassOf icd-kg:Anxiety_or_fearrelated ;
    skos:definition "Social anxiety disorder is characterised by marked and excessive fear or anxiety that consistently occurs in one or more social situations such as social interactions (e.g. having a conversation), doing something while feeling observed (e.g. eating or drinking in the presence of others), or performing in front of others (e.g. giving a speech). The individual is concerned that he or she will act in a way, or show anxiety symptoms, that will be negatively evaluated by others. Relevant social situations are consistently avoided or else endured with intense fear or anxiety. The symptoms persist for at least several months and are sufficiently severe to result in significant distress or significant impairment in personal, family, social, educational, occupational, or other important areas of functioning."^^xsd:string ;
    skos:prefLabel "Social anxiety"^^xsd:string .

icd-kg:Stimulant_dependence_including_amphetamines_methamphetamine_or_methcathinone a owl:Class ;
    icd-schema:exclusion icd-kg:Cocaine_dependence,
        icd-kg:Harmful_pattern_of_stimulants_including_amphetamines_methamphetamine_or_methcathinone,
        icd-kg:Synthetic_cathinone_dependence ;
    rdfs:subClassOf icd-kg:Stimulants_including_amphetamines_methamphetamine_or_methcathinone ;
    skos:definition "Stimulant dependence including amphetamines, methamphetamine or methcathinone is a disorder of regulation of stimulant use arising from repeated or continuous use of stimulants. The characteristic feature is a strong internal drive to use stimulants, which is manifested by impaired ability to control use, increasing priority given to use over other activities and persistence of use despite harm or negative consequences. These experiences are often accompanied by a subjective sensation of urge or craving to use stimulants. Physiological features of dependence may also be present, including tolerance to the effects of stimulants, withdrawal symptoms following cessation or reduction in use of stimulants, or repeated use of stimulants or pharmacologically similar substances to prevent or alleviate withdrawal symptoms. The features of dependence are usually evident over a period of at least 12 months but the diagnosis may be made if stimulant use is continuous (daily or almost daily) for at least 3 months."^^xsd:string ;
    skos:prefLabel "Stimulant dependence including amphetamines methamphetamine or methcathinone"^^xsd:string .

icd-kg:Synthetic_cannabinoid_dependence a owl:Class ;
    icd-schema:exclusion icd-kg:Harmful_pattern_of_synthetic_cannabinoids ;
    rdfs:subClassOf icd-kg:Synthetic_cannabinoids ;
    skos:definition "Synthetic cannabinoid dependence is a disorder of regulation of synthetic cannabinoid use arising from repeated or continuous use of synthetic cannabinoids. The characteristic feature is a strong internal drive to use synthetic cannabinoids, which is manifested by impaired ability to control use, increasing priority given to use over other activities and persistence of use despite harm or negative consequences. These experiences are often accompanied by a subjective sensation of urge or craving to use synthetic cannabinoids. Physiological features of dependence may also be present, including tolerance to the effects of synthetic cannabinoids, withdrawal symptoms following cessation or reduction in use of synthetic cannabinoids, or repeated use of synthetic cannabinoids or pharmacologically similar substances to prevent or alleviate withdrawal symptoms. The features of dependence are usually evident over a period of at least 12 months but the diagnosis may be made if synthetic cannabinoid use is continuous (daily or almost daily) for at least 3 months."^^xsd:string ;
    skos:prefLabel "Synthetic cannabinoid dependence"^^xsd:string .

icd-kg:Synthetic_cathinoneinduced_mood a owl:Class ;
    rdfs:subClassOf icd-kg:Certain_specified_synthetic_cathinoneinduced_mental_or_behavioural,
        icd-kg:Substanceinduced_mood ;
    skos:definition "Synthetic cathinone-induced mood disorder is characterised by mood symptoms (e.g., depressed or elevated mood, decreased engagement in pleasurable activities, increased or decreased energy levels) that develop during or soon after intoxication with or withdrawal from synthetic cathinones. The intensity or duration of the symptoms is substantially in excess of mood disturbances that are characteristic of Synthetic cathinone intoxication or Synthetic cathinone withdrawal. The amount and duration of synthetic cathinone use must be capable of producing mood symptoms. The symptoms are not better explained by a primary mental disorder (e.g., a Depressive disorder, a Bipolar disorder, Schizoaffective disorder), as might be the case if the mood symptoms preceded the onset of the synthetic cathinone use, if the symptoms persist for a substantial period of time after cessation of the synthetic cathinone use or withdrawal, or if there is other evidence of a pre-existing primary mental disorder with mood symptoms (e.g., a history of prior episodes not associated with synthetic cathinone use)."^^xsd:string ;
    skos:prefLabel "Synthetic cathinoneinduced mood"^^xsd:string .

icd-kg:Synthetic_cathinoneinduced_psychotic a owl:Class ;
    rdfs:subClassOf icd-kg:Substanceinduced_psychotic,
        icd-kg:Synthetic_cathinones ;
    skos:definition "Synthetic cathinone-induced psychotic disorder is characterised by psychotic symptoms (e.g., delusions, hallucinations, disorganised thinking, grossly disorganised behaviour) that develop during or soon after intoxication with or withdrawal from synthetic cathinones. The intensity or duration of the symptoms is substantially in excess of psychotic-like disturbances of perception, cognition, or behaviour that are characteristic of Synthetic cathinone intoxication or Synthetic cathinone withdrawal. The amount and duration of synthetic cathinone use must be capable of producing psychotic symptoms. The symptoms are not better explained by a primary mental disorder (e.g., Schizophrenia, a Mood disorder with psychotic symptoms), as might be the case if the psychotic symptoms preceded the onset of the synthetic cathinone use, if the symptoms persist for a substantial period of time after cessation of the synthetic cathinone use or withdrawal, or if there is other evidence of a pre-existing primary mental disorder with psychotic symptoms (e.g., a history of prior episodes not associated with synthetic cathinone use)."^^xsd:string ;
    skos:prefLabel "Synthetic cathinoneinduced psychotic"^^xsd:string .

icd-kg:Tourette_syndrome a owl:Class ;
    icd-schema:inclusion "Combined vocal and multiple motor tic disorder"^^xsd:string ;
    rdfs:subClassOf icd-kg:Obsessivecompulsive_or_related,
        icd-kg:Primary_tics_or_tic ;
    skos:definition "Tourette syndrome is a chronic tic disorder characterised by the presence of both chronic motor tics and vocal (phonic) tics, with onset during the developmental period. Motor and vocal tics are defined as sudden, rapid, non-rhythmic, and recurrent movements or vocalizations, respectively. In order to be diagnosed as Tourette syndrome, both motor and vocal tics must have been present for at least one year, although they may not manifest concurrently or consistently throughout the symptomatic course."^^xsd:string ;
    skos:prefLabel "Tourette syndrome"^^xsd:string .

icd-kg:Unknown_or_unspecified_psychoactive_substance_dependence a owl:Class ;
    icd-schema:exclusion icd-kg:Harmful_pattern_of_unknown_or_unspecified_psychoactive_substance ;
    rdfs:subClassOf icd-kg:Unknown_or_unspecified_psychoactive_substances ;
    skos:definition "Unknown or unspecified psychoactive substance dependence is a disorder of regulation of use of an unknown or unspecified substance arising from repeated or continuous use of the substance. The characteristic feature is a strong internal drive to use the unknown or unspecified substance, which is manifested by impaired ability to control use, increasing priority given to use over other activities and persistence of use despite harm or negative consequences. These experiences are often accompanied by a subjective sensation of urge or craving to use the unknown or unspecified substance. The features of dependence are usually evident over a period of at least 12 months but the diagnosis may be made if use of the unknown or unspecified substance is continuous (daily or almost daily) for at least 3 months."^^xsd:string ;
    skos:prefLabel "Unknown or unspecified psychoactive substance dependence"^^xsd:string .

icd-kg:Volatile_inhalant_dependence a owl:Class ;
    icd-schema:exclusion icd-kg:Harmful_pattern_of_volatile_inhalants ;
    rdfs:subClassOf icd-kg:Volatile_inhalants ;
    skos:definition "Volatile inhalant dependence is a disorder of regulation of volatile inhalant use arising from repeated or continuous use of volatile inhalants. The characteristic feature is a strong internal drive to use volatile inhalants, which is manifested by impaired ability to control use, increasing priority given to use over other activities and persistence of use despite harm or negative consequences. These experiences are often accompanied by a subjective sensation of urge or craving to use volatile inhalants. Physiological features of dependence may also be present, including tolerance to the effects of volatile inhalants, withdrawal symptoms following cessation or reduction in use of volatile inhalants, or repeated use of volatile inhalants or pharmacologically similar substances to prevent or alleviate withdrawal symptoms. The features of dependence are usually evident over a period of at least 12 months but the diagnosis may be made if volatile inhalant use is continuous (daily or almost daily) for at least 3 months."^^xsd:string ;
    skos:prefLabel "Volatile inhalant dependence"^^xsd:string .

icd-kg:Addictive_behaviours a owl:Class ;
    icd-schema:exclusion icd-kg:Paraphilic ;
    rdfs:subClassOf icd-kg:Substance_use_or_addictive_behaviours ;
    skos:definition "Disorders due to addictive behaviours are recognizable and clinically significant syndromes associated with distress or interference with personal functions that develop as a result of repetitive rewarding behaviours other than the use of dependence-producing substances. Disorders due to addictive behaviours include gambling disorder and gaming disorder, which may involve both online and offline behaviour."^^xsd:string ;
    skos:prefLabel "Addictive behaviours"^^xsd:string .

icd-kg:Alcohol_dependence a owl:Class ;
    icd-schema:exclusion icd-kg:Harmful_pattern_of_alcohol ;
    icd-schema:inclusion "Chronic alcoholism"^^xsd:string,
        "Dipsomania"^^xsd:string ;
    rdfs:subClassOf icd-kg:Alcohol ;
    skos:definition "Alcohol dependence is a disorder of regulation of alcohol use arising from repeated or continuous use of alcohol. The characteristic feature is a strong internal drive to use alcohol, which is manifested by impaired ability to control use, increasing priority given to use over other activities and persistence of use despite harm or negative consequences. These experiences are often accompanied by a subjective sensation of urge or craving to use alcohol. Physiological features of dependence may also be present, including tolerance to the effects of alcohol, withdrawal symptoms following cessation or reduction in use of alcohol, or repeated use of alcohol or pharmacologically similar substances to prevent or alleviate withdrawal symptoms. The features of dependence are usually evident over a period of at least 12 months but the diagnosis may be made if alcohol use is continuous (daily or almost daily) for at least 3 months."^^xsd:string ;
    skos:prefLabel "Alcohol dependence"^^xsd:string .

icd-kg:Cocaine_dependence a owl:Class ;
    icd-schema:exclusion icd-kg:Harmful_pattern_of_cocaine ;
    rdfs:subClassOf icd-kg:Cocaine ;
    skos:definition "Cocaine dependence is a disorder of regulation of cocaine use arising from repeated or continuous use of cocaine. The characteristic feature is a strong internal drive to use cocaine, which is manifested by impaired ability to control use, increasing priority given to use over other activities and persistence of use despite harm or negative consequences. These experiences are often accompanied by a subjective sensation of urge or craving to use cocaine. Physiological features of dependence may also be present, including tolerance to the effects of cocaine, withdrawal symptoms following cessation or reduction in use of cocaine, or repeated use of cocaine or pharmacologically similar substances to prevent or alleviate withdrawal symptoms. The features of dependence are usually evident over a period of at least 12 months but the diagnosis may be made if cocaine use is continuous (daily or almost daily) for at least 3 months."^^xsd:string ;
    skos:prefLabel "Cocaine dependence"^^xsd:string .

icd-kg:Conductdissocial a owl:Class ;
    rdfs:subClassOf icd-kg:Disruptive_behaviour_or_dissocial ;
    skos:definition "Conduct-dissocial disorder is characterised by a repetitive and persistent pattern of behaviour in which the basic rights of others or major age-appropriate societal norms, rules, or laws are violated such as aggression towards people or animals; destruction of property; deceitfulness or theft; and serious violations of rules. The behaviour pattern is of sufficient severity to result in significant impairment in personal, family, social, educational, occupational or other important areas of functioning. To be diagnosed, the behaviour pattern must be enduring over a significant period of time (e.g., 12 months or more). Isolated dissocial or criminal acts are thus not in themselves grounds for the diagnosis."^^xsd:string ;
    skos:prefLabel "Conductdissocial"^^xsd:string .

icd-kg:Delirium_psychoactive_substances_including_medications a owl:Class ;
    rdfs:subClassOf icd-kg:Delirium ;
    skos:definition "All definitional requirements for delirium are met. There is evidence from history, physical examination, or laboratory findings that the delirium is caused by the direct physiological effects of a substance or medication (including withdrawal). If the specific substance inducing the delirium has been identified, it should be classified using the appropriate subcategory (e.g., alcohol-induced delirium)."^^xsd:string ;
    skos:prefLabel "Delirium psychoactive substances including medications"^^xsd:string .

icd-kg:Dementia_alzheimer_disease a owl:Class ;
    rdfs:subClassOf icd-kg:Dementia ;
    skos:definition "Dementia due to Alzheimer disease is the most common form of dementia. Onset is insidious with memory impairment typically reported as the initial presenting complaint. The characteristic course is a slow but steady decline from a previous level of cognitive functioning with impairment in additional cognitive domains (such as executive functions, attention, language, social cognition and judgment, psychomotor speed, visuoperceptual or visuospatial abilities) emerging with disease progression. Dementia due to Alzheimer disease may be accompanied by mental and behavioural symptoms such as depressed mood and apathy in the initial stages of the disease and may be accompanied by psychotic symptoms, irritability, aggression, confusion, abnormalities of gait and mobility, and seizures at later stages. Positive genetic testing, family history and gradual cognitive decline are suggestive of Dementia due to Alzheimer disease."^^xsd:string ;
    skos:prefLabel "Dementia alzheimer disease"^^xsd:string .

icd-kg:DiagnosticCriteria a owl:Class ;
    skos:definition "Any feature associated or not with a medical condition. In medicine a symptom is generally subjective while a sign is objective."^^xsd:string ;
    skos:prefLabel "Diagnostic Criteria"^^xsd:string .

icd-kg:Disruptive_behaviour_or_dissocial a owl:Class ;
    rdfs:subClassOf icd-kg:Mental_behavioural_or_neurodevelopmental_disorders ;
    skos:definition "Disruptive behaviour and dissocial disorders are characterised by persistent behaviour problems that range from markedly and persistently defiant, disobedient, provocative or spiteful (i.e., disruptive) behaviours to those that persistently violate the basic rights of others or major age-appropriate societal norms, rules, or laws (i.e., dissocial). Onset of Disruptive and dissocial disorders is commonly, though not always, during childhood."^^xsd:string ;
    skos:prefLabel "Disruptive behaviour or dissocial"^^xsd:string .

icd-kg:Ejaculatory_dysfunctions a owl:Class ;
    rdfs:subClassOf icd-kg:Sexual_dysfunctions ;
    skos:definition "Ejaculatory dysfunctions refer to difficulties with ejaculation in men, including ejaculatory latencies that are experienced as too short (Male early ejaculation) or too long (Male delayed ejaculation)."^^xsd:string ;
    skos:prefLabel "Ejaculatory dysfunctions"^^xsd:string .

icd-kg:Elimination a owl:Class ;
    rdfs:subClassOf icd-kg:Mental_behavioural_or_neurodevelopmental_disorders ;
    skos:definition "Elimination disorders include the repeated voiding of urine into clothes or bed (enuresis) and the repeated passage of faeces in inappropriate places (encopresis). Elimination disorders should only be diagnosed after the individual has reached a developmental age when continence is ordinarily expected (5 years for enuresis and 4 years for encopresis). The urinary or faecal incontinence may have been present from birth (i.e., an atypical extension of normal infantile incontinence), or may have arisen following a period of acquired bladder or bowel control. An Elimination disorder should not be diagnosed if the behaviour is fully attributable to another health condition that causes incontinence, congenital or acquired abnormalities of the urinary tract or bowel, or excessive use of laxatives or diuretics."^^xsd:string ;
    skos:prefLabel "Elimination"^^xsd:string .

icd-kg:Factitious a owl:Class ;
    icd-schema:exclusion <http://id.who.int/icd/entity/1136473465> ;
    rdfs:subClassOf icd-kg:Mental_behavioural_or_neurodevelopmental_disorders ;
    skos:definition "Factitious disorders are characterised by intentionally feigning, falsifying, inducing, or aggravating medical, psychological, or behavioural signs and symptoms or injury in oneself or in another person, most commonly a child dependent, associated with identified deception. A pre-existing disorder or disease may be present, but the individual intentionally aggravates existing symptoms or falsifies or induces additional symptoms. Individuals with factitious disorder seek treatment or otherwise present themselves or another person as ill, injured, or impaired based on the feigned, falsified, or self-induced signs, symptoms, or injuries. The deceptive behaviour is not solely motivated by obvious external rewards or incentives (e.g., obtaining disability payments or evading criminal prosecution). This is in contrast to Malingering, in which obvious external rewards or incentives motivate the behaviour."^^xsd:string ;
    skos:prefLabel "Factitious"^^xsd:string .

icd-kg:Frontotemporal_dementia a owl:Class ;
    rdfs:subClassOf icd-kg:Dementia ;
    skos:definition "Frontotemporal dementia (FTD) is a group of primary neurodegenerative disorders primarily affecting the frontal and temporal lobes. Onset is typically insidious with a gradual and worsening course. Several syndromic variants (some with an identified genetic basis or familiality) are described that include presentations with predominantly marked personality and behavioral changes (such as executive dysfunction, apathy, deterioration of social cognition, repetitive behaviours, and dietary changes), predominantly language deficits (that include semantic, agrammatic/nonfluent, and logopenic forms), predominantly movement-related deficits (progressive supranuclear palsy, corticobasal degeneration, multiple systems atrophy, or amyotrophic lateral sclerosis), or a combination of these deficits. Memory function often remains relatively intact, particularly during the early stages of the disorder."^^xsd:string ;
    skos:prefLabel "Frontotemporal dementia"^^xsd:string .

icd-kg:Harmful_pattern_of_alcohol a owl:Class ;
    icd-schema:exclusion icd-kg:Alcohol_dependence ;
    rdfs:subClassOf icd-kg:Alcohol ;
    skos:definition "A pattern of alcohol use that has caused damage to a person’s physical or mental health or has resulted in behaviour leading to harm to the health of others. The pattern of alcohol use is evident over a period of at least 12 months if substance use is episodic or at least one month if use is continuous. Harm to health of the individual occurs due to one or more of the following: (1) behaviour related to intoxication; (2) direct or secondary toxic effects on body organs and systems; or (3) a harmful route of administration. Harm to health of others includes any form of physical harm, including trauma, or mental disorder that is directly attributable to behaviour related to alcohol intoxication on the part of the person to whom the diagnosis of Harmful pattern of use of alcohol applies."^^xsd:string ;
    skos:prefLabel "Harmful pattern of alcohol"^^xsd:string .

icd-kg:Harmful_pattern_of_cocaine a owl:Class ;
    icd-schema:exclusion icd-kg:Cocaine_dependence ;
    rdfs:subClassOf icd-kg:Cocaine ;
    skos:definition "A pattern of use of cocaine that has caused damage to a person’s physical or mental health or has resulted in behaviour leading to harm to the health of others. The pattern of cocaine use is evident over a period of at least 12 months if substance use is episodic or at least one month if use is continuous (i.e., daily or almost daily). Harm to health of the individual occurs due to one or more of the following: (1) behaviour related to intoxication; (2) direct or secondary toxic effects on body organs and systems; or (3) a harmful route of administration. Harm to health of others includes any form of physical harm, including trauma, or mental disorder that is directly attributable to behaviour related to cocaine intoxication on the part of the person to whom the diagnosis of Harmful pattern of use of cocaine applies."^^xsd:string ;
    skos:prefLabel "Harmful pattern of cocaine"^^xsd:string .

icd-kg:Harmful_pattern_of_other_specified_psychoactive_substance a owl:Class ;
    icd-schema:exclusion icd-kg:Other_specified_psychoactive_substance_dependence ;
    rdfs:subClassOf icd-kg:Other_specified_psychoactive_substances_including_medications ;
    skos:definition "A pattern of use of a specified psychoactive substance or medication that is not included in the other substance classes specifically identified under Disorders Due to Substance Use that has caused damage to a person’s physical or mental health or has resulted in behaviour leading to harm to the health of others. The pattern of substance use is evident over a period of at least 12 months if use is episodic or at least one month if use is continuous (i.e., daily or almost daily). Harm to health of the individual occurs due to one or more of the following: (1) behaviour related to intoxication; (2) direct or secondary toxic effects on body organs and systems; or (3) a harmful route of administration. Harm to health of others includes any form of physical harm, including trauma, or mental disorder that is directly attributable to behaviour related to intoxication due to the specified substance or medication on the part of the person to whom the diagnosis of Harmful pattern of use of other specified psychoactive substance applies."^^xsd:string ;
    skos:prefLabel "Harmful pattern of other specified psychoactive substance"^^xsd:string .

icd-kg:Harmful_pattern_of_synthetic_cathinones a owl:Class ;
    icd-schema:exclusion icd-kg:Synthetic_cathinone_dependence ;
    rdfs:subClassOf icd-kg:Synthetic_cathinones ;
    skos:definition "A pattern of use of synthetic cathinones that has caused damage to a person’s physical or mental health or has resulted in behaviour leading to harm to the health of others. The pattern of synthetic cathinone use is evident over a period of at least 12 months if substance use is episodic or at least one month if use is continuous (i.e., daily or almost daily). Harm to health of the individual occurs due to one or more of the following: (1) behaviour related to intoxication; (2) direct or secondary toxic effects on body organs and systems; or (3) a harmful route of administration. Harm to health of others includes any form of physical harm, including trauma, or mental disorder that is directly attributable to behaviour related to synthetic cathinone intoxication on the part of the person to whom the diagnosis of Harmful pattern of use of synthetic cathinones applies."^^xsd:string ;
    skos:prefLabel "Harmful pattern of synthetic cathinones"^^xsd:string .

icd-kg:Hypochondriasis a owl:Class ;
    icd-schema:exclusion icd-kg:Bodily_distress,
        icd-kg:Body_dysmorphic,
        <http://id.who.int/icd/entity/1907420475> ;
    icd-schema:inclusion "Hypochondriacal neurosis"^^xsd:string,
        "Illness anxiety disorder"^^xsd:string ;
    rdfs:subClassOf icd-kg:Anxiety_or_fearrelated,
        icd-kg:Obsessivecompulsive_or_related ;
    skos:definition "Hypochondriasis is characterised by persistent preoccupation or fear about the possibility of having one or more serious, progressive or life-threatening illnesses. The preoccupation is accompanied by either: 1) repetitive and excessive health-related behaviours, such as repeatedly checking the body for evidence of illness, spending inordinate amounts of time searching for information about the feared illness, repeatedly seeking reassurance (e.g. arranging multiple medical consultations); or 2) maladaptive avoidance behaviour related to health (e.g. avoids medical appointments). The symptoms result in significant distress or significant impairment in personal, family, social, educational, occupational or other important areas of functioning."^^xsd:string ;
    skos:prefLabel "Hypochondriasis"^^xsd:string .

icd-kg:Language a owl:Class ;
    icd-schema:exclusion icd-kg:Autism_spectrum,
        <http://id.who.int/icd/entity/1296093776>,
        <http://id.who.int/icd/entity/947280473> ;
    rdfs:subClassOf icd-kg:Speech_or_language ;
    skos:definition "Developmental language disorder is characterised by persistent deficits in the acquisition, understanding, production or use of language (spoken or signed), that arise during the developmental period, typically during early childhood, and cause significant limitations in the individual’s ability to communicate. The individual’s ability to understand, produce or use language is markedly below what would be expected given the individual’s age. The language deficits are not explained by another neurodevelopmental disorder or a sensory impairment or neurological condition, including the effects of brain injury or infection."^^xsd:string ;
    skos:prefLabel "Language"^^xsd:string .

icd-kg:MedicalSignOrSymptom a owl:Class ;
    owl:equivalentClass schema:MedicalSignOrSymptom ;
    skos:definition "Any feature associated or not with a medical condition. In medicine a symptom is generally subjective while a sign is objective."^^xsd:string ;
    skos:prefLabel "Medical Sign Or Symptom"^^xsd:string .

icd-kg:Mild_neurocognitive a owl:Class ;
    rdfs:subClassOf icd-kg:Neurocognitive ;
    skos:definition "Mild neurocognitive disorder is characterized by mild impairment in one or more cognitive domains relative to that expected given the individual’s age and general premorbid level of cognitive functioning, which represents a decline from the individual’s previous level of functioning. Diagnosis is based on report from the patient, informant, or clinical observation, and is accompanied by objective evidence of impairment by quantified clinical assessment or standardized cognitive testing. Cognitive impairment is not severe enough to significantly interfere with an individual’s ability to perform activities related to personal, family, social, educational, and/or occupational functioning or other important functional areas. Cognitive impairment is not attributable to normal aging and may be static, progressive, or may resolve or improve depending on underlying cause or treatment. Cognitive impairment may be attributable to an underlying acquired disease of the nervous system, a trauma, an infection or other disease process affecting the brain, use of specific substances or medications, nutritional deficiency or exposure to toxins, or the etiology may be undetermined. The impairment is not due to current substance intoxication or withdrawal."^^xsd:string ;
    skos:prefLabel "Mild neurocognitive"^^xsd:string .

icd-kg:Nicotine a owl:Class ;
    rdfs:subClassOf icd-kg:Substance_use ;
    skos:definition "Disorders due to use of nicotine are characterised by the pattern and consequences of nicotine use. Nicotine is the active dependence-producing constituent of the tobacco plant, Nicotiana tabacum. Nicotine is used overwhelmingly through smoking cigarettes. Increasingly, it is also used in electronic cigarettes that vaporize nicotine dissolved in a carrier solvent for inhalation (i.e., “vaping”). Pipe smoking, chewing tobacco and inhaling snuff are minor forms of use. Nicotine is a highly potent addictive compound and is the third most common psychoactive substance used worldwide after caffeine and alcohol. Nicotine Dependence and Nicotine Withdrawal are well described and Nicotine-Induced Mental Disorders are recognized."^^xsd:string ;
    skos:prefLabel "Nicotine"^^xsd:string .

icd-kg:Nonamnestic_alzheimer_disease_dementia_subtypes a owl:Class ;
    rdfs:subClassOf icd-kg:Dementia_alzheimer_disease ;
    skos:definition "These are clinical variants of Alzheimer disease dementia, which predominantly manifest as non-amnestic syndromes in their early stages, particularly prominent language, visuospatial or dysexecutive/behavioural impairment."^^xsd:string ;
    skos:prefLabel "Nonamnestic alzheimer disease dementia subtypes"^^xsd:string .

icd-kg:Oppositional_defiant a owl:Class ;
    rdfs:subClassOf icd-kg:Disruptive_behaviour_or_dissocial ;
    skos:definition "Oppositional defiant disorder is a persistent pattern (e.g., 6 months or more) of markedly defiant, disobedient, provocative or spiteful behaviour that occurs more frequently than is typically observed in individuals of comparable age and developmental level and that is not restricted to interaction with siblings. Oppositional defiant disorder may be manifest in prevailing, persistent angry or irritable mood, often accompanied by severe temper outbursts or in headstrong, argumentative and defiant behaviour. The behaviour pattern is of sufficient severity to result in significant impairment in personal, family, social, educational, occupational or other important areas of functioning"^^xsd:string ;
    skos:prefLabel "Oppositional defiant"^^xsd:string .

icd-kg:Paraphilic a owl:Class ;
    icd-schema:inclusion "paraphilias"^^xsd:string ;
    rdfs:subClassOf icd-kg:Mental_behavioural_or_neurodevelopmental_disorders ;
    skos:definition "Paraphilic disorders are characterised by persistent and intense patterns of atypical sexual arousal, manifested by sexual thoughts, fantasies, urges, or behaviours, the focus of which involves others whose age or status renders them unwilling or unable to consent and on which the person has acted or by which he or she is markedly distressed. Paraphilic disorders may include arousal patterns involving solitary behaviours or consenting individuals only when these are associated with marked distress that is not simply a result of rejection or feared rejection of the arousal pattern by others or with significant risk of injury or death."^^xsd:string ;
    skos:prefLabel "Paraphilic"^^xsd:string .

icd-kg:Personality_and_related_traits a owl:Class ;
    rdfs:subClassOf icd-kg:Mental_behavioural_or_neurodevelopmental_disorders ;
    skos:prefLabel "Personality and related traits"^^xsd:string .

icd-kg:Primary_tics_or_tic a owl:Class ;
    rdfs:subClassOf icd-kg:Neurodevelopmental ;
    skos:definition "Primary tics or tic disorders are characterised by the presence of chronic motor and/or vocal (phonic) tics. Motor and vocal tics are defined as sudden, rapid, non-rhythmic, and recurrent movements or vocalizations, respectively. In order to be diagnosed, tics must have been present for at least one year, although they may not manifest consistently."^^xsd:string ;
    skos:prefLabel "Primary tics or tic"^^xsd:string .

icd-kg:Sexual_arousal_dysfunctions a owl:Class ;
    rdfs:subClassOf icd-kg:Sexual_dysfunctions ;
    skos:definition "Sexual arousal dysfunctions include difficulties with the physiological or the subjective aspects of sexual arousal."^^xsd:string ;
    skos:prefLabel "Sexual arousal dysfunctions"^^xsd:string .

icd-kg:Sleeprelated_movement a owl:Class ;
    rdfs:subClassOf icd-kg:Sleepwake ;
    skos:definition "Sleep related movement disorders are primarily characterised by relatively simple, usually stereotyped, movements that disturb sleep or its onset. An exception is Restless legs syndrome, which is primarily a waking, sensorimotor experience but is included in Sleep-related movement disorders because it almost always also involves periodic limb movements during sleep."^^xsd:string ;
    skos:prefLabel "Sleeprelated movement"^^xsd:string .

icd-kg:Substance_use_or_addictive_behaviours a owl:Class ;
    rdfs:subClassOf icd-kg:Mental_behavioural_or_neurodevelopmental_disorders ;
    skos:definition "Disorders due to substance use and addictive behaviours are mental and behavioural disorders that develop as a result of the use of predominantly psychoactive substances, including medications, or specific repetitive rewarding and reinforcing behaviours."^^xsd:string ;
    skos:prefLabel "Substance use or addictive behaviours"^^xsd:string .

icd-kg:Symptomatic_and_course_presentations_for_mood_episodes_in_mood a owl:Class ;
    rdfs:subClassOf icd-kg:Mood ;
    skos:definition "These categories may be applied to describe the presentation and characteristics of mood episodes in the context of single episode depressive disorder, recurrent depressive disorder, bipolar type I disorder, or bipolar type II disorder. These categories indicate the presence of specific, important features of the clinical presentation or of the course, onset, and pattern of mood episodes. These categories are not mutually exclusive, and as many may be added as apply."^^xsd:string ;
    skos:prefLabel "Symptomatic and course presentations for mood episodes in mood"^^xsd:string .

icd-kg:Synthetic_cathinone_dependence a owl:Class ;
    icd-schema:exclusion icd-kg:Harmful_pattern_of_synthetic_cathinones ;
    rdfs:subClassOf icd-kg:Synthetic_cathinones ;
    skos:definition "Synthetic cathinone dependence is a disorder of regulation of synthetic cathinone use arising from repeated or continuous use of synthetic cathinones. The characteristic feature is a strong internal drive to use synthetic cathinones, which is manifested by impaired ability to control use, increasing priority given to use over other activities and persistence of use despite harm or negative consequences. These experiences are often accompanied by a subjective sensation of urge or craving to use synthetic cathinones. Physiological features of dependence may also be present, including tolerance to the effects of synthetic cathinones, withdrawal symptoms following cessation or reduction in use of synthetic cathinones, or repeated use of synthetic cathinones or pharmacologically similar substances to prevent or alleviate withdrawal symptoms. The features of dependence are usually evident over a period of at least 12 months but the diagnosis may be made if synthetic cathinone use is continuous (daily or almost daily) for at least 3 months."^^xsd:string ;
    skos:prefLabel "Synthetic cathinone dependence"^^xsd:string .

icd-kg:Adjustment a owl:Class ;
    icd-schema:exclusion icd-kg:Recurrent_depressive,
        icd-kg:Separation_anxiety,
        icd-kg:Single_episode_depressive,
        <http://id.who.int/icd/entity/129180281>,
        <http://id.who.int/icd/entity/2009949293>,
        <http://id.who.int/icd/entity/505909942> ;
    rdfs:subClassOf icd-kg:Specifically_associated_with_stress ;
    skos:definition "Adjustment disorder is a maladaptive reaction to an identifiable psychosocial stressor or multiple stressors (e.g. divorce, illness or disability, socio-economic problems, conflicts at home or work) that usually emerges within a month of the stressor. The disorder is characterised by preoccupation with the stressor or its consequences, including excessive worry, recurrent and distressing thoughts about the stressor, or constant rumination about its implications, as well as by failure to adapt to the stressor that causes significant impairment in personal, family, social, educational, occupational or other important areas of functioning. The symptoms are not better explained by another mental disorder (e.g., Mood Disorder, another Disorder Specifically Associated with Stress) and typically resolve within 6 months, unless the stressor persists for a longer duration."^^xsd:string ;
    skos:prefLabel "Adjustment"^^xsd:string .

icd-kg:Anorexia_nervosa a owl:Class ;
    icd-schema:exclusion <http://id.who.int/icd/entity/2137507044> ;
    rdfs:subClassOf icd-kg:Feeding_or_eating ;
    skos:definition "Anorexia Nervosa is characterised by significantly low body weight for the individual’s height, age and developmental stage that is not due to another health condition or to the unavailability of food. A commonly used threshold is body mass index (BMI) less than 18.5 kg/m² in adults and BMI-for-age under 5th percentile in children and adolescents. Rapid weight loss (e.g. more than 20% of total body weight within 6 months) may replace the low body weight guideline as long as other diagnostic requirements are met. Children and adolescents may exhibit failure to gain weight as expected based on the individual developmental trajectory rather than weight loss. Low body weight is accompanied by a persistent pattern of behaviours to prevent restoration of normal weight, which may include behaviours aimed at reducing energy intake (restricted eating), purging behaviours (e.g. self-induced vomiting, misuse of laxatives), and behaviours aimed at increasing energy expenditure (e.g. excessive exercise), typically associated with a fear of weight gain. Low body weight or shape is central to the person's self-evaluation or is inaccurately perceived to be normal or even excessive."^^xsd:string ;
    skos:prefLabel "Anorexia nervosa"^^xsd:string .

icd-kg:Bodily_distress a owl:Class ;
    icd-schema:exclusion icd-kg:Body_dysmorphic,
        icd-kg:Dissociative,
        icd-kg:Excoriation,
        icd-kg:Gender_incongruence,
        icd-kg:Hypochondriasis,
        icd-kg:Sexual_dysfunctions,
        icd-kg:Tourette_syndrome,
        <http://id.who.int/icd/entity/1894671574>,
        <http://id.who.int/icd/entity/1932194482>,
        <http://id.who.int/icd/entity/569175314> ;
    rdfs:subClassOf icd-kg:Of_bodily_distress_or_bodily_experience ;
    skos:definition "Bodily distress disorder is characterised by the presence of bodily symptoms that are distressing to the individual and excessive attention directed toward the symptoms, which may be manifest by repeated contact with health care providers. If another health condition is causing or contributing to the symptoms, the degree of attention is clearly excessive in relation to its nature and progression. Excessive attention is not alleviated by appropriate clinical examination and investigations and appropriate reassurance. Bodily symptoms are persistent, being present on most days for at least several months. Typically, bodily distress disorder involves multiple bodily symptoms that may vary over time. Occasionally there is a single symptom—usually pain or fatigue—that is associated with the other features of the disorder. The symptoms and associated distress and preoccupation have at least some impact on the individual’s functioning (e.g. strain in relationships, less effective academic or occupational functioning, abandonment of specific leisure activities)."^^xsd:string ;
    skos:prefLabel "Bodily distress"^^xsd:string .

icd-kg:Body_dysmorphic a owl:Class ;
    icd-schema:exclusion icd-kg:Anorexia_nervosa,
        icd-kg:Bodily_distress,
        <http://id.who.int/icd/entity/1100199287> ;
    rdfs:subClassOf icd-kg:Obsessivecompulsive_or_related ;
    skos:definition "Body Dysmorphic Disorder is characterised by persistent preoccupation with one or more perceived defects or flaws in appearance that are either unnoticeable or only slightly noticeable to others. Individuals experience excessive self-consciousness, often with ideas of reference (i.e., the conviction that people are taking notice, judging, or talking about the perceived defect or flaw). In response to their preoccupation, individuals engage in repetitive and excessive behaviours that include repeated examination of the appearance or severity of the perceived defect or flaw, excessive attempts to camouflage or alter the perceived defect, or marked avoidance of social situations or triggers that increase distress about the perceived defect or flaw. The symptoms are sufficiently severe to result in significant distress or significant impairment in personal, family, social, educational, occupational or other important areas of functioning."^^xsd:string ;
    skos:prefLabel "Body dysmorphic"^^xsd:string .

icd-kg:Bodyfocused_repetitive_behaviour a owl:Class ;
    rdfs:subClassOf icd-kg:Impulse_control,
        icd-kg:Obsessivecompulsive_or_related ;
    skos:definition "Body focused repetitive behaviour disorders are characterised by recurrent and habitual actions directed at the integument (e.g. hair-pulling, skin-picking, lip-biting), typically accompanied by unsuccessful attempts to decrease or stop the behaviour involved, and which lead to dermatological sequelae (e.g., hair loss, skin lesions, lip abrasions). The behaviour may occur in brief episodes scattered throughout the day or in less frequent but more sustained periods. The symptoms result in significant distress or significant impairment in personal, family, social, educational, occupational or other important areas of functioning."^^xsd:string ;
    skos:prefLabel "Bodyfocused repetitive behaviour"^^xsd:string .

icd-kg:Depressive a owl:Class ;
    rdfs:subClassOf icd-kg:Mood ;
    skos:definition "Depressive disorders are characterised by depressive mood (e.g., sad, irritable, empty) or loss of pleasure accompanied by other cognitive, behavioural, or neurovegetative symptoms that significantly affect the individual’s ability to function. A depressive disorder should not be diagnosed in individuals who have ever experienced a manic, mixed or hypomanic episode, which would indicate the presence of a bipolar disorder."^^xsd:string ;
    skos:prefLabel "Depressive"^^xsd:string .

icd-kg:Dissociative_drugs_including_ketamine_and_phencyclidine_%5Bpcp%5D a owl:Class ;
    icd-schema:exclusion <http://id.who.int/icd/entity/1235812153> ;
    rdfs:subClassOf icd-kg:Substance_use ;
    skos:definition "Disorders due to use of dissociative drugs including ketamine and phencyclidine [PCP] are characterised by the pattern and consequences of dissociative drug use. Dissociative drugs include ketamine and phencyclidine (PCP) and their (comparatively rare) chemical analogues. Ketamine is an intravenous anaesthetic widely used in low- and middle-income countries, particularly in Africa, and in emergency situations. Ketamine is also undergoing evaluation for treatment of some mental disorders (e.g., treatment resistant Depressive Disorders). It is also a widespread drug of nonmedical use in many countries and may be taken by the oral or nasal routes or injected. It produces a sense of euphoria but depending on the dose, emergent hallucinations and dissociation are recognised as unpleasant side effects. Phencyclidine has a more restricted worldwide distribution and also has euphoric and dissociative effects. Its use may result in bizarre behaviour uncharacteristic for the individual, including self-harm. Dissociative Drug Dependence is described but a withdrawal syndrome is not recognized by most authorities. Several Dissociative Drug-Induced Mental Disorders are recognised."^^xsd:string ;
    skos:prefLabel "Dissociative drugs including ketamine and phencyclidine [pcp]"^^xsd:string .

icd-kg:Feeding_or_eating a owl:Class ;
    rdfs:subClassOf icd-kg:Mental_behavioural_or_neurodevelopmental_disorders ;
    skos:definition "Feeding and Eating Disorders involve abnormal eating or feeding behaviours that are not explained by another health condition and are not developmentally appropriate or culturally sanctioned. Feeding disorders involve behavioural disturbances that are not related to body weight and shape concerns, such as eating of non-edible substances or voluntary regurgitation of foods. Eating disorders involve abnormal eating behaviour and preoccupation with food as well as prominent body weight and shape concerns."^^xsd:string ;
    skos:prefLabel "Feeding or eating"^^xsd:string .

icd-kg:Hallucinogens a owl:Class ;
    rdfs:subClassOf icd-kg:Substance_use ;
    skos:definition "Disorders due to use of hallucinogens are characterised by the pattern and consequences of hallucinogen use. Several thousand compounds have hallucinogenic properties, many of which are found in plants (e.g., mescaline) and fungi (e.g., psilocybin) or are chemically synthesized (e.g., lysergic acid diethylamide [LSD]). These compounds have primarily hallucinogenic properties, but some may also be stimulants. Much of the morbidity associated with these compounds arises from the acute effects related to Hallucinogen Intoxication. Hallucinogen Dependence is rare and Hallucinogen Withdrawal is not described. Among the mental disorders related to hallucinogen use, Hallucinogen-Induced Psychotic Disorder is the most frequently seen, although worldwide it is still fairly uncommon."^^xsd:string ;
    skos:prefLabel "Hallucinogens"^^xsd:string .

icd-kg:Mdma_or_related_drugs_including_mda a owl:Class ;
    icd-schema:exclusion <http://id.who.int/icd/entity/113982884> ;
    rdfs:subClassOf icd-kg:Substance_use ;
    skos:definition "Disorders due to use of MDMA or related drugs, including MDA are characterised by the pattern and consequences of MDMA or related drug use. MDMA is methylene-dioxymethamphetamine and is a common drug of abuse in many countries especially among young people. It is predominantly available in tablet form known as ‘ecstasy’. Pharmacologically, MDMA has stimulant and empathogenic properties and these encourage its use among young people for social and other interactions. Considering its wide prevalence in many countries and among many sub-groups of young people, MDMA and Related Drug Dependence and MDMA and Related Drug Withdrawal are comparatively uncommon. Substance-Induced Mental Disorders may arise from its use. Several analogues of MDMA exist, including MDA (methylene-dioxyamphetamine)."^^xsd:string ;
    skos:prefLabel "Mdma or related drugs including mda"^^xsd:string .

icd-kg:Mental_or_behavioural_associated_with_pregnancy_childbirth_or_the_puerperium a owl:Class ;
    rdfs:subClassOf icd-kg:Mental_behavioural_or_neurodevelopmental_disorders ;
    skos:definition "Syndromes associated with pregnancy or the puerperium (commencing within about 6 weeks after delivery) that involve significant mental and behavioural features. If the symptoms meet the diagnostic requirements for a specific mental disorder, that diagnosis should also be assigned."^^xsd:string ;
    skos:prefLabel "Mental or behavioural associated with pregnancy childbirth or the puerperium"^^xsd:string .

icd-kg:Of_intellectual_development a owl:Class ;
    icd-schema:exclusion icd-kg:Dementia ;
    rdfs:subClassOf icd-kg:Neurodevelopmental ;
    skos:definition "Disorders of intellectual development are a group of etiologically diverse conditions originating during the developmental period characterised by significantly below average intellectual functioning and adaptive behaviour that are approximately two or more standard deviations below the mean (approximately less than the 2.3rd percentile), based on appropriately normed, individually administered standardized tests. Where appropriately normed and standardized tests are not available, diagnosis of disorders of intellectual development requires greater reliance on clinical judgment based on appropriate assessment of comparable behavioural indicators."^^xsd:string ;
    skos:prefLabel "Of intellectual development"^^xsd:string .

icd-kg:Parasomnia a owl:Class ;
    rdfs:subClassOf icd-kg:Sleepwake ;
    skos:definition "Parasomnias are problematic behavioural or physiological events that occur while falling asleep, during sleep, or upon arousal from sleep. Parasomnias may occur during non-rapid eye movement sleep (NREM), rapid eye movement sleep (REM), or during transitions to and from sleep. They encompass abnormal sleep related complex movements, behaviours, emotions, perceptions, dreams, and autonomic nervous system activity."^^xsd:string ;
    skos:prefLabel "Parasomnia"^^xsd:string .

icd-kg:Schizoaffective a owl:Class ;
    rdfs:subClassOf icd-kg:Schizophrenia_or_other_primary_psychotic ;
    skos:definition "Schizoaffective disorder is an episodic disorder in which the diagnostic requirements of schizophrenia and a manic, mixed, or moderate or severe depressive episode are met within the same episode of illness, either simultaneously or within a few days of each other. Prominent symptoms of schizophrenia (e.g. delusions, hallucinations, disorganisation in the form of thought, experiences of influence, passivity and control) are accompanied by typical symptoms of a moderate or severe depressive episode (e.g. depressed mood, loss of interest, reduced energy), a manic episode (e.g. an extreme mood state characterised by euphoria, irritability, or expansiveness; increased activity or a subjective experience of increased energy) or a mixed episode. Psychomotor disturbances, including catatonia, may be present. Symptoms must have persisted for at least one month. The symptoms are not a manifestation of another medical condition (e.g. a brain tumor) and are not due to the effect of a substance or medication on the central nervous system (e.g. corticosteroids), including withdrawal (e.g. alcohol withdrawal)."^^xsd:string ;
    skos:prefLabel "Schizoaffective"^^xsd:string .

icd-kg:Schizophrenia a owl:Class ;
    icd-schema:exclusion icd-kg:Acute_and_transient_psychotic ;
    rdfs:subClassOf icd-kg:Schizophrenia_or_other_primary_psychotic ;
    skos:definition "Schizophrenia is characterised by disturbances in multiple mental modalities, including thinking (e.g., delusions, disorganisation in the form of thought), perception (e.g., hallucinations), self-experience (e.g., the experience that one's feelings, impulses, thoughts, or behaviour are under the control of an external force), cognition (e.g., impaired attention, verbal memory, and social cognition), volition (e.g., loss of motivation), affect (e.g., blunted emotional expression), and behaviour (e.g., behaviour that appears bizarre or purposeless, unpredictable or inappropriate emotional responses that interfere with the organisation of behaviour). Psychomotor disturbances, including catatonia, may be present. Persistent delusions, persistent hallucinations, thought disorder, and experiences of influence, passivity, or control are considered core symptoms. Symptoms must have persisted for at least one month in order for a diagnosis of schizophrenia to be assigned. The symptoms are not a manifestation of another health condition (e.g., a brain tumour) and are not due to the effect of a substance or medication on the central nervous system (e.g., corticosteroids), including withdrawal (e.g., alcohol withdrawal)."^^xsd:string ;
    skos:prefLabel "Schizophrenia"^^xsd:string .

icd-kg:Sleeprelated_breathing a owl:Class ;
    icd-schema:exclusion <http://id.who.int/icd/entity/2076031939> ;
    rdfs:subClassOf icd-kg:Sleepwake ;
    skos:definition "Sleep related breathing disorders are characterised by abnormalities of respiration during sleep. In some of these disorders, respiration is also abnormal during wakefulness. The disorders are grouped into central sleep apnoeas, obstructive sleep apnoea, and sleep related hypoventilation or hypoxemia disorders."^^xsd:string ;
    skos:prefLabel "Sleeprelated breathing"^^xsd:string .

icd-kg:Specifically_associated_with_stress a owl:Class ;
    icd-schema:exclusion <http://id.who.int/icd/entity/129180281>,
        <http://id.who.int/icd/entity/505909942> ;
    rdfs:subClassOf icd-kg:Mental_behavioural_or_neurodevelopmental_disorders ;
    skos:definition "Disorders specifically associated with stress are directly related to exposure to a stressful or traumatic event, or a series of such events or adverse experiences. For each of the disorders in this grouping, an identifiable stressor is a necessary, though not sufficient, causal factor. Although not all individuals exposed to an identified stressor will develop a disorder, the disorders in this grouping would not have occurred without experiencing the stressor. Stressful events for some disorders in this grouping are within the normal range of life experiences (e.g., divorce, socio-economic problems, bereavement). Other disorders require the experience of a stressor of an extremely threatening or horrific nature (i.e., potentially traumatic events). With all disorders in this grouping, it is the nature, pattern, and duration of the symptoms that arise in response to the stressful events—together with associated functional impairment—that distinguishes the disorders."^^xsd:string ;
    skos:prefLabel "Specifically associated with stress"^^xsd:string .

icd-kg:Speech_fluency a owl:Class ;
    icd-schema:exclusion <http://id.who.int/icd/entity/1894671574> ;
    rdfs:subClassOf icd-kg:Speech_or_language ;
    skos:definition "Developmental speech fluency disorder is characterised by frequent or pervasive disruption of the normal rhythmic flow and rate of speech characterised by repetitions and prolongations in sounds, syllables, words, and phrases, as well as blocking and word avoidance or substitutions. The speech dysfluency is persistent over time. The onset of speech dysfluency occurs during the developmental period and speech fluency is markedly below what would be expected for age. Speech dysfluency results in significant impairment in social communication, personal, family, social, educational, occupational or other important areas of functioning. The speech dysfluency is not better accounted for by a Disorder of Intellectual Development, a Disease of the Nervous System, a sensory impairment, or a structural abnormality, or other speech or voice disorder."^^xsd:string ;
    skos:prefLabel "Speech fluency"^^xsd:string .

icd-kg:Speech_or_language a owl:Class ;
    rdfs:subClassOf icd-kg:Neurodevelopmental ;
    skos:definition "Developmental speech or language disorders arise during the developmental period and are characterised by difficulties in understanding or producing speech and language or in using language in context for the purposes of communication that are outside the limits of normal variation expected for age and level of intellectual functioning. The observed speech and language problems are not attributable to regional, social, or cultural/ethnic language variations and are not fully explained by anatomical or neurological abnormalities. The presumptive aetiology for Developmental speech or language disorders is complex, and in many individual cases, is unknown."^^xsd:string ;
    skos:prefLabel "Speech or language"^^xsd:string .

icd-kg:Stereotyped_movement a owl:Class ;
    icd-schema:exclusion <http://id.who.int/icd/entity/1894671574>,
        <http://id.who.int/icd/entity/682424259> ;
    rdfs:subClassOf icd-kg:Neurodevelopmental ;
    skos:definition "Stereotyped movement disorder is characterised by the persistent (e.g., lasting several months) presence of voluntary, repetitive, stereotyped, apparently purposeless (and often rhythmic) movements that arise during the early developmental period, are not caused by the direct physiological effects of a substance or medication (including withdrawal), and markedly interfere with normal activities or result in self-inflicted bodily injury. Stereotyped movements that are non-injurious can include body rocking, head rocking, finger-flicking mannerisms, and hand flapping. Stereotyped self-injurious behaviours can include repetitive head banging, face slapping, eye poking, and biting of the hands, lips, or other body parts."^^xsd:string ;
    skos:prefLabel "Stereotyped movement"^^xsd:string .

icd-kg:Volatile_inhalants a owl:Class ;
    rdfs:subClassOf icd-kg:Substance_use ;
    skos:definition "Disorders due to use of volatile inhalants are characterised by the pattern and consequences of volatile inhalant use. Volatile inhalants include a range of compounds that are in the gaseous or vapour phase at ambient temperatures and include various organic solvents, glues, gasoline (petrol), nitrites and gases such as nitrous oxide, trichloroethane, butane, toluene, fluorocarbons, ether and halothane. They have a range of pharmacological properties but are predominantly central nervous system depressants, with many also having vasoactive effects. They tend to be used by younger persons and may be used when access to alternative psychoactive substances is difficult or impossible. Volatile Inhalant Intoxication is well recognized. Volatile inhalants have dependence-producing properties and Volatile Inhalant Dependence and Volatile Inhalant Withdrawal is recognized although comparatively uncommon worldwide. Volatile Inhalant-Induced Mental Disorders are described. They may also cause neurocognitive impairment, including Dementia."^^xsd:string ;
    skos:prefLabel "Volatile inhalants"^^xsd:string .

icd-kg:Acute_and_transient_psychotic a owl:Class ;
    rdfs:subClassOf icd-kg:Schizophrenia_or_other_primary_psychotic ;
    skos:definition "Acute and transient psychotic disorder is characterised by acute onset of psychotic symptoms that emerge without a prodrome and reach their maximal severity within two weeks. Symptoms may include delusions, hallucinations, disorganisation of thought processes, perplexity or confusion, and disturbances of affect and mood. Catatonia-like psychomotor disturbances may be present. Symptoms typically change rapidly, both in nature and intensity, from day to day, or even within a single day. The duration of the episode does not exceed 3 months, and most commonly lasts from a few days to 1 month. The symptoms are not a manifestation of another medical condition (e.g. a brain tumour) and are not due to the effect of a substance or medication on the central nervous system (e.g. corticosteroids), including withdrawal (e.g. alcohol withdrawal)."^^xsd:string ;
    skos:prefLabel "Acute and transient psychotic"^^xsd:string .

icd-kg:Cannabis a owl:Class ;
    icd-schema:exclusion icd-kg:Synthetic_cannabinoids,
        <http://id.who.int/icd/entity/1389430127> ;
    rdfs:subClassOf icd-kg:Substance_use ;
    skos:definition "Disorders due to use of cannabis are characterised by the pattern and consequences of cannabis use. Cannabis is the collective term for a range of psychoactive preparations of the cannabis plant, Cannabis sativa, and related species and hybrids. Cannabis contains cannabinoids, a class of diverse chemical compounds that act on endogenous cannabinoid receptors that modulate neurotransmitter release in the brain. The principal psychoactive cannabinoid is δ-9-tetrahydrocannabinol (THC). Cannabis is typically smoked in the form of the flowering heads or leaves of the Cannabis plant; tobacco is often mixed with cannabis when smoked. There are also cannabis oils that are prepared from these same sources. These preparations vary considerably in their THC potency. Cannabis has predominantly central nervous system depressant effects and produces a characteristic euphoria that may be part of the presenting features of Cannabis Intoxication, which may also include impairment in cognitive and psychomotor functioning. Cannabis has dependence-producing properties resulting in Cannabis Dependence in some people and Cannabis Withdrawal when use is reduced or discontinued. Cannabis is associated with a range of Cannabis-Induced Mental Disorders."^^xsd:string ;
    skos:prefLabel "Cannabis"^^xsd:string .

icd-kg:Dissociative a owl:Class ;
    rdfs:subClassOf icd-kg:Mental_behavioural_or_neurodevelopmental_disorders ;
    skos:definition "Dissociative disorders are characterised by involuntary disruption or discontinuity in the normal integration of one or more of the following: identity, sensations, perceptions, affects, thoughts, memories, control over bodily movements, or behaviour. Disruption or discontinuity may be complete, but is more commonly partial, and can vary from day to day or even from hour to hour. The symptoms of dissociative disorders are not due to the direct effects of a medication or substance, including withdrawal effects, are not better explained by another Mental, behavioural, or neurodevelopmental disorder, a Sleep-wake disorder, a Disease of the nervous system or other health condition, and are not part of an accepted cultural, religious, or spiritual practice. Dissociative symptoms in dissociative disorders are sufficiently severe to result in significant impairment in personal, family, social, educational, occupational or other important areas of functioning."^^xsd:string ;
    skos:prefLabel "Dissociative"^^xsd:string .

icd-kg:Dissociative_neurological_symptom a owl:Class ;
    icd-schema:exclusion icd-kg:Factitious ;
    rdfs:subClassOf icd-kg:Dissociative ;
    skos:definition "Dissociative neurological symptom disorder is characterised by the presentation of motor, sensory, or cognitive symptoms that imply an involuntary discontinuity in the normal integration of motor, sensory, or cognitive functions and are not consistent with a recognised disease of the nervous system, other mental or behavioural disorder, or other medical condition. The symptoms do not occur exclusively during another dissociative disorder and are not due to the effects of a substance or medication on the central nervous system, including withdrawal effects, or a Sleep-Wake disorder."^^xsd:string ;
    skos:prefLabel "Dissociative neurological symptom"^^xsd:string .

icd-kg:Impulse_control a owl:Class ;
    rdfs:subClassOf icd-kg:Mental_behavioural_or_neurodevelopmental_disorders ;
    skos:definition "Impulse control disorders are characterised by the repeated failure to resist an impulse, drive, or urge to perform an act that is rewarding to the person, at least in the short-term, despite consequences such as longer-term harm either to the individual or to others, marked distress about the behaviour pattern, or significant impairment in personal, family, social, educational, occupational, or other important areas of functioning. Impulse Control Disorders involve a range of specific behaviours, including fire-setting, stealing, sexual behaviour, and explosive outbursts."^^xsd:string ;
    skos:prefLabel "Impulse control"^^xsd:string .

icd-kg:Other_specified_psychoactive_substances_including_medications a owl:Class ;
    rdfs:subClassOf icd-kg:Substance_use ;
    skos:definition "Disorders due to use of other specified psychoactive substances, including medications are characterised by the pattern and consequences of psychoactive substances that are not included among the major substance classes specifically identified. Examples include khat, antidepressants, medications with anticholinergic properties (e.g., benztropine), and some antihistamines."^^xsd:string ;
    skos:prefLabel "Other specified psychoactive substances including medications"^^xsd:string .

icd-kg:Substanceinduced_psychotic a owl:Class ;
    rdfs:subClassOf icd-kg:Schizophrenia_or_other_primary_psychotic ;
    skos:prefLabel "Substanceinduced psychotic"^^xsd:string .

icd-kg:Synthetic_cannabinoids a owl:Class ;
    icd-schema:exclusion icd-kg:Cannabis ;
    rdfs:subClassOf icd-kg:Substance_use ;
    skos:definition "Disorders due to use of synthetic cannabinoids are characterised by the pattern and consequences of synthetic cannabinoid use. Synthetic cannabinoids are synthesized diverse chemical compounds that are potent agonists for endogenous cannabinoid receptors. There are several hundred such compounds. The synthetic compound is typically sprayed onto a vehicle such as cannabis or tea leaves and then smoked. The effect of these compounds is distinctly different from smoking naturally cultivated cannabis in that the euphoric effects are typically accompanied or dominated by psychotic-like symptoms (e.g., paranoia, hallucinations, and disorganized behavior). Synthetic Cannabinoid Intoxication may therefore present more frequently with psychotic symptoms in addition to the more typical effects of cannabis. Synthetic cannabinoids are also dependence-producing and Synthetic Cannabinoid Dependence and Synthetic Cannabinoid Withdrawal are recognized. Synthetic Cannabinoid-Induced Mental Disorders also occur; in particular Synthetic Cannabinoid-Induced Psychotic Disorder is recognized."^^xsd:string ;
    skos:prefLabel "Synthetic cannabinoids"^^xsd:string .

icd-kg:Unknown_or_unspecified_psychoactive_substances a owl:Class ;
    rdfs:subClassOf icd-kg:Substance_use ;
    skos:definition "Disorders due to use of unknown or unspecified psychoactive substances are characterised by the pattern and consequences of psychoactive substance use when the specific substance is unknown or unspecified. These categories may be used in clinical situations in which it is clear that the disturbance is due to substance use but the specific class of substance is unknown. Once the relevant substance is identified, the disturbance should be recoded under the appropriate substance class."^^xsd:string ;
    skos:prefLabel "Unknown or unspecified psychoactive substances"^^xsd:string .

icd-kg:Bipolar_or_related a owl:Class ;
    rdfs:subClassOf icd-kg:Mood ;
    skos:definition "Bipolar and related disorders are episodic mood disorders defined by the occurrence of Manic, Mixed or Hypomanic episodes or symptoms. These episodes typically alternate over the course of these disorders with Depressive episodes or periods of depressive symptoms."^^xsd:string ;
    skos:prefLabel "Bipolar or related"^^xsd:string .

icd-kg:Caffeine a owl:Class ;
    icd-schema:exclusion icd-kg:Stimulants_including_amphetamines_methamphetamine_or_methcathinone,
        <http://id.who.int/icd/entity/656164398> ;
    rdfs:subClassOf icd-kg:Substance_use ;
    skos:definition "Disorders due to use of caffeine are characterised by the pattern and consequences of caffeine use. Caffeine is a mild psychostimulant and diuretic that is found in the beans of the coffee plant (Coffea species) and is a constituent of coffee, cola drinks, chocolate, a range of proprietary 'energy drinks' and weight-loss aids. It is the most commonly used psychoactive substance worldwide and several clinical conditions related to its use are described, although severe disorders are comparatively rare considering its ubiquity. Caffeine Intoxication related to consumption of relatively higher doses (i.e., > 1 g per day) is described. Caffeine Withdrawal is common upon cessation of use among individuals who have used caffeine for a prolonged period or in large amounts. Caffeine-Induced Anxiety Disorder has been described, often following intoxication or heavy use."^^xsd:string ;
    skos:prefLabel "Caffeine"^^xsd:string .

icd-kg:Cocaine a owl:Class ;
    icd-schema:exclusion icd-kg:Stimulants_including_amphetamines_methamphetamine_or_methcathinone,
        <http://id.who.int/icd/entity/1385385359> ;
    rdfs:subClassOf icd-kg:Substance_use ;
    skos:definition "Disorders due to use of cocaine are characterised by the pattern and consequences of cocaine use. Cocaine is a compound found in the leaves of the coca plant, Erythroxylum coca, which is indigenous to countries in northern regions of South America. Cocaine has a limited place in medical treatment as an anaesthetic and vasoconstrictive agent. It is commonly used illicitly and widely available across the world, where it is found in two main forms: cocaine hydrochloride and cocaine freebase (also known as ‘crack’). Cocaine is a central nervous system stimulant, and Cocaine Intoxication typically includes a state of euphoria and hyperactivity. Cocaine has potent dependence-producing properties and Cocaine Dependence is a common cause of morbidity and of clinical presentations. Cocaine Withdrawal has a characteristic course that includes lethargy and depressed mood. A range of Cocaine-Induced Mental Disorders is described."^^xsd:string ;
    skos:prefLabel "Cocaine"^^xsd:string .

icd-kg:Delirium a owl:Class ;
    rdfs:subClassOf icd-kg:Neurocognitive,
        icd-kg:Secondary_neurocognitive_syndrome ;
    skos:definition "Delirium is characterized by a disturbance of attention, orientation, and awareness that develops within a short period of time, typically presenting as significant confusion or global neurocognitive impairment, with transient symptoms that may fluctuate depending on the underlying causal condition or etiology. Delirium often includes disturbance of behaviour and emotion, and may include impairment in multiple cognitive domains. A disturbance of the sleep-wake cycle, including reduced arousal of acute onset or total sleep loss with reversal of the sleep-wake cycle, may also be present. Delirium may be caused by the direct physiological effects of a medical condition not classified under mental, behavioural or neurodevelopmental disorders, by the direct physiological effects of a substance or medication, including withdrawal, or by multiple or unknown etiological factors."^^xsd:string ;
    skos:prefLabel "Delirium"^^xsd:string .

icd-kg:Multiple_specified_psychoactive_substances_including_medications a owl:Class ;
    rdfs:subClassOf icd-kg:Substance_use ;
    skos:definition "Disorders due to use of multiple specified psychoactive substances, including medications are characterised by the pattern and consequences of multiple psychoactive substances. Although this grouping is provided for coding purposes, in most clinical situations it is recommended that multiple specific disorders due to substance use be assigned rather than using categories from this grouping."^^xsd:string ;
    skos:prefLabel "Multiple specified psychoactive substances including medications"^^xsd:string .

icd-kg:Neurocognitive a owl:Class ;
    icd-schema:exclusion icd-kg:Neurodevelopmental ;
    rdfs:subClassOf icd-kg:Mental_behavioural_or_neurodevelopmental_disorders ;
    skos:definition "Neurocognitive disorders are characterised by primary clinical deficits in cognitive functioning that are acquired rather than developmental. That is, neurocognitive disorders do not include disorders characterised by deficits in cognitive function that are present from birth or that typically arise during the developmental period, which are classified in the grouping neurodevelopmental disorders. Rather, neurocognitive disorders represent a decline from a previously attained level of functioning. Although cognitive deficits are present in many mental disorders (e.g., schizophrenia, bipolar disorders), only disorders whose core features are cognitive are included in the neurocognitive disorders grouping. In cases where the underlying pathology and aetiology for neurocognitive disorders can be determined, the identified etiology should be classified separately."^^xsd:string ;
    skos:prefLabel "Neurocognitive"^^xsd:string .

icd-kg:Secondary_mental_or_behavioural_syndromes_associated_with_or_diseases_classified_elsewhere a owl:Class ;
    icd-schema:exclusion icd-kg:Bodily_distress,
        <http://id.who.int/icd/entity/1404135736>,
        <http://id.who.int/icd/entity/1581976053> ;
    rdfs:subClassOf icd-kg:Mental_behavioural_or_neurodevelopmental_disorders ;
    skos:definition "This grouping includes syndromes characterised by the presence of prominent psychological or behavioural symptoms judged to be direct pathophysiological consequences of a medical condition not classified under mental and behavioural disorders, based on evidence from the history, physical examination, or laboratory findings. The symptoms are not accounted for by delirium or by another mental and behavioural disorder, and are not a psychologically mediated response to a severe medical condition (e.g., adjustment disorder or anxiety symptoms in response to being diagnosed with a life-threatening illness). These categories should be used in addition to the diagnosis for the presumed underlying disorder or disease when the psychological and behavioural symptoms are sufficiently severe to warrant specific clinical attention."^^xsd:string ;
    skos:prefLabel "Secondary mental or behavioural syndromes associated with or diseases classified elsewhere"^^xsd:string .

icd-kg:Synthetic_cathinones a owl:Class ;
    rdfs:subClassOf icd-kg:Substance_use ;
    skos:definition "Disorders due to use of synthetic cathinones are characterised by the pattern and consequences of synthetic cathinone use. Synthetic cathinones (also known as ‘bath salts’) are synthetic compounds with stimulant properties related to cathinone found in the khat plant, Catha edulis. The use of synthetic cathinones is common in young populations in many countries. They may produce a range of disorders including Synthetic Cathinone Intoxication, Synthetic Cathinone Dependence and Synthetic Cathinone Withdrawal. Several synthetic cathinone-induced mental disorders are recognised."^^xsd:string ;
    skos:prefLabel "Synthetic cathinones"^^xsd:string .

icd-kg:Alcohol a owl:Class ;
    icd-schema:exclusion <http://id.who.int/icd/entity/499098434> ;
    rdfs:subClassOf icd-kg:Substance_use ;
    skos:definition "Disorders due to use of alcohol are characterised by the pattern and consequences of alcohol use. Alcohol—more specifically termed ethyl alcohol or ethanol—is an intoxicating compound produced by fermentation of sugars usually in agricultural products such as fruits, cereals, and vegetables with or without subsequent distillation. There are a wide variety of alcoholic drinks, with alcohol concentrations typically ranging from 1.5% to 60%. Alcohol is predominantly a central nervous system depressant. In addition to ability to produce Alcohol Intoxication, alcohol has dependence-producing properties, resulting in Alcohol Dependence in some people and Alcohol Withdrawal when alcohol use is reduced or discontinued. Unlike most other substances, elimination of alcohol from the body occurs at a constant rate, such that its clearance follows a linear rather than a logarithmic course. Alcohol is implicated in a wide range of harms affecting most organs and systems of the body (e.g., cirrhosis of the liver, gastrointestinal cancers, pancreatitis). Harm to others resulting from behaviour during Alcohol Intoxication is well recognized and is included in the definitions of harmful use of alcohol (i.e., Episode of Harmful Use of Alcohol and Harmful Pattern of Use of Alcohol). Several alcohol-induced mental disorders (e.g., Alcohol-Induced Psychotic Disorder) and alcohol-related forms of neurocognitive impairment (e.g., Dementia Due to Use of Alcohol) are recognized."^^xsd:string ;
    skos:prefLabel "Alcohol"^^xsd:string .

icd-kg:Anxiety_or_fearrelated a owl:Class ;
    rdfs:subClassOf icd-kg:Mental_behavioural_or_neurodevelopmental_disorders ;
    skos:definition "Anxiety and fear-related disorders are characterised by excessive fear and anxiety and related behavioural disturbances, with symptoms that are severe enough to result in significant distress or significant impairment in personal, family, social, educational, occupational, or other important areas of functioning. Fear and anxiety are closely related phenomena; fear represents a reaction to perceived imminent threat in the present, whereas anxiety is more future-oriented, referring to perceived anticipated threat. A key differentiating feature among the Anxiety and fear-related disorders are disorder-specific foci of apprehension, that is, the stimulus or situation that triggers the fear or anxiety. The clinical presentation of Anxiety and fear-related disorders typically includes specific associated cognitions that can assist in differentiating among the disorders by clarifying the focus of apprehension."^^xsd:string ;
    skos:prefLabel "Anxiety or fearrelated"^^xsd:string .

icd-kg:Opioids a owl:Class ;
    icd-schema:exclusion <http://id.who.int/icd/entity/603861372> ;
    rdfs:subClassOf icd-kg:Substance_use ;
    skos:definition "Disorders due to use of opioids are characterised by the pattern and consequences of opioid use. Opioids is a generic term that encompasses the constituents or derivatives of the opium poppy Papaver somniferum as well as a range of synthetic and semisynthetic compounds, some related to morphine and others chemically distinct but all having their primary actions on the µ opioid receptor. Examples of opioids include morphine, diacetylmorphine (heroin), fentanyl, pethidine, oxycodone, hydromorphone, methadone, buprenorphine, codeine and d-propoxyphene. The opioids all have analgesic properties of different potencies and are primarily central nervous system depressants. They suppress respiration as well as other vital functions and are a common cause of overdose and related deaths. Certain opioids are used or administered parenterally, including heroin, a common and potent opioid that is primarily used non-medically. Therapeutic opioids are prescribed for a range of indications worldwide, and are essential for pain management in cancer pain and palliative care, although they are also used for non-therapeutic reasons. In some countries morbidity and mortality related to therapeutic opioids is greater than that related to heroin. All opioids may result in Opioid Intoxication, Opioid Dependence and Opioid Withdrawal. A range of Opioid-Induced Disorders occur, some of which occur following Opioid Withdrawal."^^xsd:string ;
    skos:prefLabel "Opioids"^^xsd:string .

icd-kg:Sedatives_hypnotics_or_anxiolytics a owl:Class ;
    icd-schema:exclusion <http://id.who.int/icd/entity/756014816> ;
    rdfs:subClassOf icd-kg:Substance_use ;
    skos:definition "Disorders due to use of sedatives, hypnotics or anxiolytics are characterised by the pattern and consequences of use of these substances. Sedatives, hypnotics, and anxiolytics are typically prescribed for the short-term treatment of anxiety or insomnia and are also employed to provide sedation for medical procedures. They include the benzodiazepines and the non-benzodiazepine positive allosteric modulators of GABA receptors (i.e., ‘Z-drugs’) as well as many other compounds. Sedatives, hypnotics, and anxiolytics include barbiturates, which are available much less commonly now than in previous decades. Sedatives, hypnotics, and anxiolytics have dependence-inducing properties that are related to the dose and duration of their use. They may cause intoxication, dependence and withdrawal. Several other mental disorders induced by sedatives, hypnotics, or anxiolytics are recognized."^^xsd:string ;
    skos:prefLabel "Sedatives hypnotics or anxiolytics"^^xsd:string .

icd-kg:Sexual_dysfunctions a owl:Class ;
    rdfs:subClassOf icd-kg:Mental_behavioural_or_neurodevelopmental_disorders ;
    skos:definition "Sexual Dysfunctions are syndromes that comprise the various ways in which adult people may have difficulty experiencing personally satisfying, non-coercive sexual activities. Sexual response is a complex interaction of psychological, interpersonal, social, cultural and physiological processes and one or more of these factors may affect any stage of the sexual response. In order to be considered a sexual dysfunction, the dysfunction must: 1) occur frequently, although it may be absent on some occasions; 2) have been present for at least several months; and 3) be associated with clinically significant distress."^^xsd:string ;
    skos:prefLabel "Sexual dysfunctions"^^xsd:string .

icd-kg:Sleepwake a owl:Class ;
    rdfs:subClassOf icd-kg:Mental_behavioural_or_neurodevelopmental_disorders ;
    skos:definition "Sleep-wake disorders are characterised by difficulty initiating or maintaining sleep (insomnia disorders), excessive sleepiness (hypersomnolence disorders), respiratory disturbance during sleep (sleep-related breathing disorders), disorders of the sleep-wake schedule (circadian rhythm sleep-wake disorders), abnormal movements during sleep (sleep-related movement disorders), or problematic behavioural or physiological events that occur while falling asleep, during sleep, or upon arousal from sleep (parasomnia disorders)."^^xsd:string ;
    skos:prefLabel "Sleepwake"^^xsd:string .

icd-kg:Mood a owl:Class ;
    rdfs:subClassOf icd-kg:Mental_behavioural_or_neurodevelopmental_disorders ;
    skos:definition "Mood Disorders refers to a superordinate grouping of Bipolar and Depressive Disorders. Mood disorders are defined according to particular types of mood episodes and their pattern over time. The primary types of mood episodes are Depressive episode, Manic episode, Mixed episode, and Hypomanic episode. Mood episodes are not independently diagnosable entities, and therefore do not have their own diagnostic codes. Rather, mood episodes make up the primary components of most of the Depressive and Bipolar Disorders."^^xsd:string ;
    skos:prefLabel "Mood"^^xsd:string .

icd-kg:Personality a owl:Class ;
    rdfs:subClassOf icd-kg:Personality_and_related_traits ;
    skos:definition "Personality disorder is characterised by problems in functioning of aspects of the self (e.g., identity, self-worth, accuracy of self-view, self-direction), and/or interpersonal dysfunction (e.g., ability to develop and maintain close and mutually satisfying relationships, ability to understand others’ perspectives and to manage conflict in relationships) that have persisted over an extended period of time (e.g., 2 years or more). The disturbance is manifest in patterns of cognition, emotional experience, emotional expression, and behaviour that are maladaptive (e.g., inflexible or poorly regulated) and is manifest across a range of personal and social situations (i.e., is not limited to specific relationships or social roles). The patterns of behaviour characterizing the disturbance are not developmentally appropriate and cannot be explained primarily by social or cultural factors, including socio-political conflict. The disturbance is associated with substantial distress or significant impairment in personal, family, social, educational, occupational or other important areas of functioning."^^xsd:string ;
    skos:prefLabel "Personality"^^xsd:string .

icd-kg:Recurrent_depressive a owl:Class ;
    icd-schema:exclusion icd-kg:Adjustment,
        icd-kg:Bipolar_or_related,
        icd-kg:Single_episode_depressive ;
    icd-schema:inclusion "seasonal depressive disorder"^^xsd:string ;
    rdfs:subClassOf icd-kg:Depressive ;
    skos:definition "Recurrent depressive disorder is characterised by a history of at least two depressive episodes separated by at least several months without significant mood disturbance. A depressive episode is characterised by a period of depressed mood or diminished interest in activities occurring most of the day, nearly every day during a period lasting at least two weeks accompanied by other symptoms such as difficulty concentrating, feelings of worthlessness or excessive or inappropriate guilt, hopelessness, recurrent thoughts of death or suicide, changes in appetite or sleep, psychomotor agitation or retardation, and reduced energy or fatigue. There have never been any prior manic, hypomanic, or mixed episodes, which would indicate the presence of a Bipolar disorder."^^xsd:string ;
    skos:prefLabel "Recurrent depressive"^^xsd:string .

icd-kg:Schizophrenia_or_other_primary_psychotic a owl:Class ;
    rdfs:subClassOf icd-kg:Mental_behavioural_or_neurodevelopmental_disorders ;
    skos:definition "Schizophrenia and other primary psychotic disorders are characterised by significant impairments in reality testing and alterations in behaviour manifest in positive symptoms such as persistent delusions, persistent hallucinations, disorganised thinking (typically manifest as disorganised speech), grossly disorganised behaviour, and experiences of passivity and control, negative symptoms such as blunted or flat affect and avolition, and psychomotor disturbances. The symptoms occur with sufficient frequency and intensity to deviate from expected cultural or subcultural norms. These symptoms do not arise as a feature of another mental and behavioural disorder (e.g., a mood disorder, delirium, or a disorder due to substance use). The categories in this grouping should not be used to classify the expression of ideas, beliefs, or behaviours that are culturally sanctioned."^^xsd:string ;
    skos:prefLabel "Schizophrenia or other primary psychotic"^^xsd:string .

icd-kg:Single_episode_depressive a owl:Class ;
    icd-schema:exclusion icd-kg:Adjustment,
        icd-kg:Bipolar_or_related,
        icd-kg:Recurrent_depressive ;
    rdfs:subClassOf icd-kg:Depressive ;
    skos:definition "Single episode depressive disorder is characterised by the presence or history of one depressive episode when there is no history of prior depressive episodes. A depressive episode is characterised by a period of depressed mood or diminished interest in activities occurring most of the day, nearly every day during a period lasting at least two weeks accompanied by other symptoms such as difficulty concentrating, feelings of worthlessness or excessive or inappropriate guilt, hopelessness, recurrent thoughts of death or suicide, changes in appetite or sleep, psychomotor agitation or retardation, and reduced energy or fatigue. There have never been any prior manic, hypomanic, or mixed episodes, which would indicate the presence of a bipolar disorder."^^xsd:string ;
    skos:prefLabel "Single episode depressive"^^xsd:string .

icd-kg:Stimulants_including_amphetamines_methamphetamine_or_methcathinone a owl:Class ;
    icd-schema:exclusion icd-kg:Caffeine,
        icd-kg:Cocaine,
        icd-kg:Synthetic_cathinones,
        <http://id.who.int/icd/entity/154205648> ;
    rdfs:subClassOf icd-kg:Substance_use ;
    skos:definition "Disorders due to use of stimulants including amphetamines, methamphetamine or methcathinone are characterised by the pattern and consequences of use of these substances. There is a wide array of naturally occurring and synthetically produced psychostimulants other than cocaine. The most numerous of this group are the amphetamine-type substances, including methamphetamine. Prescribed stimulants including dexamphetamine are indicated for a limited number of conditions such as for Attention Deficit Hyperactivity Disorder. Methcathinone, known in many countries as ephedrone, is a synthetic potent stimulant that is a structural analogue of methamphetamine and is related to cathinone. All these drugs have primarily psychostimulant properties and are also vasoconstrictors to a varying degree. They induce euphoria and hyperactivity as may be seen in Stimulant Intoxication. They have potent dependence-producing properties, which may lead to the diagnosis of Stimulant Dependence and Stimulant Withdrawal following the cessation of use. Several Stimulant-Induced Mental Disorders are described."^^xsd:string ;
    skos:prefLabel "Stimulants including amphetamines methamphetamine or methcathinone"^^xsd:string .

icd-kg:Dementia a owl:Class ;
    icd-schema:exclusion icd-kg:Delirium,
        icd-kg:Neurodevelopmental,
        icd-kg:Of_intellectual_development,
        <http://id.who.int/icd/entity/1000337196>,
        <http://id.who.int/icd/entity/1328725971>,
        <http://id.who.int/icd/entity/835503193> ;
    icd-schema:inclusion "Dementia NOS"^^xsd:string ;
    rdfs:subClassOf icd-kg:Neurocognitive ;
    skos:definition "Dementia is characterized by the presence of marked impairment in two or more cognitive domains relative to that expected given the individual’s age and general premorbid level of cognitive functioning, which represents a decline from the individual’s previous level of functioning. Memory impairment is present in most forms of dementia, but cognitive impairment is not restricted to memory (i.e., there is impairment in other areas such as executive functions, attention, language, social cognition and judgment, psychomotor speed, visuoperceptual or visuospatial abilities). Neurobehavioural changes may also be present and, in some forms of dementia, may be the presenting symptom. Cognitive impairment is not attributable to normal aging and is severe enough to significantly interfere with independence in an individual’s performance of activities of daily living. The cognitive impairment is presumed to be attributable to an underlying acquired disease of the nervous system, a trauma, an infection or other disease process affecting the brain, or to use of specific substances or medications, nutritional deficiency or exposure to toxins, or the etiology may be undetermined. The impairment is not due to current substance intoxication or withdrawal."^^xsd:string ;
    skos:prefLabel "Dementia"^^xsd:string .

icd-kg:Dementia_diseases_classified_elsewhere a owl:Class ;
    rdfs:subClassOf icd-kg:Dementia ;
    skos:prefLabel "Dementia diseases classified elsewhere"^^xsd:string .

icd-kg:Disease a owl:Class ;
    icd-kg:hasDiagnosticRequirements icd-kg:DiagnosticCriteria ;
    owl:equivalentClass schema:Disease ;
    skos:definition "A disorder with homogeneous therapeutic possibilities and an identified pathophysiological mechanism. Developmental anomalies are excluded."^^xsd:string ;
    skos:prefLabel "Disease"^^xsd:string ;
    schema:signOrSymptom icd-kg:MedicalSignOrSymptom .

icd-kg:Obsessivecompulsive_or_related a owl:Class ;
    rdfs:subClassOf icd-kg:Mental_behavioural_or_neurodevelopmental_disorders ;
    skos:definition "Obsessive-compulsive and related disorders is a group of disorders characterised by repetitive thoughts and behaviours that are believed to share similarities in aetiology and key diagnostic validators. Cognitive phenomena such as obsessions, intrusive thoughts and preoccupations are central to a subset of these conditions (i.e., obsessive-compulsive disorder, body dysmorphic disorder, hypochondriasis, and olfactory reference disorder) and are accompanied by related repetitive behaviours. Hoarding Disorder is not associated with intrusive unwanted thoughts but rather is characterised by a compulsive need to accumulate possessions and distress related to discarding them. Also included in the grouping are body-focused repetitive behaviour disorders, which are primarily characterised by recurrent and habitual actions directed at the integument (e.g., hair-pulling, skin-picking) and lack a prominent cognitive aspect. The symptoms result in significant distress or significant impairment in personal, family, social, educational, occupational, or other important areas of functioning."^^xsd:string ;
    skos:prefLabel "Obsessivecompulsive or related"^^xsd:string .

icd-kg:Autism_spectrum a owl:Class ;
    icd-schema:exclusion <http://id.who.int/icd/entity/201200685> ;
    icd-schema:inclusion "Autistic disorder"^^xsd:string ;
    rdfs:subClassOf icd-kg:Neurodevelopmental ;
    skos:definition "Autism spectrum disorder is characterised by persistent deficits in the ability to initiate and to sustain reciprocal social interaction and social communication, and by a range of restricted, repetitive, and inflexible patterns of behaviour, interests or activities that are clearly atypical or excessive for the individual’s age and sociocultural context. The onset of the disorder occurs during the developmental period, typically in early childhood, but symptoms may not become fully manifest until later, when social demands exceed limited capacities. Deficits are sufficiently severe to cause impairment in personal, family, social, educational, occupational or other important areas of functioning and are usually a pervasive feature of the individual’s functioning observable in all settings, although they may vary according to social, educational, or other context. Individuals along the spectrum exhibit a full range of intellectual functioning and language abilities."^^xsd:string ;
    skos:prefLabel "Autism spectrum"^^xsd:string .

icd-kg:Bipolar_type_ii a owl:Class ;
    rdfs:subClassOf icd-kg:Bipolar_or_related ;
    skos:definition "Bipolar type II disorder is an episodic mood disorder defined by the occurrence of one or more hypomanic episodes and at least one depressive episode. A hypomanic episode is a persistent mood state lasting for at least several days characterised by persistent elevation of mood or increased irritability as well as increased activity or a subjective experience of increased energy, accompanied by other characteristic symptoms such as increased talkativeness, rapid or racing thoughts, increased self-esteem, decreased need for sleep, distractability, and impulsive or reckless behavior. The symptoms represent a change from the individual’s typical mood, energy level, and behavior but are not severe enough to cause marked impairment in functioning. A depressive episode is characterised by a period of depressed mood or diminished interest in activities occurring most of the day, nearly every day during a period lasting at least two weeks accompanied by other symptoms such as changes in appetite or sleep, psychomotor agitation or retardation, fatigue, feelings of worthless or excessive or inappropriate guilt, feelings or hopelessness, difficulty concentrating, and suicidality. There is no history of manic or mixed episodes."^^xsd:string ;
    skos:prefLabel "Bipolar type ii"^^xsd:string .

icd-kg:Neurodevelopmental a owl:Class ;
    rdfs:subClassOf icd-kg:Mental_behavioural_or_neurodevelopmental_disorders ;
    skos:definition "Neurodevelopmental disorders are behavioural and cognitive disorders that arise during the developmental period that involve significant difficulties in the acquisition and execution of specific intellectual, motor, language, or social functions. Although behavioural and cognitive deficits are present in many mental and behavioural disorders that can arise during the developmental period (e.g., Schizophrenia, Bipolar disorder), only disorders whose core features are neurodevelopmental are included in this grouping. The presumptive etiology for neurodevelopmental disorders is complex, and in many individual cases is unknown."^^xsd:string ;
    skos:prefLabel "Neurodevelopmental"^^xsd:string .

icd-kg:Bipolar_type_i a owl:Class ;
    icd-schema:exclusion icd-kg:Bipolar_type_ii,
        icd-kg:Cyclothymic ;
    rdfs:subClassOf icd-kg:Bipolar_or_related ;
    skos:definition "Bipolar type I disorder is an episodic mood disorder defined by the occurrence of one or more manic or mixed episodes. A manic episode is an extreme mood state lasting at least one week unless shortened by a treatment intervention characterised by euphoria, irritability, or expansiveness, and by increased activity or a subjective experience of increased energy, accompanied by other characteristic symptoms such as rapid or pressured speech, flight of ideas, increased self-esteem or grandiosity, decreased need for sleep, distractibility, impulsive or reckless behaviour, and rapid changes among different mood states (i.e., mood lability). A mixed episode is characterised by the presence of several prominent manic and several prominent depressive symptoms consistent with those observed in manic episodes and depressive episodes, which either occur simultaneously or alternate very rapidly (from day to day or within the same day). Symptoms must include an altered mood state consistent with a manic and/or depressive episode (i.e., depressed, dysphoric, euphoric or expansive mood), and be present most of the day, nearly every day, during a period of at least 2 weeks, unless shortened by a treatment intervention. Although the diagnosis can be made based on evidence of a single manic or mixed episode, typically manic or mixed episodes alternate with depressive episodes over the course of the disorder."^^xsd:string ;
    skos:prefLabel "Bipolar type i"^^xsd:string .

icd-kg:Substanceinduced_mood a owl:Class ;
    rdfs:subClassOf icd-kg:Mood ;
    skos:prefLabel "Substanceinduced mood"^^xsd:string .

icd-kg:Substance_use a owl:Class ;
    rdfs:subClassOf icd-kg:Substance_use_or_addictive_behaviours ;
    skos:definition "Disorders due to substance use include disorders that result from a single occasion or repeated use of substances that have psychoactive properties, including certain medications. Disorders related to fourteen classes or groups of psychoactive substances are included. Typically, initial use of these substances produces pleasant or appealing psychoactive effects that are rewarding and reinforcing with repeated use. With continued use, many of the included substances have the capacity to produce dependence. They also have the potential to cause numerous forms of harm, both to mental and physical health. Disorders due to harmful non-medical use of non-psychoactive substances are also included in this grouping."^^xsd:string ;
    skos:prefLabel "Substance use"^^xsd:string .

icd-kg:Mental_behavioural_or_neurodevelopmental_disorders a owl:Class ;
    icd-schema:exclusion <http://id.who.int/icd/entity/2009949293>,
        <http://id.who.int/icd/entity/505909942> ;
    rdfs:subClassOf icd-kg:Disease ;
    skos:definition "Mental, behavioural and neurodevelopmental disorders are syndromes characterised by clinically significant disturbance in an individual's cognition, emotional regulation, or behaviour that reflects a dysfunction in the psychological, biological, or developmental processes that underlie mental and behavioural functioning. These disturbances are usually associated with distress or impairment in personal, family, social, educational, occupational, or other important areas of functioning."^^xsd:string ;
    skos:prefLabel "Mental behavioural or neurodevelopmental disorders"^^xsd:string .

